# imports: https://w3id.org/semanticarts/ontology/gistCore12.0.1
# imports: https://w3id.org/treasuryoflives/ontology/tolCoreX.x.x

@prefix gist: <https://w3id.org/semanticarts/ns/ontology/gist/> .
@prefix owl: <http://www.w3.org/2002/07/owl#> .
@prefix rdf: <http://www.w3.org/1999/02/22-rdf-syntax-ns#> .
@prefix rdfs: <http://www.w3.org/2000/01/rdf-schema#> .
@prefix skos: <http://www.w3.org/2004/02/skos/core#> .
@prefix tolo: <https://w3id.org/treasuryoflives/ns/ontology/tol/> .
@prefix xsd: <http://www.w3.org/2001/XMLSchema#> .

<https://w3id.org/treasuryoflives/ontology/tolAdmin>
	a owl:Ontology ;
	owl:imports
		<https://w3id.org/semanticarts/ontology/gistCore12.0.1> ,
		<https://w3id.org/treasuryoflives/ontology/tolCoreX.x.x>
		;
	owl:versionIRI <https://w3id.org/treasuryoflives/ontology/tolAdminX.x.x> ;
	skos:definition "Classes and properties to support Treasury of Lives administrative functions."@en ;
	skos:prefLabel "Treasury of Lives Admin Ontology"@en ;
	gist:license "TBD"@en ;
	.

tolo:Rank
	a owl:Class ;
	rdfs:subClassOf gist:Category ;
	skos:definition "Relative standing or position."@en ;
	skos:example "Primary or secondary image of a person"@en ;
	skos:prefLabel "Rank"@en ;
	skos:scopeNote "Used primarily for non-numeric values. Numeric values can use gist:sequence."@en ;
	.

tolo:Subscription
	a owl:Class ;
	owl:equivalentClass [
		a owl:Class ;
		owl:intersectionOf (
			gist:TemporalRelation
			[
				a owl:Restriction ;
				owl:onProperty gist:hasParticipant ;
				owl:someValuesFrom gist:Organization ;
			]
			[
				a owl:Restriction ;
				owl:onProperty tolo:hasContactPerson ;
				owl:someValuesFrom gist:Person ;
			]
			[
				a owl:Restriction ;
				owl:onProperty gist:isCategorizedBy ;
				owl:someValuesFrom tolo:SubscriptionAccessType ;
			]
			[
				a owl:Restriction ;
				owl:onProperty gist:isCategorizedBy ;
				owl:someValuesFrom gist:EntityActiveStatus ;
			]
			[
				a owl:Restriction ;
				owl:onProperty gist:isCategorizedBy ;
				owl:someValuesFrom tolo:SubscriptionTier ;
			]
		) ;
	] ;
	skos:definition "A subscription to the Treasury of Lives website."@en ;
	skos:editorialNote "Add class equivalence based on property restrictions."@en ;
	skos:prefLabel "Subscription"@en ;
	.

tolo:SubscriptionAccessType
	a owl:Class ;
	rdfs:subClassOf
		gist:Category ,
		[
			a owl:Restriction ;
			owl:onProperty [
				owl:inverseOf gist:isCategorizedBy ;
			] ;
			owl:someValuesFrom tolo:Subscription ;
		]
		;
	skos:definition "Indicates how a subscriber is allowed to access the Treasury of Lives site. Values are IP-based or email. IP-based access requires one or more IP addresses to be registered."@en ;
	skos:prefLabel "Subscription Access Type"@en ;
	.

tolo:SubscriptionTier
	a owl:Class ;
	rdfs:subClassOf
		gist:Category ,
		[
			a owl:Restriction ;
			owl:onProperty [
				owl:inverseOf gist:isCategorizedBy ;
			] ;
			owl:someValuesFrom tolo:Subscription ;
		]
		;
	skos:definition "A level of subscription with specific privileges."@en ;
	skos:editorialNote "Using a category rather than an integer in case we want to attach information or apply SHACL validation to tiers."@en ;
	skos:prefLabel "Subscription Tier"@en ;
	.

tolo:UserAccount
	a owl:Class ;
	skos:definition "An account for a person with editing access to the Treasury of Lives website."@en ;
	skos:editorialNote "Tied to a person, has certain privileges."@en ;
	skos:prefLabel "User Account"@en ;
	.

tolo:createDateTime
	a owl:AnnotationProperty ;
	skos:definition "The timestamp of the creation of metadata related to some resource."@en ;
	skos:prefLabel "create datetime"@en ;
	.

tolo:domain
	a owl:DatatypeProperty ;
	skos:definition "An internet domain owned by a person or organization."@en ;
	skos:editorialNote "See whether we can get full URLs - then use url property."@en ;
	skos:example "stanford.edu, cornell.edu"@en ;
	skos:prefLabel "domain"@en ;
	skos:scopeNote "Note that these are not full URLs."@en ;
	.

tolo:editUrl
	a owl:AnnotationProperty ;
	skos:definition "Links a piece of content in HTML format, such as a biography, summary, description, etc., to an HTML editor where it can be edited."@en ;
	skos:prefLabel "edit URL"@en ;
	skos:scopeNote "This is a temporary workaround because the primary editing platform has no built-in HTML editor. Once this is implemented this property can be removed."@en ;
	.

tolo:fileName
	a owl:DatatypeProperty ;
	rdfs:range xsd:string ;
	skos:definition "The name of a file, such as an image file."@en ;
	skos:editorialNote "Should this go in the admin or display ontology? Is it an annotation property?"@en ;
	skos:prefLabel "file name"@en ;
	.

tolo:filePath
	a owl:DatatypeProperty ;
	rdfs:range xsd:string ;
	skos:definition "The full path to a file, such as an image file."@en ;
	skos:editorialNote "Should this go in the admin or display ontology? Is it an annotation property?"@en ;
	skos:prefLabel "file path"@en ;
	.

tolo:hasContactPerson
	a owl:ObjectProperty ;
	rdfs:range gist:Person ;
	skos:definition "The contact person for an organization or temporal relation such as a subscription."@en ;
	skos:prefLabel "has contact person"@en ;
	.

tolo:hasThumbnail
	a owl:ObjectProperty ;
	rdfs:domain tolo:Image ;
	rdfs:range tolo:Image ;
	skos:definition "Relates an image to a reduced-size version used to help in recognizing and organizing a collection of images."@en ;
	skos:editorialNote "Should this go in the admin or display ontology? Is it an annotation property?"@en ;
	skos:prefLabel "has thumbnail"@en ;
	.

tolo:ipAddress
	a owl:DatatypeProperty ;
	rdfs:range xsd:string ;
	skos:altLabel "IP address"@en ;
	skos:definition "A numberic label assigned to a device connected to a computer network that uses the Internet Protocol for communication. IP addresses serve two main functions: network interface identification and location addressing."@en ;
	skos:editorialNote "Could define class IpAddress as subclass of gist:Address, but doesn't seem necessary."@en ;
	skos:prefLabel "internet protocol address"@en ;
	skos:scopeNote "Subscribers with IP access (see tolo:SubscriptionAccessType) register one or more IP addresses through which they are authorized to access subscriber content on the Treasury of Lives site. Value can be either a full or wildcarded IP address."@en ;
	.

tolo:isCreatedBy
	a owl:ObjectProperty ;
	rdfs:range tolo:UserAccount ;
	skos:definition "The user account which created metadata related to some resource, such as an image."@en ;
	skos:prefLabel "is created by"@en ;
	.

tolo:isLastModifiedBy
	a owl:ObjectProperty ;
	rdfs:range tolo:UserAccount ;
	skos:definition "The user account which last modified metadata related to some resource, such as an image."@en ;
	skos:prefLabel "is last modified by"@en ;
	.

tolo:lastModifiedDateTime
	a owl:DatatypeProperty ;
	rdfs:subPropertyOf gist:atDateTime ;
	skos:definition "The timestamp of the last modification of metadata related to some resource."@en ;
	skos:prefLabel "last modified datetime"@en ;
	.

tolo:sourceUrl
	a owl:DatatypeProperty ;
	rdfs:range xsd:anyURI ;
	skos:definition "The URL of the source of an image or other content."@en ;
	skos:prefLabel "source URL"@en ;
	.

