# imports: https://w3id.org/semanticarts/ontology/gistCore12.1.0

@prefix bdo: <http://purl.bdrc.io/ontology/core/> .
@prefix gist: <https://w3id.org/semanticarts/ns/ontology/gist/> .
@prefix media-txt: <https://www.iana.org/assignments/media-types/text/> .
@prefix owl: <http://www.w3.org/2002/07/owl#> .
@prefix rdf: <http://www.w3.org/1999/02/22-rdf-syntax-ns#> .
@prefix rdfs: <http://www.w3.org/2000/01/rdf-schema#> .
@prefix skos: <http://www.w3.org/2004/02/skos/core#> .
@prefix told: <https://w3id.org/treasuryoflives/ns/data/tol/> .
@prefix tolo: <https://w3id.org/treasuryoflives/ns/ontology/tol/> .
@prefix tolx: <https://w3id.org/treasuryoflives/ns/taxonomy/tol/> .
@prefix wiki: <https://www.wikidata.org/wiki/> .
@prefix xsd: <http://www.w3.org/2001/XMLSchema#> .

<https://w3id.org/treasuryoflives/ontology/tolCoreX.x.x>
	a owl:Ontology ;
	owl:imports <https://w3id.org/semanticarts/ontology/gistCore12.1.0> ;
	owl:versionIRI <https://w3id.org/treasuryoflives/ontology/tolCoreX.x.x> ;
	skos:definition "The Treasury of Lives Core Ontology enables the description of historical and contemporary figures in the culture and religion of Tibet, Inner Asia, and the Himalaya. It is used by the Treasury of Lives born-digitial biographical collection (https://treasuryoflives.org) to publish and share its data as Linked Open Data, facilitate the consumption of external RDF, and to to enhance the narrative text with structured data."@en ;
	skos:editoralNote "Add rdfs:isDefinedBy using onto-toolkit."@en ;
	skos:editorialNote """
		Temporarily removing imports:
			<http://id.loc.gov/ontologies/bibframe-2-1-0> ,
			<http://purl.bdrc.io/ontology/core> to make Protege easier to read."""@en ;
	skos:prefLabel "Treasury of Lives Core Ontology"@en ;
	gist:license "TBD"@en ;
	.

gist:EntityActiveStatus
	a owl:Class ;
	rdfs:subClassOf gist:Category ;
	skos:definition "Indicates whether an entity is active or inactive."@en ;
	skos:prefLabel "Entity Active Status"@en ;
	skos:scopeNote "Can be applied to many types of entities."@en ;
	.

tolo:Author
	a owl:Class ;
	rdfs:subClassOf gist:Person ;
	skos:definition "A person who has authored or contributed to authoring at least one work."@en ;
	skos:prefLabel "Author"@en ;
	.

tolo:AuthorStatement
	a owl:Class ;
	owl:equivalentClass [
		a owl:Class ;
		owl:intersectionOf (
			gist:Text
			[
				a owl:Restriction ;
				owl:onProperty [
					owl:inverseOf tolo:hasStatement ;
				] ;
				owl:someValuesFrom tolo:Biography ;
			]
		) ;
	] ;
	skos:definition "A disclaimer or disclosure about the author of a biography."@en ;
	skos:example "A statement indicating that the author of the biography is a relative or student of its subject."@en ;
	skos:prefLabel "Author Statement"@en ;
	.

tolo:Authorship
	a owl:Class ;
	owl:equivalentClass [
		a owl:Class ;
		owl:intersectionOf (
			gist:TemporalRelation
			[
				a owl:Restriction ;
				owl:onProperty gist:hasParticipant ;
				owl:someValuesFrom tolo:Author ;
			]
			[
				a owl:Restriction ;
				owl:onProperty gist:hasParticipant ;
				owl:someValuesFrom tolo:Biography ;
			]
		) ;
	] ;
	skos:definition "Relates a bio to a person who has authored it."@en ;
	skos:editorialNote
		"Though there is a display order of multiple authors of a single biography, we do not currently distinguish primary from secondary author in the model, because there may be more than two authors and we still need to specify the display order."@en ,
		"Using a simple model of authorship until there is a use case for a more complex model with a generic Contribution class and roles as in BIBFRAME."@en
		;
	skos:prefLabel "Authorship"@en ;
	.

tolo:Biography
	a owl:Class ;
	rdfs:subClassOf
		gist:FormattedContent ,
		[
			a owl:Restriction ;
			owl:onProperty gist:isAbout ;
			owl:someValuesFrom tolo:Person ;
		]
		;
	skos:definition "A written account of another person's life."@en ;
	skos:editorialNote "If we want to bring BIBFRAME into the mix, would be a subclass of bf:Work."@en ;
	skos:prefLabel "Biography"@en ;
	skos:scopeNote "Author bios are not tolo:Biographies because authors are instances of gist:Person but not tolo:Person."@en ;
	.

tolo:Birth
	a owl:Class ;
	rdfs:subClassOf
		gist:HistoricalEvent ,
		gist:PhysicalEvent ,
		[
			a owl:Restriction ;
			owl:onProperty tolo:isEventOf ;
			owl:allValuesFrom tolo:Person ;
		] ,
		[
			a owl:Restriction ;
			owl:onProperty gist:occursIn ;
			owl:cardinality "1"^^xsd:nonNegativeInteger ;
		] ,
		[
			a owl:Restriction ;
			owl:onProperty tolo:isEventOf ;
			owl:cardinality "1"^^xsd:nonNegativeInteger ;
		] ,
		[
			a owl:Restriction ;
			owl:onProperty tolo:inYear ;
			owl:minCardinality "1"^^xsd:nonNegativeInteger ;
		]
		;
	skos:definition "TBD"@en ;
	skos:prefLabel "Birth"@en ;
	.

tolo:Death
	a owl:Class ;
	rdfs:subClassOf
		gist:HistoricalEvent ,
		gist:PhysicalEvent ,
		[
			a owl:Restriction ;
			owl:onProperty tolo:isEventOf ;
			owl:allValuesFrom tolo:Person ;
		] ,
		[
			a owl:Restriction ;
			owl:onProperty gist:occursIn ;
			owl:cardinality "1"^^xsd:nonNegativeInteger ;
		] ,
		[
			a owl:Restriction ;
			owl:onProperty tolo:isEventOf ;
			owl:cardinality "1"^^xsd:nonNegativeInteger ;
		] ,
		[
			a owl:Restriction ;
			owl:onProperty tolo:inYear ;
			owl:minCardinality "1"^^xsd:nonNegativeInteger ;
		]
		;
	skos:definition "TBD"@en ;
	skos:editorialNote "Can deities have birth and death? We may need to loosen the restriction."@en ;
	skos:prefLabel "Death"@en ;
	.

tolo:Founding
	a owl:Class ;
	rdfs:subClassOf gist:Event ;
	skos:definition "The event of establishng or originating an institution such as a monastery. A founding object is used to attach various dates (year, alternate year, century, etc.), as well as the founder, to the institution."@en ;
	skos:prefLabel "Founding"@en ;
	.

tolo:HistoricalPeriod
	a owl:Class ;
	rdfs:subClassOf gist:TimeInterval ;
	skos:definition "A named time interval with historical significance."@en ;
	skos:example "The 10th century, the eary/mid/late 19th century."@en ;
	skos:prefLabel "Historical Period"@en ;
	skos:scopeNote "Whereas a time interval is any period of time, such as 2-4pm this afternoon or 1848-1947, a historical period is named and cited in relation to historical events or culture. Historical periods include full and partial centuries, which are ordinally numbered."@en ;
	.

tolo:HusbandStatus
	a owl:Class ;
	rdfs:subClassOf
		gist:Category ,
		[
			a owl:Restriction ;
			owl:onProperty [
				owl:inverseOf gist:isCategorizedBy ;
			] ;
			owl:allValuesFrom tolo:Marriage ;
		]
		;
	skos:definition "Indicates whether a marriage relationship has a junior or senior husband."@en ;
	skos:example "Junior, senior"@en ;
	skos:prefLabel "Husband Status"@en ;
	.

tolo:IdType
	a owl:Class ;
	rdfs:subClassOf gist:Category ;
	skos:definition "A kind of identifier, usually associated with an allocating organization."@en ;
	skos:example "Gendun Drub has Himalayan Art (HAR) identifier 582."@en ;
	skos:prefLabel "ID Type"@en ;
	skos:scopeNote "The ID type is used to construct links by specifying a URL fragment to combine with the identifier to form a URL and a display label to use as link text."@en ;
	.

tolo:Incarnation
	a owl:Class ;
	rdfs:subClassOf
		[
			a owl:Restriction ;
			owl:onProperty [
				owl:inverseOf gist:hasMember ;
			] ;
			owl:allValuesFrom tolo:IncarnationLineage ;
		] ,
		[
			a owl:Restriction ;
			owl:onProperty gist:providesOrderFor ;
			owl:allValuesFrom tolo:Person ;
		]
		;
	owl:equivalentClass [
		a owl:Class ;
		owl:intersectionOf (
			tolo:LineageMember
			[
				a owl:Restriction ;
				owl:onProperty [
					owl:inverseOf gist:hasMember ;
				] ;
				owl:someValuesFrom tolo:IncarnationLineage ;
			]
			[
				a owl:Restriction ;
				owl:onProperty gist:providesOrderFor ;
				owl:someValuesFrom tolo:Person ;
			]
			[
				a owl:Restriction ;
				owl:onProperty gist:sequence ;
				owl:someValuesFrom xsd:integer ;
			]
			[
				a owl:Restriction ;
				owl:onProperty tolo:ordinal ;
				owl:someValuesFrom xsd:integer ;
			]
		) ;
	] ;
	skos:definition "The relationship connecting a person to an incarnation lineage and expressing the sequence and ordinal of the person in the lineage."@en ;
	skos:editorialNote "Connects person to lineage."@en ;
	skos:example "The Third Dalai Lama."@en ;
	skos:prefLabel
		"Incarnation"@en ,
		"sprul sku"@bo-x-ewts
		;
	skos:scopeNote "The sequence and ordinal may differ in some cases, and in some cases there may be no ordinal."@en ;
	.

tolo:IncarnationLineage
	a owl:Class ;
	rdfs:subClassOf [
		a owl:Restriction ;
		owl:onProperty gist:hasMember ;
		owl:allValuesFrom tolo:Incarnation ;
	] ;
	owl:equivalentClass [
		a owl:Class ;
		owl:intersectionOf (
			tolo:Lineage
			[
				a owl:Restriction ;
				owl:onProperty gist:hasMember ;
				owl:someValuesFrom tolo:Incarnation ;
			]
		) ;
	] ;
	skos:definition "A consecutive line of people regarded as incarnations of a non-living person or mythical figure."@en ;
	skos:example "The Dalai Lamas, the Karmapas."@en ;
	skos:prefLabel
		"Incarnation Lineage"@en ,
		"skye brgyud"@bo-x-ewts
		;
	skos:scopeNote "An incarnation lineage is enumerated chronologically and can branch into multiple lines. Usually associated with a seat, such as a monastery, and a tradition."@en ;
	.

tolo:KinshipGroup
	a owl:Class ;
	rdfs:subClassOf
		gist:Collection ,
		[
			a owl:Restriction ;
			owl:onProperty gist:hasMember ;
			owl:allValuesFrom [
				a owl:Class ;
				owl:unionOf (
					tolo:Person
					tolo:Marriage
					tolo:RulerLineage
				) ;
			] ;
		]
		;
	skos:definition "A social unit consisting of people with a common ancestor."@en ;
	skos:example "The Adro clan; the Jangling family."@en ;
	skos:prefLabel "Kinship Group"@en ;
	skos:scopeNote "Includes Tibetan concepts that may individually mean something more specific, such as: rig (rigs) for clan, race, family; gyu (rgyud) for lineage, descent; dungrab (gdung rabs) for descendants, lineage, generation; dung (gdung) for progeny, descendants, lineage, descent line; ru (rus) for bone, bloodline, lineage, family, clan; khang (khang) for household and tsang (tshang) for family and household. Marriages are also members of kinship groups, distinguishing patrilocal from matrilocal marriages."@en ;
	.

tolo:KinshipGroupType
	a owl:Class ;
	owl:equivalentClass [
		owl:intersectionOf (
			gist:Category
			[
				a owl:Restriction ;
				owl:onProperty [
					owl:inverseOf gist:isCategorizedBy ;
				] ;
				owl:allValuesFrom tolo:KinshipGroup ;
			]
		) ;
	] ;
	skos:definition "A type of kinship group."@en ;
	skos:example "Lhasa Aristocracy."@en ;
	skos:prefLabel "Kinship Group Type"@en ;
	skos:scopeNote "Currently only one type is defined."@en ;
	.

tolo:Lineage
	a owl:Class ;
	owl:equivalentClass [
		a owl:Class ;
		owl:intersectionOf (
			gist:OrderedCollection
			[
				a owl:Restriction ;
				owl:onProperty gist:hasMember ;
				owl:allValuesFrom tolo:LineageMember ;
			]
			[
				a owl:Restriction ;
				owl:onProperty gist:hasMember ;
				owl:someValuesFrom tolo:LineageMember ;
			]
		) ;
	] ;
	skos:definition "A line of persons serving in a certain role or function, such as the heads of a particular monastery or an incarnation lineage."@en ;
	skos:prefLabel "Lineage"@en ;
	.

tolo:LineageMember
	a owl:Class ;
	rdfs:subClassOf
		gist:OrderedMember ,
		[
			a owl:Restriction ;
			owl:onProperty gist:sequence ;
			owl:someValuesFrom xsd:integer ;
		] ,
		[
			a owl:Restriction ;
			owl:onProperty tolo:ordinal ;
			owl:someValuesFrom xsd:integer ;
		]
		;
	skos:definition "TBD"@en ;
	skos:prefLabel "Lineage Member"@en ;
	.

tolo:Marriage
	a owl:Class ;
	owl:equivalentClass [
		owl:intersectionOf (
			gist:Agreement
			[
				a owl:Restriction ;
				owl:onProperty tolo:hasWife ;
				owl:someValuesFrom tolo:Person ;
			]
			[
				a owl:Restriction ;
				owl:onProperty tolo:hasHusband ;
				owl:someValuesFrom tolo:Person ;
			]
			[
				a owl:Restriction ;
				owl:onProperty [
					owl:inverseOf gist:hasMember ;
				] ;
				owl:someValuesFrom tolo:KinshipGroup ;
			]
		) ;
	] ;
	skos:definition "A culturally and often legally recognized union between two people, called spouses, that establishes rights and obligations between them."@en ;
	skos:prefLabel "Marriage"@en ;
	skos:scopeNote "A marriage is associated with the birth kinship group of either the father ('patrilocal') or mother ('matrilocal')."@en ;
	.

tolo:MarriageTerminationCause
	a owl:Class ;
	rdfs:subClassOf
		gist:Category ,
		[
			a owl:Restriction ;
			owl:onProperty [
				owl:inverseOf gist:isCategorizedBy ;
			] ;
			owl:allValuesFrom tolo:Marriage ;
		]
		;
	skos:definition "The reason for the termination of a marriage."@en ;
	skos:example "Death, divorce, dissolution."@en ;
	skos:prefLabel "Marriage Termination Cause"@en ;
	.

tolo:MarriageType
	a owl:Class ;
	rdfs:subClassOf
		gist:Category ,
		[
			a owl:Restriction ;
			owl:onProperty [
				owl:inverseOf gist:isCategorizedBy ;
			] ;
			owl:allValuesFrom tolo:Marriage ;
		]
		;
	skos:definition "A category characterizing a marriage as either matrilocal or patrilocal (default)."@en ;
	skos:editorialNote "Is this used? I think now we connect a marriage to a kinship group."@en ;
	skos:prefLabel "Marriage Type"@en ;
	.

tolo:Monastery
	a owl:Class ;
	owl:equivalentClass [
		a owl:Class ;
		owl:intersectionOf (
			gist:Place
			[
				a owl:Restriction ;
				owl:onProperty gist:isCategorizedBy ;
				owl:oneOf (
					tolx:_PlaceType_monastery
					tolx:_PlaceType_nunnery
				) ;
			]
		) ;
	] ;
	skos:definition "A community of ordained individuals affiliated with a particular religious tradition with a common annual ritual calendar and rules. The community is organized hierarchically, with established roles such as abbot, treasurer, and the like. Human-created structures such as temples, assembly halls, residential houses and meditation halls are typical features."@en ;
	skos:editorialNote "Has a founder, has monastery lineage, ..."@en ;
	skos:prefLabel
		"Monastery"@en ,
		"dgon pa"@bo-x-ewts ,
		"དགོན་པ་"@bo ,
		"寺院"@zh-HANI
		;
	skos:scopeNote "This term designates both the community and the physical structures that house it. Note that nunneries are included but differentiated by a different taxonomic type."@en ;
	.

tolo:MonasteryHead
	a owl:Class ;
	rdfs:subClassOf
		[
			a owl:Restriction ;
			owl:onProperty [
				owl:inverseOf gist:hasMember ;
			] ;
			owl:allValuesFrom tolo:MonasteryHeadLineage ;
		] ,
		[
			a owl:Restriction ;
			owl:onProperty gist:providesOrderFor ;
			owl:allValuesFrom tolo:Person ;
		]
		;
	owl:equivalentClass [
		a owl:Class ;
		owl:intersectionOf (
			gist:OrderedMember
			[
				a owl:Restriction ;
				owl:onProperty [
					owl:inverseOf gist:hasMember ;
				] ;
				owl:someValuesFrom tolo:MonasteryHeadLineage ;
			]
			[
				a owl:Restriction ;
				owl:onProperty gist:providesOrderFor ;
				owl:someValuesFrom tolo:Person ;
			]
			[
				a owl:Restriction ;
				owl:onProperty gist:sequence ;
				owl:someValuesFrom xsd:integer ;
			]
		) ;
	] ;
	skos:definition "TBD"@en ;
	skos:prefLabel "Monastery Head"@en ;
	.

tolo:MonasteryHeadLineage
	a owl:Class ;
	rdfs:subClassOf [
		a owl:Restriction ;
		owl:onProperty gist:hasMember ;
		owl:allValuesFrom tolo:MonasteryHead ;
	] ;
	owl:disjointWith tolo:IncarnationLineage ;
	owl:equivalentClass
		[
			a owl:Class ;
			owl:intersectionOf (
				gist:OrderedCollection
				[
					a owl:Restriction ;
					owl:onProperty gist:hasMember ;
					owl:someValuesFrom tolo:MonasteryHead ;
				]
			) ;
		] ,
		[
			a owl:Class ;
			owl:intersectionOf (
				tolo:Lineage
				[
					a owl:Restriction ;
					owl:onProperty gist:hasMember ;
					owl:someValuesFrom [
						a owl:Restriction ;
						owl:onProperty gist:isCategorizedBy ;
						owl:someValuesFrom tolx:_Role_monastery_head ;
					] ;
				]
				[
					a owl:Restriction ;
					owl:onProperty gist:isConnectedTo ;
					owl:someValuesFrom tolo:Monastery ;
				]
			) ;
		]
		;
	skos:definition
		"A consecutive line of monastery heads."@en ,
		"A lineage of heads of a particular monastery."@en
		;
	skos:editorialNote
		"Are there discrepancies between ordinal and sequence as for incarnations?"@en ,
		"We may just use the generic Lineage instead."@en
		;
	skos:prefLabel "Monastery Head Lineage"@en ;
	.

tolo:MonasteryLineage
	a owl:Class ;
	owl:equivalentClass [
		a owl:Class ;
		owl:intersectionOf (
			tolo:Lineage
			[
				a owl:Restriction ;
				owl:onProperty gist:isCategorizedBy ;
				owl:oneOf (
					tolx:_Role_monastery_head
					tolx:_Role_lay_administrator
				) ;
			]
			[
				a owl:Restriction ;
				owl:onProperty gist:isConnectedTo ;
				owl:someValuesFrom tolo:Monastery ;
			]
		) ;
	] ;
	skos:definition "A lineage of heads or lay administrators of a particular monastery."@en ;
	skos:editorialNote "The role is attached to the lineage rather than the individual lineage members, as this makes the most sense; however, it creates a different triple pattern from the non-lineage one where roles are connected directly to persons."@en ;
	skos:example "Katok Khenpo, Drepung are monastery head lineages."@en ;
	skos:prefLabel "Monastery Lineage"@en ;
	.

tolo:Person
	a owl:Class ;
	rdfs:subClassOf
		bdo:Person ,
		gist:Person ,
		wiki:Person
		;
	skos:definition "An individual being who was born, lived, and died in the human realm and is or potentiallly is the subject of a Treasury of Lives biography."@en ;
	skos:prefLabel
		"Person"@en ,
		"mi"@bo-x-ewts
		;
	skos:scopeNote "May include quasi-historical figures. Encompasses persons from other data sources, such as BDRC, who are referenced from biographies but do not have a biography on the ToL site. Other persons in the data such as users, subscriber contacts, and authors are instances of gist:Person rather than tolo:Person (unless they also become the subject of a biography)."@en ;
	.

tolo:PlaceType
	a owl:Class ;
	rdfs:subClassOf
		gist:Category ,
		[
			a owl:Restriction ;
			owl:onProperty [
				owl:inverseOf gist:isCategorizedBy ;
			] ;
			owl:allValuesFrom gist:Place ;
		]
		;
	skos:definition "A category indicating a kind of place based on natural features or human-designated function."@en ;
	skos:example "Lake, mountain, monastery, school, temple, hermitage."@en ;
	skos:prefLabel "Place Type"@en ;
	skos:scopeNote
		"Some places may have more than one type; e.g., a cave may also function as a hermitage."@en ,
		"There is no clear line between what we might think of as institutions or organizations, such as a monastic order, and the physical structures that house them, so they are all typed as gist:Place and categorized with a tolo:PlaceType."@en
		;
	.

tolo:Role
	a owl:Class ;
	rdfs:subClassOf gist:Category ;
	skos:definition "A role, office, or vocation played by a person, typically, though not always, in an institutional context."@en ;
	skos:example "Artist, government officer, monastic officer, Indian master."@en ;
	skos:prefLabel "Role"@en ;
	.

tolo:RulerLineage
	a owl:Class ;
	owl:equivalentClass [
		a owl:Class ;
		owl:intersectionOf (
			tolo:Lineage
			[
				a owl:Restriction ;
				owl:onProperty gist:isCategorizedBy ;
				owl:hasValue tolx:_Role_ruler ;
			]
			[
				a owl:Restriction ;
				owl:onProperty gist:isConnectedTo ;
				owl:someValuesFrom gist:GeoRegion ;
			]
			[
				a owl:Restriction ;
				owl:onProperty [
					owl:inverseOf gist:hasMember ;
				] ;
				owl:someValuesFrom tolo:KinshipGroup ;
			]
		) ;
	] ;
	skos:definition "A lineage of members of a royal family who inherit the role of ruler of the home region. In addition to a kinship group and region, the lineage may also be associated with a place or institution, such as a palace or monastery."@en ;
	skos:editorialNote "The role is attached to the lineage rather than the individual lineage members, as this makes the most sense; however, it creates a different triple pattern from the non-lineage one where roles are connected directly to persons."@en ;
	skos:example "Derge, Chone."@en ;
	skos:prefLabel "Ruler Lineage"@en ;
	.

tolo:StatusAssignment
	a owl:Class ;
	rdfs:subClassOf gist:TemporalRelation ;
	skos:definition "A temporal object expressing a relationship between some resource and a status it is assigned, used to add datetimes, notes, assigner, and other data."@en ;
	skos:prefLabel "Status Assignment"@en ;
	skos:scopeNote "Status assignments will have an actual start datetime, as well as an actual end datetime if there is a subsequent assignment of a different value in the same taxonomy (e.g., from EntityActiveStatus_active to EntityActiveStatus_inactive). The end date of one will be the start date of the next one. Consistency in both precision (use of datetime rather than date) and start/end vs single dates is recommended for ease of querying, even if only date precision is required in specific cases."@en ;
	.

tolo:TeacherStudentRelationship
	a owl:Class ;
	owl:equivalentClass [
		a owl:Class ;
		owl:intersectionOf (
			gist:TemporalRelation
			gist:Agreement
			[
				a owl:Restriction ;
				owl:onProperty gist:hasGiver ;
				owl:someValuesFrom tolo:Person ;
			]
			[
				a owl:Restriction ;
				owl:onProperty gist:hasRecipient ;
				owl:someValuesFrom tolo:Person ;
			]
			[
				a owl:Restriction ;
				owl:onProperty gist:conformsTo ;
				owl:someValuesFrom tolo:Tradition ;
			]
		) ;
	] ;
	skos:definition "A time-delimited relationship between a teacher and a student."@en ;
	skos:prefLabel "Teacher-Student Relationship"@en ;
	.

tolo:Tradition
	a owl:Class ;
	rdfs:subClassOf gist:Intention ;
	skos:definition "An instance of Tibetan religion that identifies as a cohesive group with distinct modes of ritual and learning, as well as associated institutions such as monasteries."@en ;
	skos:example "The major schools and subschools of Tibetan Buddhism as well as Bon."@en ;
	skos:prefLabel
		"Tradition"@en ,
		"chos lugs"@bo-x-ewts
		;
	.

tolo:Vocation
	a owl:Class ;
	owl:equivalentClass [
		a owl:Class ;
		owl:intersectionOf (
			gist:TemporalRelation
			[
				a owl:Restriction ;
				owl:onProperty gist:hasParticipant ;
				owl:someValuesFrom tolo:Person ;
			]
			[
				a owl:Restriction ;
				owl:onProperty gist:isCategorizedBy ;
				owl:someValuesFrom tolo:Role ;
			]
		) ;
	] ;
	skos:definition "Relates a person to a role played by that person, possibly for a defined period of time."@en ;
	skos:prefLabel "Vocation"@en ;
	.

tolo:Website
	a owl:Class ;
	rdfs:subClassOf
		gist:Content ,
		gist:Network
		;
	skos:definition "A collection of one or more web pages and related content that is identified by a common domain name and published on at least one web server."@en ;
	skos:example "Lotsawa House, Rubin Museum of Art"@en ;
	skos:prefLabel "Website"@en ;
	.

tolo:WifeStatus
	a owl:Class ;
	rdfs:subClassOf
		gist:Category ,
		[
			a owl:Restriction ;
			owl:onProperty [
				owl:inverseOf gist:isCategorizedBy ;
			] ;
			owl:allValuesFrom tolo:Marriage ;
		]
		;
	skos:definition "Indicates whether a marriage relationship has a junior or senior wife."@en ;
	skos:example "Junior, senior"@en ;
	skos:prefLabel "Wife Status"@en ;
	.

tolo:WorkType
	a owl:Class ;
	rdfs:subClassOf gist:Category ;
	skos:definition "A category of work or intellectual property based on materials, form, or content."@en ;
	skos:example "Painting, sculpture, rock carving, letter, initiation card."@en ;
	skos:prefLabel "Work Type"@en ;
	.

tolo:actualYear
	a owl:DatatypeProperty ;
	rdfs:subPropertyOf tolo:inYear ;
	skos:definition "The year in which something existed or took place."@en ;
	skos:example "Gyergom Tsultime Sengge was born in 1144 and died in 1204."@en ;
	skos:prefLabel "actual year"@en ;
	.

tolo:alternateYear
	a owl:DatatypeProperty ;
	rdfs:subPropertyOf tolo:inYear ;
	skos:definition "The year in which something is proposed to have existed or taken place."@en ;
	skos:example "According to one source, Botrul Dongak Tenpai Nyima was born in 1900, while according to another source his birth year was XXX and he died in 1902. No indication of greater or less likelihood of the two possibilities is implied."@en ;
	skos:prefLabel "alternate year"@en ;
	skos:scopeNote "Differs from tolo:approximateYear, which specifies a single year but is intended to be inexact. In this case, various scholars have proposed different years. If there is an alternate year, there is no actual year; rather, both proposed dates are asserted as alternates."@en ;
	.

tolo:approximateEndYear
	a owl:DatatypeProperty ;
	rdfs:subPropertyOf tolo:inYear ;
	skos:definition "The approximate year in which an event or relationship, such as a marriage, ended."@en ;
	skos:prefLabel "approximate end year"@en ;
	.

tolo:approximateStartYear
	a owl:DatatypeProperty ;
	rdfs:subPropertyOf tolo:inYear ;
	skos:definition "The approximate year in which an event or relationship, such as a marriage, began."@en ;
	skos:prefLabel "approximate start year"@en ;
	.

tolo:approximateYear
	a owl:DatatypeProperty ;
	rdfs:subPropertyOf tolo:inYear ;
	skos:definition "The approximate year in which something existed or took place."@en ;
	skos:example "The birth event of Lhagyari Namgyel Gyatso took place in approximately 1927."@en ;
	skos:prefLabel "approximate year"@en ;
	skos:scopeNote "Differs from tolo:alternateYear, which is used when there is more than one proposed year. In this case, only one year is asserted, but it is intended to be inexact, thus encompassing some number of years before and/or after."@en ;
	.

tolo:birthFamilyName
	a owl:DatatypeProperty ;
	rdfs:subPropertyOf tolo:familyName ;
	rdfs:domain tolo:Person ;
	rdfs:range rdf:langString ;
	skos:definition "The family name a person is assigned at birth."@en ;
	skos:editorialNote "Not sure we need this - we might link to genealogical groups by birth or by marriage."@en ;
	skos:prefLabel "birth family name"@en ;
	skos:scopeNote "A family name other than the birth name can be acquired through marriage."@en ;
	.

tolo:creationDate
	a owl:DatatypeProperty ;
	rdfs:subClassOf gist:atDateTime ;
	skos:definition "The date something was created, with day precision."@en ;
	skos:prefLabel "creation date"@en ;
	skos:scopeNote "Differs from the timestamp when the image metadata was entered into the database."@en ;
	gist:domainIncludes
		gist:Content ,
		gist:IntellectualProperty
		;
	.

tolo:credit
	a owl:DatatypeProperty ;
	rdfs:domain gist:FormattedContent ;
	rdfs:range xsd:string ;
	skos:definition "A note acknowledging the source of an image."@en ;
	skos:editorialNote "Should this go in the admin or display ontology?"@en ;
	skos:prefLabel "credit"@en ;
	skos:scopeNote "Note that the credit applies to the image file, not the work of art it depicts."@en ;
	.

tolo:depicts
	a owl:ObjectProperty ;
	skos:definition "Relates an image or work of art such as a painting or sculpture to an object it represents."@en ;
	skos:example "The painting identified as HAR 65789 depicts Sachen Kunga Nyingpo; the ivory sculpture identified as HAR 65232 depicts Lhachok Sengge."@en ;
	skos:prefLabel "depicts"@en ;
	skos:scopeNote
		"Image files as well as the works themselves can serve as the subject of this property. E.g., a specific JPG file depicts the HAR 65789 painting; that painting depicts Sachen Kunga Nyingpo. Indirectly we can say that the file depicts the person, though it is not currently clear that the relationship is always transitive."@en ,
		"The object depicted does not have to be a concrete, physical thing; it could be an abstract concept, or an artwork may depict nothing."@en ,
		"This property typically applies to visual representation, as opposed to gist:isAbout, which applies to textual description or representation."@en
		;
	gist:domainIncludes
		gist:FormattedContent ,
		gist:IntellectualProperty
		;
	.

tolo:dissolutionYear
	a owl:DatatypeProperty ;
	rdfs:subPropertyOf gist:actualEndYear ;
	skos:definition "The year an agreement such as marriage was ended. In the case of marriage, this refers to divorce rather than the end of a marriage by death of one of the spouses."@en ;
	skos:editorialNote
		"Use if we need to distinguish divorce from death as the end of a marriage."@en ,
		"We may want to do this like birth and death - have a Dissolution object with a year. If there are many things with actual/approximate/alternate values, (dissolution, founding, etc.) we should establish this as a general pattern."@en
		;
	skos:prefLabel "dissolution year"@en ;
	.

tolo:existsDuring
	a owl:ObjectProperty ;
	skos:definition "Relates an entity to an event, time period, or other temporal object during which it does or did exist."@en ;
	skos:example "Trimalo lived during the 7th century; Dorje Sherab lived during the 12th and 13th centuries."@en ;
	skos:prefLabel "exists during"@en ;
	skos:scopeNote "The subject of tolo:existsDuring is a non-temporal resource. The property contrasts with tolo:occursDuring, which relates a temporal resource to a containing temporal resource."@en ;
	gist:domainIncludes
		gist:LivingThing ,
		gist:PhysicalIdentifiableItem ,
		tolo:Person
		;
	gist:rangeIncludes
		gist:Event ,
		gist:TemporalRelation ,
		gist:TimeInterval ,
		tolo:HistoricalPeriod
		;
	.

tolo:familyName
	a owl:DatatypeProperty ;
	rdfs:subPropertyOf gist:name ;
	rdfs:domain [
		a owl:Class ;
		owl:unionOf (
			tolo:Person
			tolo:Marriage
		) ;
	] ;
	rdfs:range rdf:langString ;
	skos:definition "The name a person bears based on his/her genealogic or marital relationships."@en ;
	skos:prefLabel "family name"@en ;
	skos:scopeNote "Also applies to marriages; in an ordinary marriage, the marriage, spouses, and children take the husband's family name; in a makpa marriage, the wife's. The marriage name can be inferred from the individuals' family names, or vice versa."@en ;
	.

tolo:firstName
	a owl:DatatypeProperty ;
	rdfs:subClassOf gist:name ;
	rdfs:domain tolo:Person ;
	skos:definition "The first name of a person."@en ;
	skos:prefLabel "first name"@en ;
	skos:scopeNote "Neutral as to whether the first name is the given or family name."@en ;
	.

tolo:fullName
	a owl:DatatypeProperty ;
	rdfs:subClassOf gist:name ;
	skos:definition "The full name of a person."@en ;
	skos:prefLabel "full name"@en ;
	skos:scopeNote "Generally used with persons but conceivably could have other uses."@en ;
	gist:domainIncludes tolo:Person ;
	.

tolo:hasFinalRestingPlace
	a owl:ObjectProperty ;
	rdfs:subPropertyOf gist:hasPhysicalLocation ;
	rdfs:domain tolo:Person ;
	skos:definition "Relates a person to (one of) his/her final resting place(s)."@en ;
	skos:editorialNote "Consider connecting to Death rather than Person."@en ;
	skos:prefLabel "has final resting place"@en ;
	skos:scopeNote "Significant people such as the Dalai Lamas have reliquary stupas in geographic locations like temples or chapels. Sometimes there can be relics in multiple places."@en ;
	.

tolo:hasFraternalNephew
	a owl:ObjectProperty ;
	rdfs:subPropertyOf bdo:hasNephew ;
	owl:propertyChainAxiom (
		bdo:hasBrother
		bdo:hasSon
	) ;
	skos:definition "Relates a person to the son of his/her brother."@en ;
	skos:prefLabel "has fraternal nephew"@en ;
	skos:scopeNote
		"We do not currently distinguish biological, adoptive, half, and step relationships."@en ,
		"While a nephew can be related through either a sibling or sibling-in-law, a fraternal nephew is always related through a brother."@en
		;
	.

tolo:hasFraternalNiece
	a owl:ObjectProperty ;
	rdfs:subPropertyOf bdo:hasNiece ;
	owl:propertyChainAxiom (
		bdo:hasBrother
		bdo:hasSon
	) ;
	skos:definition "Relates a person to the daughter of his/her brother."@en ;
	skos:prefLabel "has fraternal niece"@en ;
	skos:scopeNote
		"We do not currently distinguish biological, adoptive, half, and step relationships."@en ,
		"While a niece can be related through either a sibling or sibling-in-law, a fraternal niece is always related through a brother."@en
		;
	.

tolo:hasHusband
	a owl:ObjectProperty ;
	rdfs:subPropertyOf tolo:hasSpouse ;
	rdfs:domain tolo:Marriage ;
	rdfs:range tolo:Person ;
	skos:definition "Relates a marriage relationship to the husband."@en ;
	skos:prefLabel "has husband"@en ;
	skos:scopeNote "Use bdo:hasHusband to assert a direct relationship from wife to husband."@en ;
	.

tolo:hasMaternalCousin
	a owl:ObjectProperty ;
	rdfs:subPropertyOf bdo:hasCousin ;
	skos:definition "Relates a person to his/her cousin on the mother's side."@en ;
	skos:prefLabel "has maternal cousin"@en ;
	skos:scopeNote "We do not currently distinguish biological, adoptive, half, and step relationships."@en ;
	.

tolo:hasMaternalGrandfather
	a owl:ObjectProperty ;
	rdfs:subPropertyOf
		bdo:hasGrandfather ,
		tolo:hasMaternalGrandparent
		;
	owl:propertyChainAxiom (
		tolo:hasMother
		tolo:hasFather
	) ;
	skos:definition "Relates a person to his/her mother's father."@en ;
	skos:prefLabel "has maternal grandfather"@en ;
	skos:scopeNote "We do not currently distinguish biological, adoptive, half, and step relationships."@en ;
	.

tolo:hasMaternalGrandmother
	a owl:ObjectProperty ;
	rdfs:subPropertyOf
		bdo:hasGrandmother ,
		tolo:hasMaternalGrandparent
		;
	owl:propertyChainAxiom (
		bdo:hasMother
		bdo:hasMother
	) ;
	skos:definition "Relates a person to his/her mother's mother."@en ;
	skos:prefLabel "has maternal grandmother"@en ;
	skos:scopeNote "We do not currently distinguish biological, adoptive, half, and step relationships."@en ;
	.

tolo:hasMaternalGrandparent
	a owl:ObjectProperty ;
	rdfs:subPropertyOf bdo:hasGrandmother ;
	owl:propertyChainAxiom (
		bdo:hasMother
		bdo:hasParent
	) ;
	skos:definition "Relates a person to his/her mother's parent."@en ;
	skos:prefLabel "has maternal grandmother"@en ;
	skos:scopeNote "We do not currently distinguish biological, adoptive, half, and step relationships."@en ;
	.

tolo:hasPaternalCousin
	a owl:ObjectProperty ;
	rdfs:subPropertyOf bdo:hasCousin ;
	skos:definition "Relates a person to his/her cousin on the father's side."@en ;
	skos:prefLabel "has paternal cousin"@en ;
	skos:scopeNote "We do not currently distinguish biological, adoptive, half, and step relationships."@en ;
	.

tolo:hasPaternalGrandfather
	a owl:ObjectProperty ;
	rdfs:subPropertyOf
		bdo:hasGrandfather ,
		tolo:hasPaternalGrandparent
		;
	owl:propertyChainAxiom (
		bdo:hasFather
		bdo:hasFather
	) ;
	skos:definition "Relates a person to his/her father's father."@en ;
	skos:prefLabel "has paternal grandfather"@en ;
	skos:scopeNote "We do not currently distinguish biological, adoptive, half, and step relationships."@en ;
	.

tolo:hasPaternalGrandmother
	a owl:ObjectProperty ;
	rdfs:subPropertyOf
		bdo:hasGrandmother ,
		tolo:hasPaternalGrandparent
		;
	owl:propertyChainAxiom (
		bdo:hasFather
		bdo:hasMother
	) ;
	skos:definition "Relates a person to his/her father's mother."@en ;
	skos:prefLabel "has paternal grandmother"@en ;
	skos:scopeNote "We do not currently distinguish biological, adoptive, half, and step relationships."@en ;
	.

tolo:hasPaternalGrandparent
	a owl:ObjectProperty ;
	rdfs:subPropertyOf bdo:hasGrandparent ;
	owl:propertyChainAxiom (
		bdo:hasFather
		bdo:hasParent
	) ;
	skos:definition "Relates a person to his/her fathers's parent."@en ;
	skos:prefLabel "has maternal grandmother"@en ;
	skos:scopeNote "We do not currently distinguish biological, adoptive, half, and step relationships."@en ;
	.

tolo:hasPreincarnation
	a owl:ObjectProperty ;
	rdfs:domain tolo:Person ;
	rdfs:range tolo:Person ;
	skos:definition "The relationship of a person to a non-living person or mythical figure who is named as a previous emanation."@en ;
	skos:example "Jamgong Kongtrul had the preincarnation Tarnatha."@en ;
	skos:prefLabel "has preincarnation"@en ;
	skos:scopeNote "Not part of the ordered members of incarnation lines and thus represented as a direct relationship between two people. We do not currently have the data to populate this property."@en ;
	.

tolo:hasSororallNephew
	a owl:ObjectProperty ;
	rdfs:subPropertyOf bdo:hasNephew ;
	owl:propertyChainAxiom (
		bdo:hasSister
		bdo:hasSon
	) ;
	skos:definition "Relates a person to his/her sister's son."@en ;
	skos:prefLabel "has sororal nephew"@en ;
	skos:scopeNote
		"We do not currently distinguishbiological, adoptive, half, and step relationships."@en ,
		"While a nephew can be related through either a sibling or sibling-in-law, a sororal nephew is always related through a sister."@en
		;
	.

tolo:hasSororallNiece
	a owl:ObjectProperty ;
	rdfs:subPropertyOf bdo:hasNiece ;
	owl:propertyChainAxiom (
		bdo:hasSister
		bdo:hasDaughter
	) ;
	skos:definition "Relates a person to his/her sister's daughter."@en ;
	skos:prefLabel "has sororal niece"@en ;
	skos:scopeNote
		"We do not currently distinguish biological, adoptive, half, and step relationships."@en ,
		"While a niece can be related through either a sibling or sibling-in-law, a sororal nephew is always related through a sister."@en
		;
	.

tolo:hasSource
	a owl:ObjectProperty ;
	rdfs:domain gist:ContentExpression ;
	rdfs:range gist:ContentExpression ;
	skos:definition "Relates a piece of content to a source of information used to create that content."@en ;
	skos:prefLabel "has source"@en ;
	skos:scopeNote
		"There is currently minimal parsing of source text to generate sources due to the complexity of this task. Pages are in a separate field and the remainder of the source is in a skos:prefLabel."@en ,
		"Written sources are used to create content about persons (i.e., biographies) and places on the Treasury of Lives website and cited with this content."@en
		;
	.

tolo:hasSourceStatement
	a owl:ObjectProperty ;
	rdfs:domain tolo:FormattedContent ;
	rdfs:range gist:FormattedContent ;
	skos:definition "Relates a piece of content to a statement of its sources."@en ;
	skos:prefLabel "has source statement"@en ;
	.

tolo:hasSpouse
	a owl:ObjectProperty ;
	rdfs:subPropertyOf gist:hasParty ;
	rdfs:domain tolo:Marriage ;
	rdfs:range tolo:Person ;
	skos:definition "Relates a marriage relationship to one of the spouses."@en ;
	skos:prefLabel "has spouse"@en ;
	skos:scopeNote "Use bdo:hasHusband or bdo:hasWife to assert a direct relationship from wife to husband or husband to wife, respectively."@en ;
	.

tolo:hasStatement
	a owl:ObjectProperty ;
	rdfs:domain tolo:Biography ;
	rdfs:range tolo:AuthorStatement ;
	skos:definition "Relates a biography to a disclaimer or disclosure about its authorship."@en ;
	skos:example "A biography has a statement indicating that its author is a relative or student of its subject."@en ;
	skos:prefLabel "has statement"@en ;
	.

tolo:hasSummary
	a owl:ObjectProperty ;
	rdfs:domain tolo:FormattedContent ;
	rdfs:range gist:FormattedContent ;
	skos:definition "Relates a piece of content, such as a biography, to a brief statement or restatement of the main points of a larger work."@en ;
	skos:prefLabel "has summary"@en ;
	.

tolo:hasWife
	a owl:ObjectProperty ;
	rdfs:subPropertyOf tolo:hasSpouse ;
	rdfs:domain tolo:Marriage ;
	rdfs:range tolo:Person ;
	skos:definition "Relates a marriage relationship to the wife."@en ;
	skos:prefLabel "has wife"@en ;
	skos:scopeNote "Use bdo:hasWife to assert a direct relationship from husband to wife."@en ;
	.

tolo:inYear
	a owl:DatatypeProperty ;
	rdfs:subPropertyOf gist:atDateTime ;
	skos:definition "The year in which something existed or took place, ambiguous as to start/end and planned/actual/approximate/alternate."@en ;
	skos:example "Gyergom Tsultime Sengge's birth took place in 1144."@en ;
	skos:prefLabel "in year"@en ;
	skos:scopeNote "This is a covering concept for approximate, actual, and alternate years (as for births, deaths, and foundings) but would generally not be materialized directly."@en ;
	.

tolo:isAssignmentOf
	a owl:ObjectProperty ;
	skos:definition "Relates an assignment to the resource it assigns."@en ;
	skos:example "Assignment of a wife status to a marriage."@en ;
	skos:prefLabel "is assignment of"@en ;
	gist:domainIncludes tolo:StatusAssignment ;
	gist:rangeIncludes gist:Category ;
	.

tolo:isAssignmentTo
	a owl:ObjectProperty ;
	skos:definition "Relates an assignment to the thing the resource is assigned to."@en ;
	skos:example "Assignment of a wife status to a marriage."@en ;
	skos:prefLabel "is assignment to"@en ;
	gist:domainIncludes gist:StatusAssignment ;
	.

tolo:isBranchOf
	a owl:ObjectProperty ;
	skos:definition "Relates a monastery to a larger monastery in another location of which it is a subsidiary or affiliate."@en ;
	skos:editorialNote "Consider whether the domain/rangeIncludes should be tightened to rdfs:domain/range."@en ;
	skos:example "The Adzom Gar monastery is a branch of the Katok monastery."@en ;
	skos:prefLabel "is branch of"@en ;
	skos:scopeNote "Differs from the tolo:isDerivedFrom relationship between monasteries, which is used for monasteries in exile."@en ;
	gist:domainIncludes tolo:Monastery ;
	gist:rangeIncludes tolo:Monastery ;
	.

tolo:isCreatedBy
	a owl:ObjectProperty ;
	skos:definition "Relates a man-made object to a person who created it."@en ;
	skos:prefLabel "is created by"@en ;
	gist:domainIncludes
		gist:Content ,
		gist:IntellectualProperty
		;
	.

tolo:isDerivedFrom
	a owl:ObjectProperty ;
	skos:definition "Relates a resource to another it is derived from. This could be in the context of a hierarchy, as for traditions and incarnation lineages, or not, as for monasteries in exile."@en ;
	skos:example "The Barom Kagyu tradition is derived from, or branches off of, the Marpa Kagyu tradition; the Kalu Rinpoche incarnation lineage is derived from the Jamgon Kongtrul lineage; the Ganden and Ganden Tritok Khang monasteries in India are derived from the Ganden monastery in Tibet."@en ;
	skos:prefLabel "is derived from"@en ;
	gist:domainIncludes
		tolo:IncarnationLineage ,
		tolo:Monastery ,
		tolo:Tradition
		;
	gist:rangeIncludes
		tolo:IncarnationLineage ,
		tolo:Monastery ,
		tolo:Tradition
		;
	.

tolo:lastName
	a owl:DatatypeProperty ;
	rdfs:subClassOf gist:name ;
	rdfs:domain tolo:Person ;
	skos:definition "The last name of a person."@en ;
	skos:prefLabel "last name"@en ;
	skos:scopeNote "Neutral as to whether the last name is the given or family name."@en ;
	.

tolo:level
	a owl:DatatypeProperty ;
	rdfs:range xsd:integer ;
	skos:altLabel "priority"@en ;
	skos:definition "A level in a hierarchy."@en ;
	skos:example "The level of a mapping priority; the tier of a subscription."@en ;
	skos:prefLabel "level"@en ;
	.

tolo:localName
	a owl:DatatypeProperty ;
	skos:definition "The local name of an IRI."@en ;
	skos:prefLabel "local name"@en ;
	.

tolo:nameVariant
	a owl:DatatypeProperty ;
	rdfs:subPropertyOf gist:name ;
	skos:altLabel "alternate name"@en ;
	skos:definition "An alternate name for a person."@en ;
	skos:example "Gyergom Nyipa (Wylie gyer sgom gnyis pa) is an alternate name for Gyergom Tsultrim Sengge (Wylie gyer sgom tshul khrims seng+ge)."@en ;
	skos:prefLabel "name variant"@en ;
	skos:scopeNote "The primary/alternate distinction may be source- or system-dependent. Other systems or sources may prefer a name different from Treasury of Lives' primary name."@en ;
	.

tolo:occursBy
	a
		owl:ObjectProperty ,
		owl:TransitiveProperty
		;
	skos:definition "Relates an event or temporal resource to another that temporally contains it."@en ;
	skos:example "The exact founding year or century of Pabongkha Hermitage is unknown, but it occurred by at least the 7th century."@en ;
	skos:prefLabel "occurs by"@en ;
	skos:scopeNote "Less precise than tolo:occursDuring."@en ;
	gist:domainIncludes
		gist:Event ,
		gist:TemporalRelation
		;
	gist:rangeIncludes gist:TimeInterval ;
	.

tolo:occursDuring
	a
		owl:ObjectProperty ,
		owl:TransitiveProperty
		;
	skos:definition "Relates one event, time interval, or temporal resource to another that temporally contains it."@en ;
	skos:example "The birth of Gyergom Tsultrim Sengge occurred during the 12th century; the exact year of the founding of Nyima Tang Monastery is unknown, but it occurred sometime during the 7th century."@en ;
	skos:prefLabel "occurs during"@en ;
	skos:scopeNote "Used when a more precise value, such as year, is unknown or uncertain."@en ;
	gist:domainIncludes
		gist:Event ,
		gist:TemporalRelation ,
		gist:TimeInterval
		;
	gist:rangeIncludes
		gist:Event ,
		gist:TemporalRelation ,
		gist:TimeInterval
		;
	.

tolo:ordinal
	a owl:DatatypeProperty ;
	rdfs:range xsd:integer ;
	skos:definition "An integer used to designate position in a lineage."@en ;
	skos:example "The First Dalai Lama"@en ;
	skos:prefLabel "ordinal"@en ;
	skos:scopeNote
		"Incarnation ordinals reflect the accepted convention of the position of a given individual in the sequence of lives. These occasionally, though rarely, differ from the incarnation sequence due to contested numbering strategies or from the line's originating individual not being counted as the 'first.' An example of the first variant would be the Panchen Lama incarnation line, which has two ordinal sequences based on differing systems of which individual counts as the First Panchen Lama. In this instance, the actual incarnation sequence is the same in both systems, but lines up with the ordinals in one system and differs in the other. An example of the other variant would be the First Shechen Kongtrul, who is the second member of an incarnation sequence that begins with Jamgon Kongtrul."@en ,
		"This value is stored as an integer value and converted to an ordinal string for display purposes. This provides more flexibility than storing as an ordinal string."@en
		;
	.

tolo:pages
	a owl:DatatypeProperty ;
	rdfs:domain gist:ContentExpression ;
	rdfs:range xsd:string ;
	owl:deprecated "true"^^xsd:boolean ;
	skos:definition "Particular page number(s) of a work."@en ;
	skos:editorialNote "Currently deprecated - do not use."@en ;
	skos:prefLabel "page(s)"@en ;
	skos:scopeNote
		"Note that this is a string rather than a number, to account for page ranges."@en ,
		"Used on the Treasury of Lives website in citations of sources."@en
		;
	.

tolo:primaryName
	a owl:DatatypeProperty ;
	rdfs:subPropertyOf gist:name ;
	owl:deprecated "true"^^xsd:boolean ;
	skos:definition "The primary or preferred name of a person or other resource."@en ;
	skos:example "Gyergom Tsultrim Sengge is the primary name of the individual called Gyergom Nyipa by the Library of Congress."@en ;
	skos:prefLabel "primary name"@en ;
	skos:scopeNote
		"The primary/alternate distinction may be source- or system-dependent. Other systems or sources may a different name primary."@en ,
		"The same name may be rendered differently in different transliteration or transcription systems. For example, ToL displays a primary name in both its own and the Extended Wylie systems and possibly others."@en
		;
	.

tolo:publicationDate
	a owl:DatatypeProperty ;
	rdfs:subClassOf gist:atDateTime ;
	skos:definition "The date a biography was published, with day precision."@en ;
	skos:prefLabel "publication date"@en ;
	skos:scopeNote "Differs from the timestamp when the biography metadata was entered into the database (tolo:createDateTime)."@en ;
	.

tolo:references
	a owl:ObjectProperty ;
	skos:definition "Relates content, such as a biography, to a another content instance that was either used as a source or provides additional information about the content."@en ;
	skos:example "The biography of Gyergom Tsultrim Sengge has source 'Secret Visions of the Fifth Dalai Lama by Samten G. Karmay."@en ;
	skos:prefLabel "references"@en ;
	.

tolo:residesIn
	a owl:ObjectProperty ;
	rdfs:range gist:Place ;
	skos:definition "Relates something to the place where it lives or exists."@en ;
	skos:prefLabel "resides in"@en ;
	.

tolo:title
	a owl:DatatypeProperty ;
	rdfs:range rdf:langString ;
	skos:definition "An appellation of dignity, honor, distinction, or preeminence attached to a person or family by virtue of rank, office, precedent, privilege, attainment, or lands."@en ;
	skos:prefLabel "title"@en ;
	.

tolo:updateDate
	a owl:DatatypeProperty ;
	rdfs:subClassOf gist:atDateTime ;
	skos:definition "The date a biography was updated, with day precision."@en ;
	skos:prefLabel "update date"@en ;
	skos:scopeNote "Differs from the timestamp when the biography metadata was last modified in the database (tolo:lastModifiedDateTime)."@en ;
	.

tolo:url
	a owl:DatatypeProperty ;
	rdfs:range xsd:anyURI ;
	skos:definition "A URL."@en ;
	skos:prefLabel "url"@en ;
	.

