# imports: https://w3id.org/semanticarts/ontology/gistCore12.0.1

@prefix bdo: <http://purl.bdrc.io/ontology/core/> .
@prefix gist: <https://w3id.org/semanticarts/ns/ontology/gist/> .
@prefix media-txt: <https://www.iana.org/assignments/media-types/text/> .
@prefix owl: <http://www.w3.org/2002/07/owl#> .
@prefix rdf: <http://www.w3.org/1999/02/22-rdf-syntax-ns#> .
@prefix rdfs: <http://www.w3.org/2000/01/rdf-schema#> .
@prefix skos: <http://www.w3.org/2004/02/skos/core#> .
@prefix told: <https://w3id.org/treasuryoflives/ns/data/tol/> .
@prefix tolo: <https://w3id.org/treasuryoflives/ns/ontology/tol/> .
@prefix tolx: <https://w3id.org/treasuryoflives/ns/taxonomy/tol/> .
@prefix wiki: <https://www.wikidata.org/wiki/> .
@prefix xsd: <http://www.w3.org/2001/XMLSchema#> .

<https://w3id.org/treasuryoflives/ontology/tolCoreX.x.x>
	a owl:Ontology ;
	owl:imports <https://w3id.org/semanticarts/ontology/gistCore12.0.1> ;
	owl:versionIRI <https://w3id.org/treasuryoflives/ontology/tolCoreX.x.x> ;
	skos:definition "The Treasury of Lives Core Ontology enables the description of historical and contemporary figures in the culture and religion of Tibet, Inner Asia, and the Himalaya. It is used by the Treasury of Lives born-digitial biographical collection (https://treasuryoflives.org) to publish and share its data as Linked Open Data, facilitate the consumption of external RDF, and to to enhance the narrative text with structured data."@en ;
	skos:editoralNote
		"Add rdfs:isDefinedBy using onto-toolkit."@en ,
		"Combining all terms into one module for now; may break up into separate modules later."@en
		;
	skos:editorialNote """
		Temporarily removing imports:
			<http://id.loc.gov/ontologies/bibframe-2-1-0> ,
			<http://purl.bdrc.io/ontology/core> to make Protege easier to read."""@en ;
	skos:prefLabel "Treasury of Lives Core Ontology"@en ;
	gist:license "TBD"@en ;
	.

gist:EntityActiveStatus
	a owl:Class ;
	rdfs:subClassOf gist:Category ;
	skos:definition "Indicates whether an entity is active or inactive."@en ;
	skos:prefLabel "Entity Active Status"@en ;
	skos:scopeNote "Can be applied to many types of entities."@en ;
	.

tolo:Author
	a owl:Class ;
	rdfs:subClassOf tolo:Person ;
	skos:definition "A person who has authored or contributed to authoring at least one work."@en ;
	skos:prefLabel "Author"@en ;
	.

tolo:AuthorStatement
	a owl:Class ;
	owl:equivalentClass [
		a owl:Class ;
		owl:intersectionOf (
			gist:Text
			[
				a owl:Restriction ;
				owl:onProperty [
					owl:inverseOf tolo:hasStatement ;
				] ;
				owl:someValuesFrom tolo:Biography ;
			]
		) ;
	] ;
	skos:definition "A disclaimer or disclosure about the author of a biography."@en ;
	skos:example "A statement indicating that the author of the biography is a relative or student of its subject."@en ;
	skos:prefLabel "Author Statement"@en ;
	.

tolo:Authorship
	a owl:Class ;
	owl:equivalentClass [
		a owl:Class ;
		owl:intersectionOf (
			gist:TemporalRelation
			[
				a owl:Restriction ;
				owl:onProperty gist:hasParticipant ;
				owl:someValuesFrom tolo:Author ;
			]
			[
				a owl:Restriction ;
				owl:onProperty gist:hasParticipant ;
				owl:someValuesFrom tolo:Biography ;
			]
		) ;
	] ;
	skos:definition "Relates a bio to a person who has authored it."@en ;
	skos:editorialNote
		"Though there is a display order of multiple authors of a single biography, we do not currently distinguish primary from secondary author in the model, because there may be more than two authors and we still need to specify the display order."@en ,
		"Using a simple model of authorship until there is a use case for a more complex model with contributions and roles as in BIBFRAME."@en
		;
	skos:prefLabel "Authorship"@en ;
	.

tolo:Biography
	a owl:Class ;
	rdfs:subClassOf
		gist:FormattedContent ,
		[
			a owl:Restriction ;
			owl:onProperty gist:isExpressedIn ;
			owl:hasValue media-txt:html ;
		] ,
		[
			a owl:Restriction ;
			owl:onProperty gist:isAbout ;
			owl:someValuesFrom tolo:Person ;
		]
		;
	skos:definition "A written account of another person's life, formatted in HTML for publication on the Treasury of Lives website."@en ;
	skos:editorialNote "Using subclass axioms rather than equivalence because the author bios should not be inferred into the class. TODO: Generalize the model a bit for external consumption: define a generic Biography class, subclass of bf:Work (or gist:Content?), then HtmlBio as formatted html content, etc."@en ;
	skos:example "The Treasury of Lives biography of Rongzom Chokyi Zangpo is published on the Treasury of Lives website at https://treasuryoflives.org/biographies/view/Rongzom-Chokyi-Zangpo/6194."@en ;
	skos:prefLabel "Biography"@en ;
	skos:scopeNote "A biography involves more than just basic facts like education, work, relationships, and death; it portrays a person's experience of these life events."@en ;
	.

tolo:Birth
	a owl:Class ;
	rdfs:subClassOf
		gist:HistoricalEvent ,
		gist:PhysicalEvent ,
		[
			a owl:Restriction ;
			owl:onProperty tolo:isEventOf ;
			owl:allValuesFrom tolo:Person ;
		] ,
		[
			a owl:Restriction ;
			owl:onProperty gist:occursIn ;
			owl:cardinality "1"^^xsd:nonNegativeInteger ;
		] ,
		[
			a owl:Restriction ;
			owl:onProperty tolo:isEventOf ;
			owl:cardinality "1"^^xsd:nonNegativeInteger ;
		] ,
		[
			a owl:Restriction ;
			owl:onProperty tolo:inYear ;
			owl:minCardinality "1"^^xsd:nonNegativeInteger ;
		]
		;
	skos:definition "TBD"@en ;
	skos:editorialNote "Can deities have birth and death? We may need to loosen the restriction."@en ;
	skos:prefLabel "Birth"@en ;
	.

tolo:BuildingType
	a owl:Class ;
	rdfs:subClassOf
		gist:Category ,
		[
			a owl:Restriction ;
			owl:onProperty [
				owl:inverseOf gist:isCategorizedBy ;
			] ;
			owl:allValuesFrom gist:Building ;
		]
		;
	skos:definition "Indicates the specific type of a building."@en ;
	skos:example "Manor, government building, palace, temple."@en ;
	skos:prefLabel "Building Type"@en ;
	.

tolo:Death
	a owl:Class ;
	rdfs:subClassOf
		gist:HistoricalEvent ,
		gist:PhysicalEvent ,
		[
			a owl:Restriction ;
			owl:onProperty tolo:isEventOf ;
			owl:allValuesFrom tolo:Person ;
		] ,
		[
			a owl:Restriction ;
			owl:onProperty gist:occursIn ;
			owl:cardinality "1"^^xsd:nonNegativeInteger ;
		] ,
		[
			a owl:Restriction ;
			owl:onProperty tolo:isEventOf ;
			owl:cardinality "1"^^xsd:nonNegativeInteger ;
		] ,
		[
			a owl:Restriction ;
			owl:onProperty tolo:inYear ;
			owl:minCardinality "1"^^xsd:nonNegativeInteger ;
		]
		;
	skos:definition "TBD"@en ;
	skos:editorialNote "Can deities have birth and death? We may need to loosen the restriction."@en ;
	skos:prefLabel "Death"@en ;
	.

tolo:HistoricalPeriod
	a owl:Class ;
	rdfs:subClassOf gist:TimeInterval ;
	skos:definition "A named time interval with historical significance."@en ;
	skos:example "The 10th century, the eary/mid/late 19th century."@en ;
	skos:prefLabel "Historical Period"@en ;
	skos:scopeNote "Whereas a time interval is any period of time, such as 2-4pm this afternoon or 1848-1947, a historical period is named and cited in relation to historical events or culture. Historical periods include full and partial centuries, which are ordinally numbered."@en ;
	.

tolo:Incarnation
	a owl:Class ;
	rdfs:subClassOf
		[
			a owl:Restriction ;
			owl:onProperty [
				owl:inverseOf gist:hasMember ;
			] ;
			owl:allValuesFrom tolo:IncarnationLineage ;
		] ,
		[
			a owl:Restriction ;
			owl:onProperty gist:providesOrderFor ;
			owl:allValuesFrom tolo:Person ;
		]
		;
	owl:equivalentClass [
		a owl:Class ;
		owl:intersectionOf (
			gist:OrderedMember
			[
				a owl:Restriction ;
				owl:onProperty [
					owl:inverseOf gist:hasMember ;
				] ;
				owl:someValuesFrom tolo:IncarnationLineage ;
			]
			[
				a owl:Restriction ;
				owl:onProperty gist:providesOrderFor ;
				owl:someValuesFrom tolo:Person ;
			]
			[
				a owl:Restriction ;
				owl:onProperty gist:sequence ;
				owl:someValuesFrom xsd:integer ;
			]
		) ;
	] ;
	skos:definition "The relationship connecting a person to an incarnation lineage and expressing the sequence and ordinal of the person in the lineage."@en ;
	skos:editorialNote "Connects person to lineage."@en ;
	skos:example "The Third Dalai Lama."@en ;
	skos:prefLabel
		"Incarnation"@en ,
		"sprul sku"@bo-x-ewts
		;
	skos:scopeNote "The sequence and ordinal may differ in some cases, and in some cases there may be no ordinal."@en ;
	.

tolo:IncarnationLineage
	a owl:Class ;
	rdfs:subClassOf [
		a owl:Restriction ;
		owl:onProperty gist:hasMember ;
		owl:allValuesFrom tolo:Incarnation ;
	] ;
	owl:equivalentClass [
		a owl:Class ;
		owl:intersectionOf (
			gist:OrderedCollection
			[
				a owl:Restriction ;
				owl:onProperty gist:hasMember ;
				owl:someValuesFrom tolo:Incarnation ;
			]
		) ;
	] ;
	skos:definition "A consecutive line of people regarded as incarnations of a non-living person or mythical figure."@en ;
	skos:example "The Dalai Lamas, the Karmapas."@en ;
	skos:prefLabel
		"Incarnation Lineage"@en ,
		"skye brgyud"@bo-x-ewts
		;
	skos:scopeNote "An incarnation lineage is enumerated chronologically and can branch into multiple lines. Usually associated with a seat, such as a monastery, and a tradition."@en ;
	.

tolo:Institution
	a owl:Class ;
	owl:equivalentClass [
		a owl:Class ;
		owl:intersectionOf (
			gist:Organization
			[
				a owl:Restriction ;
				owl:onProperty gist:isCategorizedBy ;
				owl:someValuesFrom tolo:InstitutionType ;
			]
		) ;
	] ;
	skos:definition "A human-made organization typically connected to a single or multiple physical buildings with a shared mission, identity, norms and rules that often contains subsidiary members or suborganizations."@en ;
	skos:example "Choding Monastery, Nyarongsha School, Mentsikhang Hospital."@en ;
	skos:prefLabel "Institution"@en ;
	skos:scopeNote "An institution is not a place per se - e.g., a monastery could move to a different site - but is associated with a place."@en ;
	.

tolo:InstitutionType
	a owl:Class ;
	rdfs:subClassOf
		gist:Category ,
		[
			a owl:Restriction ;
			owl:onProperty [
				owl:inverseOf gist:isCategorizedBy ;
			] ;
			owl:allValuesFrom tolo:Institution ;
		]
		;
	skos:definition "Indicates the specific type of an institution."@en ;
	skos:example "Monastery, hospital, school, etc."@en ;
	skos:prefLabel "Institution Type"@en ;
	skos:scopeNote "Using the class-type pattern, some institution types will also be represented as subclasses because they have specialized restrictions."@en ;
	.

tolo:KinshipGroup
	a owl:Class ;
	rdfs:subClassOf
		gist:Collection ,
		[
			a owl:Restriction ;
			owl:onProperty gist:hasMember ;
			owl:allValuesFrom tolo:Person ;
		]
		;
	skos:definition "A social unit consisting of people with a common ancestor."@en ;
	skos:example "The Adro clan; the Jangling family."@en ;
	skos:prefLabel "Kinship Group"@en ;
	skos:scopeNote "Includes Tibetan concepts that may individually mean something more specific, such as: rig (rigs) for clan, race, family; gyu (rgyud) for lineage, descent; dungrab (gdung rabs) for descendants, lineage, generation; dung (gdung) for progeny, descendants, lineage, descent line; ru (rus) for bone, bloodline, lineage, family, clan; khang (khang) for household and tsang (tshang) for family and household."@en ;
	.

tolo:KinshipGroupType
	a owl:Class ;
	owl:equivalentClass [
		owl:intersectionOf (
			gist:Category
			[
				a owl:Restriction ;
				owl:onProperty [
					owl:inverseOf gist:isCategorizedBy ;
				] ;
				owl:allValuesFrom tolo:KinshipGroup ;
			]
		) ;
	] ;
	skos:definition "A type of kinship group."@en ;
	skos:example "Lhasa Aristocracy."@en ;
	skos:prefLabel "Kinship Group Type"@en ;
	skos:scopeNote "Currently only one type is defined."@en ;
	.

tolo:LandmarkType
	a owl:Class ;
	rdfs:subClassOf
		gist:Category ,
		[
			a owl:Restriction ;
			owl:onProperty [
				owl:inverseOf gist:isCategorizedBy ;
			] ;
			owl:allValuesFrom gist:Landmark ;
		]
		;
	skos:definition "Indicates the specific type of a landmark."@en ;
	skos:example "Stupa, hermitage, lake, mountain, hidden land, cave"@en ;
	skos:prefLabel "Landmark Type"@en ;
	.

tolo:Marriage
	a owl:Class ;
	owl:equivalentClass [
		owl:intersectionOf (
			gist:Agreement
			gist:TemporalRelation
			[
				a owl:Restriction ;
				owl:onProperty gist:hasParty ;
				owl:allValuesFrom tolo:Person ;
			]
			[
				a owl:Restriction ;
				owl:onProperty gist:isCategorizedBy ;
				owl:onClass tolo:MarriageRank ;
				owl:cardinality "1"^^xsd:nonNegativeInteger ;
			]
			[
				a owl:Restriction ;
				owl:onProperty gist:hasParty ;
				owl:onClass tolo:Person ;
				owl:qualifiedCardinality "2"^^xsd:nonNegativeInteger ;
			]
			[
				a owl:Restriction ;
				owl:onProperty tolo:familyName ;
				owl:cardinality "1"^^xsd:nonNegativeInteger ;
			]
			[
				a owl:Restriction ;
				owl:onProperty tolo:familyName ;
				owl:cardinality "1"^^xsd:nonNegativeInteger ;
			]
		) ;
	] ;
	skos:definition "A culturally and often legally recognized union between two people, called spouses, that establishes rights and obligations between them."@en ;
	skos:editorialNote
		"Cardinality restriction on gist:hasParty of 2 generates Protege error, so using qualified cardinality restriction instead."@en ,
		"Predicates should be directed from the relationship to the other objects, to support named graph drops to delete the relationship."@en
		;
	skos:prefLabel "Marriage"@en ;
	.

tolo:MarriageRank
	a owl:Class ;
	rdfs:subClassOf
		gist:Category ,
		[
			a owl:Restriction ;
			owl:onProperty [
				owl:inverseOf gist:isCategorizedBy ;
			] ;
			owl:allValuesFrom tolo:Marriage ;
		]
		;
	skos:definition "A category differentiating senior (first) from subsequent (junior) marriages in polygamous relationships."@en ;
	skos:prefLabel "Marriage Rank"@en ;
	skos:scopeNote "The associated spouse is termed a junior or senior wife/husband. There is only one senior wife or husband; all others are uniformly designated junior."@en ;
	.

tolo:MarriageTerminationCause
	a owl:Class ;
	rdfs:subClassOf
		gist:Category ,
		[
			a owl:Restriction ;
			owl:onProperty [
				owl:inverseOf gist:isCategorizedBy ;
			] ;
			owl:allValuesFrom tolo:Marriage ;
		]
		;
	skos:definition "The reason for the termination of a marriage."@en ;
	skos:example "Death, divorce, dissolution."@en ;
	skos:prefLabel "Marriage Termination Cause"@en ;
	.

tolo:Monastery
	a owl:Class ;
	owl:equivalentClass [
		a owl:Class ;
		owl:intersectionOf (
			tolo:Institution
			[
				a owl:Restriction ;
				owl:onProperty gist:isCategorizedBy ;
				owl:hasValue tolx:_InstitutionType_monastery ;
			]
		) ;
	] ;
	skos:definition "TBD"@en ;
	skos:editorialNote "Has a founder, has abotts, ..."@en ;
	skos:prefLabel "Monastery"@en ;
	.

tolo:Person
	a owl:Class ;
	rdfs:subClassOf
		bdo:Person ,
		gist:Person ,
		wiki:Person
		;
	skos:definition "An individual being who was born, lived, and died in the human realm."@en ;
	skos:prefLabel
		"Person"@en ,
		"mi"@bo-x-ewts
		;
	skos:scopeNote "May include quasi-historical figures."@en ;
	.

tolo:SourceStatement
	a owl:Class ;
	rdfs:subClassOf
		gist:Content ,
		[
			a owl:Restriction ;
			owl:onProperty gist:isAbout ;
			owl:someValuesFrom gist:Content ;
		]
		;
	skos:definition "A statement of the sources used to compile a piece of content."@en ;
	skos:editorialNote "Could alternatively model with an object property hasSourceStatement."@en ;
	skos:prefLabel "Source Statement"@en ;
	.

tolo:Summary
	a owl:Class ;
	rdfs:subClassOf
		gist:Content ,
		[
			a owl:Restriction ;
			owl:onProperty gist:isAbout ;
			owl:someValuesFrom gist:Content ;
		]
		;
	skos:definition "A brief statement or restatement of the main points of a larger work."@en ;
	skos:editorialNote "Could alternatively model with an object property hasSummary."@en ;
	skos:prefLabel "Summary"@en ;
	.

tolo:TeacherStudentRelationship
	a owl:Class ;
	owl:equivalentClass [
		a owl:Class ;
		owl:intersectionOf (
			gist:TemporalRelation
			gist:Agreement
			[
				a owl:Restriction ;
				owl:onProperty gist:hasGiver ;
				owl:someValuesFrom tolo:Person ;
			]
			[
				a owl:Restriction ;
				owl:onProperty gist:hasRecipient ;
				owl:someValuesFrom tolo:Person ;
			]
			[
				a owl:Restriction ;
				owl:onProperty gist:conformsTo ;
				owl:someValuesFrom tolo:Tradition ;
			]
		) ;
	] ;
	skos:definition "A time-delimited relationship between a teacher and a student."@en ;
	skos:prefLabel "Teacher-Student Relationship"@en ;
	.

tolo:Tradition
	a owl:Class ;
	rdfs:subClassOf gist:Intention ;
	skos:definition "An instance of Tibetan religion that identifies as a cohesive group with distinct modes of ritual and learning, as well as associated institutions such as monasteries."@en ;
	skos:example "The major schools and subschools of Tibetan Buddhism as well as Bon."@en ;
	skos:prefLabel
		"Tradition"@en ,
		"chos lugs"@bo-x-ewts
		;
	.

tolo:actualYear
	a owl:DatatypeProperty ;
	rdfs:subPropertyOf tolo:inYear ;
	skos:definition "The year in which something existed or took place."@en ;
	skos:example "Gyergom Tsultime Sengge was born in 1144 and died in 1204."@en ;
	skos:prefLabel "actual year"@en ;
	.

tolo:alternateYear
	a owl:DatatypeProperty ;
	rdfs:subPropertyOf tolo:inYear ;
	skos:definition "The year in which something is proposed to have existed or taken place."@en ;
	skos:example "According to one source, Botrul Dongak Tenpai Nyima was born in 1900, while according to another source his birth year was XXX and he died in 1902. No indication of greater or less likelihood of the two possibilities is implied."@en ;
	skos:prefLabel "alternate year"@en ;
	skos:scopeNote "Differs from tolo:approximateYear, which specifies a single year but is intended to be inexact. In this case, various scholars have proposed different years. If there is an alternate year, there is no actual year; rather, both proposed dates are asserted as alternates."@en ;
	.

tolo:approximateYear
	a owl:DatatypeProperty ;
	rdfs:subPropertyOf tolo:inYear ;
	skos:definition "The approximate year in which something existed or took place."@en ;
	skos:example "The birth event of Lhagyari Namgyel Gyatso took place in approximately 1927."@en ;
	skos:prefLabel "approximate year"@en ;
	skos:scopeNote "Differs from tolo:alternateYear, which is used when there is more than one proposed year. In this case, only one year is asserted, but it is intended to be inexact, thus encompassing some number of years before and/or after."@en ;
	.

tolo:birthFamilyName
	a owl:DatatypeProperty ;
	rdfs:subPropertyOf tolo:familyName ;
	rdfs:domain tolo:Person ;
	rdfs:range rdf:langString ;
	skos:definition "The family name a person is assigned at birth."@en ;
	skos:prefLabel "birth family name"@en ;
	skos:scopeNote "A family name other than the birth name can be acquired through marriage."@en ;
	.

tolo:dissolutionYear
	a owl:DatatypeProperty ;
	rdfs:subPropertyOf gist:actualEndYear ;
	skos:definition "The year an agreement such as marriage was ended. In the case of marriage, this refers to divorce rather than the end of a marriage by death of one of the spouses."@en ;
	skos:editorialNote
		"Use if we need to distinguish divorce from death as the end of a marriage."@en ,
		"We may want to do this like birth and death - have a Dissolution object with a year. If there are many things with actual/approximate/alternate values, (dissolution, founding, etc.) we should establish this as a general pattern."@en
		;
	skos:prefLabel "dissolution year"@en ;
	.

tolo:existsDuring
	a owl:ObjectProperty ;
	skos:definition "Relates an entity to an event, time period, or other temporal object during which it does or did exist."@en ;
	skos:example "Trimalo lived during the 7th century; Dorje Sherab lived during the 12th and 13th centuries."@en ;
	skos:prefLabel "exists during"@en ;
	skos:scopeNote "The subject of tolo:existsDuring is a non-temporal resource. The property contrasts with tolo:occursDuring, which relates a temporal resource to a containing temporal resource."@en ;
	gist:domainIncludes
		gist:LivingThing ,
		gist:PhysicalIdentifiableItem ,
		tolo:Person
		;
	gist:rangeIncludes
		gist:Event ,
		gist:TemporalRelation ,
		gist:TimeInterval ,
		tolo:HistoricalPeriod
		;
	.

tolo:familyName
	a owl:DatatypeProperty ;
	rdfs:subPropertyOf gist:name ;
	rdfs:domain [
		a owl:Class ;
		owl:unionOf (
			tolo:Person
			tolo:Marriage
		) ;
	] ;
	rdfs:range rdf:langString ;
	skos:definition "The name a person bears based on his/her genealogic or marital relationships."@en ;
	skos:prefLabel "family name"@en ;
	skos:scopeNote "Also applies to marriages; in an ordinary marriage, the marriage, spouses, and children take the husband's family name; in a makpa marriage, the wife's. The marriage name can be inferred from the individuals' family names, or vice versa."@en ;
	.

tolo:firstName
	a owl:DatatypeProperty ;
	rdfs:subClassOf gist:name ;
	rdfs:domain tolo:Person ;
	skos:definition "The first name of a person."@en ;
	skos:prefLabel "first name"@en ;
	skos:scopeNote "Neutral as to whether the first name is the given or family name."@en ;
	.

tolo:foundingYear
	a owl:DatatypeProperty ;
	rdfs:subPropertyOf gist:actualStartYear ;
	skos:definition "TODO"@en ;
	skos:editorialNote "We may want to follow the pattern of Birth and Death here, instead of just using a property. Depends on what other information is available. We could have Founding with an agent and a date."@en ;
	skos:example "The Tshal-pa tradition was founded in 1123."@en ;
	skos:prefLabel "founding year"@en ;
	.

tolo:fullName
	a owl:DatatypeProperty ;
	rdfs:subClassOf gist:name ;
	skos:definition "The full name of a person."@en ;
	skos:prefLabel "full name"@en ;
	skos:scopeNote "Generally used with persons but conceivably could have other uses."@en ;
	gist:domainIncludes tolo:Person ;
	.

tolo:hasEvent
	a owl:ObjectProperty ;
	rdfs:range gist:Event ;
	skos:definition "Relates something to an event pertaining to it."@en ;
	skos:example "A person's birth or death; the founding of an institution; the dissolution of a marriage."@en ;
	skos:prefLabel "has event"@en ;
	.

tolo:hasFinalRestingPlace
	a owl:ObjectProperty ;
	rdfs:subPropertyOf gist:hasPhysicalLocation ;
	rdfs:domain tolo:Person ;
	skos:definition "Relates a person to (one of) his/her final resting place(s)."@en ;
	skos:editorialNote "Consider connecting to Death rather than Person."@en ;
	skos:prefLabel "has final resting place"@en ;
	skos:scopeNote "Significant people such as the Dalai Lamas have reliquary stupas in geographic locations like temples or chapels. Sometimes there can be relics in multiple places."@en ;
	.

tolo:hasFounder
	a owl:ObjectProperty ;
	rdfs:range tolo:Person ;
	skos:definition "TBD."@en ;
	skos:prefLabel "has founder"@en ;
	.

tolo:hasFraternalNephew
	a owl:ObjectProperty ;
	rdfs:subPropertyOf bdo:hasNephew ;
	owl:propertyChainAxiom (
		bdo:hasBrother
		bdo:hasSon
	) ;
	skos:definition "Relates a person to the son of his/her brother."@en ;
	skos:prefLabel "has fraternal nephew"@en ;
	skos:scopeNote
		"We do not currently distinguish biological, adoptive, half, and step relationships."@en ,
		"While a nephew can be related through either a sibling or sibling-in-law, a fraternal nephew is always related through a brother."@en
		;
	.

tolo:hasFraternalNiece
	a owl:ObjectProperty ;
	rdfs:subPropertyOf bdo:hasNiece ;
	owl:propertyChainAxiom (
		bdo:hasBrother
		bdo:hasSon
	) ;
	skos:definition "Relates a person to the daughter of his/her brother."@en ;
	skos:prefLabel "has fraternal niece"@en ;
	skos:scopeNote
		"We do not currently distinguish biological, adoptive, half, and step relationships."@en ,
		"While a niece can be related through either a sibling or sibling-in-law, a fraternal niece is always related through a brother."@en
		;
	.

tolo:hasJuniorHusband
	a owl:ObjectProperty ;
	rdfs:subPropertyOf bdo:hasHusband ;
	rdfs:domain tolo:Person ;
	rdfs:range tolo:Person ;
	skos:definition "The relationship of a wife to her husband in a junior marriage, which is any but the first of multiple simultaneous marriages."@en ;
	skos:note "In polyandrous relationships, the senior husband is considered to be the father of all the children, since the precise genealogy is unknown. The junior husbands are considered uncles."@en ;
	skos:prefLabel "has junior husband"@en ;
	skos:scopeNote "This property will generally not be asserted, but rather inferred from the relationships of the spouses to a Marriage object and the MarriageRank of that object."@en ;
	.

tolo:hasJuniorWife
	a owl:ObjectProperty ;
	rdfs:subPropertyOf bdo:hasWife ;
	rdfs:domain tolo:Person ;
	rdfs:range tolo:Person ;
	skos:definition "The relationship of a husband to his wife in a junior marriage, which is any but the first of multiple simultaneous marriages."@en ;
	skos:prefLabel "has junior wife"@en ;
	skos:scopeNote "This property will generally not be asserted, but rather inferred from the relationships of the spouses to a Marriage object and the MarriageRank of that object."@en ;
	.

tolo:hasMaternalCousin
	a owl:ObjectProperty ;
	rdfs:subPropertyOf bdo:hasCousin ;
	skos:definition "Relates a person to his/her cousin on the mother's side."@en ;
	skos:prefLabel "has maternal cousin"@en ;
	skos:scopeNote "We do not currently distinguish biological, adoptive, half, and step relationships."@en ;
	.

tolo:hasMaternalGrandfather
	a owl:ObjectProperty ;
	rdfs:subPropertyOf
		bdo:hasGrandfather ,
		tolo:hasMaternalGrandparent
		;
	owl:propertyChainAxiom (
		tolo:hasMother
		tolo:hasFather
	) ;
	skos:definition "Relates a person to his/her mother's father."@en ;
	skos:prefLabel "has maternal grandfather"@en ;
	skos:scopeNote "We do not currently distinguish biological, adoptive, half, and step relationships."@en ;
	.

tolo:hasMaternalGrandmother
	a owl:ObjectProperty ;
	rdfs:subPropertyOf
		bdo:hasGrandmother ,
		tolo:hasMaternalGrandparent
		;
	owl:propertyChainAxiom (
		bdo:hasMother
		bdo:hasMother
	) ;
	skos:definition "Relates a person to his/her mother's mother."@en ;
	skos:prefLabel "has maternal grandmother"@en ;
	skos:scopeNote "We do not currently distinguish biological, adoptive, half, and step relationships."@en ;
	.

tolo:hasMaternalGrandparent
	a owl:ObjectProperty ;
	rdfs:subPropertyOf bdo:hasGrandmother ;
	owl:propertyChainAxiom (
		bdo:hasMother
		bdo:hasParent
	) ;
	skos:definition "Relates a person to his/her mother's parent."@en ;
	skos:prefLabel "has maternal grandmother"@en ;
	skos:scopeNote "We do not currently distinguish biological, adoptive, half, and step relationships."@en ;
	.

tolo:hasPaternalCousin
	a owl:ObjectProperty ;
	rdfs:subPropertyOf bdo:hasCousin ;
	skos:definition "Relates a person to his/her cousin on the father's side."@en ;
	skos:prefLabel "has paternal cousin"@en ;
	skos:scopeNote "We do not currently distinguish biological, adoptive, half, and step relationships."@en ;
	.

tolo:hasPaternalGrandfather
	a owl:ObjectProperty ;
	rdfs:subPropertyOf
		bdo:hasGrandfather ,
		tolo:hasPaternalGrandparent
		;
	owl:propertyChainAxiom (
		bdo:hasFather
		bdo:hasFather
	) ;
	skos:definition "Relates a person to his/her father's father."@en ;
	skos:prefLabel "has paternal grandfather"@en ;
	skos:scopeNote "We do not currently distinguish biological, adoptive, half, and step relationships."@en ;
	.

tolo:hasPaternalGrandmother
	a owl:ObjectProperty ;
	rdfs:subPropertyOf
		bdo:hasGrandmother ,
		tolo:hasPaternalGrandparent
		;
	owl:propertyChainAxiom (
		bdo:hasFather
		bdo:hasMother
	) ;
	skos:definition "Relates a person to his/her father's mother."@en ;
	skos:prefLabel "has paternal grandmother"@en ;
	skos:scopeNote "We do not currently distinguish biological, adoptive, half, and step relationships."@en ;
	.

tolo:hasPaternalGrandparent
	a owl:ObjectProperty ;
	rdfs:subPropertyOf bdo:hasGrandparent ;
	owl:propertyChainAxiom (
		bdo:hasFather
		bdo:hasParent
	) ;
	skos:definition "Relates a person to his/her fathers's parent."@en ;
	skos:prefLabel "has maternal grandmother"@en ;
	skos:scopeNote "We do not currently distinguish biological, adoptive, half, and step relationships."@en ;
	.

tolo:hasPreincarnation
	a owl:ObjectProperty ;
	skos:definition "The relationship of a person to a non-living person or mythical figure who is named as a previous emanation."@en ;
	skos:example "Jamgong Kongtrul had the preincarnation Tarnatha."@en ;
	skos:prefLabel "has preincarnation"@en ;
	skos:scopeNote "Not part of the ordered members of incarnation lines and thus represented as a direct relationship between two people."@en ;
	.

tolo:hasSeniorHusband
	a owl:ObjectProperty ;
	rdfs:subPropertyOf bdo:hasHusband ;
	rdfs:domain tolo:Person ;
	rdfs:range tolo:Person ;
	skos:definition "The relationship of a wife to her husband in a senior marriage, which is the first marriage of multiple simultaneous marriages."@en ;
	skos:note "In polyandrous relationships, the senior husband is considered to be the father of all the children, since the precise genealogy is unknown. The junior husbands are considered uncles."@en ;
	skos:prefLabel "has senior husband"@en ;
	skos:scopeNote "This property will generally not be asserted, but rather inferred from the relationships of the spouses to a Marriage object and the MarriageRank of that object."@en ;
	.

tolo:hasSeniorWife
	a owl:ObjectProperty ;
	rdfs:subPropertyOf bdo:hasWife ;
	rdfs:domain tolo:Person ;
	rdfs:range tolo:Person ;
	skos:definition "The relationship of a husband to his wife in a senior marriage, which is the first of multiple simultaneous marriages."@en ;
	skos:prefLabel "has senior wife"@en ;
	skos:scopeNote "This property will generally not be asserted, but rather inferred from the relationships of the spouses to a Marriage object and the MarriageRank of that object."@en ;
	.

tolo:hasSororallNephew
	a owl:ObjectProperty ;
	rdfs:subPropertyOf bdo:hasNephew ;
	owl:propertyChainAxiom (
		bdo:hasSister
		bdo:hasSon
	) ;
	skos:definition "Relates a person to his/her sister's son."@en ;
	skos:prefLabel "has sororal nephew"@en ;
	skos:scopeNote
		"We do not currently distinguishbiological, adoptive, half, and step relationships."@en ,
		"While a nephew can be related through either a sibling or sibling-in-law, a sororal nephew is always related through a sister."@en
		;
	.

tolo:hasSororallNiece
	a owl:ObjectProperty ;
	rdfs:subPropertyOf bdo:hasNiece ;
	owl:propertyChainAxiom (
		bdo:hasSister
		bdo:hasDaughter
	) ;
	skos:definition "Relates a person to his/her sister's daughter."@en ;
	skos:prefLabel "has sororal niece"@en ;
	skos:scopeNote
		"We do not currently distinguish biological, adoptive, half, and step relationships."@en ,
		"While a niece can be related through either a sibling or sibling-in-law, a sororal nephew is always related through a sister."@en
		;
	.

tolo:hasStatement
	a owl:ObjectProperty ;
	rdfs:domain tolo:Biography ;
	rdfs:range tolo:AuthorStatement ;
	skos:definition "Relates a biography to a disclaimer or disclosure about its authorship."@en ;
	skos:example "A biography has a statement indicating that its author is a relative or student of its subject."@en ;
	skos:prefLabel "has statement"@en ;
	.

tolo:inYear
	a owl:DatatypeProperty ;
	rdfs:subPropertyOf gist:atDateTime ;
	skos:definition "The year in which something existed or took place, ambiguous as to start/end and planned/actual/approximate/alternate."@en ;
	skos:example "Gyergom Tsultime Sengge's birth took place in 1144."@en ;
	skos:prefLabel "in year"@en ;
	.

tolo:isAffiliatedWith
	a owl:ObjectProperty ;
	owl:deprecated "true"^^xsd:boolean ;
	skos:definition "Relates a person, organization, or lineage to a group, institution, religion, or larger organization it is connected to."@en ;
	skos:editorialNote "For now using gist:isConnectedTo instead; seems adequate and it's hard to pin down a narrower meaning of affiliation. Note that this property would not be a subproperty of gist:isConnectedTo because it is not symmetric."@en ;
	skos:example "A teacher is affiliated with a tradition; an incarnation lineage is associated with a monastery and tradition."@en ;
	skos:prefLabel "is affiliated with"@en ;
	.

tolo:isChildIn
	a owl:ObjectProperty ;
	rdfs:domain tolo:Person ;
	rdfs:range tolo:Marriage ;
	skos:definition "Relates a child to a materialized marriage relationship."@en ;
	skos:editorialNote "Do we need this, or is it sufficient to relate the child to its parents?"@en ;
	skos:prefLabel "is child in"@en ;
	.

tolo:isDerivedFrom
	a owl:ObjectProperty ;
	skos:definition "Relates a resource in a hierarchy to its parent entity in that hierarchy."@en ;
	skos:editorialNote "Consider better names - e.g., hasParentEntity, branchesFrom."@en ;
	skos:example "The Barom Kagyu tradition is derived from, or branches off of, the Marpa Kagyu tradition."@en ;
	skos:prefLabel "is derived from"@en ;
	gist:domainIncludes tolo:Tradition ;
	gist:rangeIncludes tolo:Tradition ;
	.

tolo:isEventOf
	a owl:ObjectProperty ;
	owl:inverseOf tolo:hasEvent ;
	skos:definition "Relates an event to the thing it pertains to."@en ;
	skos:example "A person's birth or death; the founding of an institution; the dissolution of a marriage."@en ;
	skos:prefLabel "is event of"@en ;
	.

tolo:isHusbandIn
	a owl:ObjectProperty ;
	rdfs:domain tolo:Person ;
	rdfs:range tolo:Marriage ;
	skos:definition "Relates a husband to a materialized marriage relationship."@en ;
	skos:prefLabel "is husband in"@en ;
	skos:scopeNote "This could be asserted, or inferred from isSpouseIn and the gender of the person."@en ;
	.

tolo:isSpouseIn
	a owl:ObjectProperty ;
	rdfs:domain tolo:Person ;
	rdfs:range tolo:Marriage ;
	skos:definition "Relates a person to a materialized marriage relationship."@en ;
	skos:prefLabel "is spouse in"@en ;
	skos:scopeNote "It is generally preferable to use the more specific isWifeIn or isHusbandIn, though these could also be inferred from isSpouseIn and the gender of the person. gist:hasParticipant is not specific enough, because children are also related to the marriage."@en ;
	.

tolo:isWifeIn
	a owl:ObjectProperty ;
	rdfs:domain tolo:Person ;
	rdfs:range tolo:Marriage ;
	skos:definition "Relates a wife to a materialized marriage relationship."@en ;
	skos:prefLabel "is wife in"@en ;
	skos:scopeNote "This could be asserted, or inferred from isSpouseIn and the gender of the person."@en ;
	.

tolo:lastName
	a owl:DatatypeProperty ;
	rdfs:subClassOf gist:name ;
	rdfs:domain tolo:Person ;
	skos:definition "The last name of a person."@en ;
	skos:prefLabel "last name"@en ;
	skos:scopeNote "Neutral as to whether the last name is the given or family name."@en ;
	.

tolo:marriedFamilyName
	a owl:DatatypeProperty ;
	rdfs:subPropertyOf tolo:familyName ;
	rdfs:domain tolo:Person ;
	rdfs:range rdf:langString ;
	skos:definition "The family name a person is assigned through a marital relationship."@en ;
	skos:prefLabel "married family name"@en ;
	.

tolo:nameVariant
	a owl:DatatypeProperty ;
	rdfs:subPropertyOf gist:name ;
	skos:altLabel "alternate name"@en ;
	skos:definition "An alternate name for a person."@en ;
	skos:example "Gyergom Nyipa (Wylie gyer sgom gnyis pa) is an alternate name for Gyergom Tsultrim Sengge (Wylie gyer sgom tshul khrims seng+ge)."@en ;
	skos:prefLabel "name variant"@en ;
	skos:scopeNote "The primary/alternate distinction may be source- or system-dependent. Other systems or sources may prefer a name different from Treasury of Lives' primary name."@en ;
	.

tolo:occursDuring
	a
		owl:ObjectProperty ,
		owl:TransitiveProperty
		;
	skos:definition "Relates one temporal resource to another that temporally contains it."@en ;
	skos:example "The birth of Gyergom Tsultrim Sengge occurred during the 12th century."@en ;
	skos:prefLabel "occurs during"@en ;
	skos:scopeNote "Contrasts with tolo:occursDuring, whose subject is a non-temporal resource."@en ;
	gist:domainIncludes
		gist:Event ,
		gist:TemporalRelation ,
		gist:TimeInterval
		;
	gist:rangeIncludes
		gist:Event ,
		gist:TemporalRelation ,
		gist:TimeInterval
		;
	.

tolo:ordinal
	a owl:DatatypeProperty ;
	rdfs:range xsd:integer ;
	skos:definition "An integer used to designate position in a lineage."@en ;
	skos:example "The First Dalai Lama"@en ;
	skos:prefLabel "ordinal"@en ;
	skos:scopeNote
		"Suggested implementation is to store as an integer value and convert to an ordinal for display purposes. This provides more flexibility than storing as an ordinal string."@en ,
		"The ordinal is generally but not always the same as the actual sequence in the lineage (ordered collection). In some incarnation lineages, for example, TBD..."@en
		;
	.

tolo:primaryName
	a owl:DatatypeProperty ;
	rdfs:subPropertyOf gist:name ;
	owl:deprecated "true"^^xsd:boolean ;
	skos:definition "The primary or preferred name of a person or other resource."@en ;
	skos:example "Gyergom Tsultrim Sengge is the primary name of the individual called Gyergom Nyipa by the Library of Congress."@en ;
	skos:prefLabel "primary name"@en ;
	skos:scopeNote
		"The primary/alternate distinction may be source- or system-dependent. Other systems or sources may a different name primary."@en ,
		"The same name may be rendered differently in different transliteration or transcription systems. For example, ToL displays a primary name in both its own and the Extended Wylie systems and possibly others."@en
		;
	.

tolo:residesIn
	a owl:ObjectProperty ;
	rdfs:range gist:Place ;
	skos:definition "Relates something to the place where it lives or exists."@en ;
	skos:prefLabel "resides in"@en ;
	.

tolo:title
	a owl:DatatypeProperty ;
	rdfs:range rdf:langString ;
	skos:definition "An appellation of dignity, honor, distinction, or preeminence attached to a person or family by virtue of rank, office, precedent, privilege, attainment, or lands."@en ;
	skos:prefLabel "title"@en ;
	.

