# imports: https://ontologies.semanticarts.com/o/gistCore11.0.0

@prefix bdo: <http://purl.bdrc.io/ontology/core/> .
@prefix bf: <http://id.loc.gov/ontologies/bibframe/> .
@prefix dct: <http://purl.org/dc/terms/> .
@prefix foaf: <http://xmlns.com/foaf/0.1/> .
@prefix gist: <https://ontologies.semanticarts.com/gist/> .
@prefix owl: <http://www.w3.org/2002/07/owl#> .
@prefix rdf: <http://www.w3.org/1999/02/22-rdf-syntax-ns#> .
@prefix rdfs: <http://www.w3.org/2000/01/rdf-schema#> .
@prefix skos: <http://www.w3.org/2004/02/skos/core#> .
@prefix tol: <https://ontologies.treasuryoflives.org/tol/> .
@prefix tolx: <https://taxonomies.treasuryoflives.org/> .
@prefix vann: <http://purl.org/vocab/vann/> .
@prefix xml: <http://www.w3.org/XML/1998/namespace> .
@prefix xsd: <http://www.w3.org/2001/XMLSchema#> .

<https://ontologies.treasuryoflives.org/tolCore>
	a owl:Ontology ;
	dct:license "TBD"^^xsd:string ;
	vann:preferredNamespacePrefix "tol"^^xsd:string ;
	owl:imports <https://ontologies.semanticarts.com/o/gistCore11.0.0> ;
	owl:versionIRI <https://ontologies.treasuryoflives.org/tolCore0.0.1> ;
	skos:definition "The Treasury of Lives Core Ontology enables the description of historical and contemporary figures in the culture and religion of Tibet, Inner Asia, and the Himalaya. It is used by the Treasury of Lives born-digitial biographical collection (https://treasuryoflives.org) to publish and share its data as Linked Open Data, facilitate the consumption of external RDF, and to to enhance the narrative text with structured data."^^xsd:string ;
	skos:editoralNote
		"Add rdfs:isDefinedBy using onto-toolkit."^^xsd:string ,
		"Combining all terms into one module for now; maybe break up into separate modules later."^^xsd:string
		;
	skos:editorialNote """
		Temporarily removing imports:
			<http://id.loc.gov/ontologies/bibframe-2-1-0> ,
			<http://purl.bdrc.io/ontology/core> to make Protege easier to read."""^^xsd:string ;
	skos:prefLabel "Treasury of Lives Core Ontology"^^xsd:string ;
	.

tol:Birth
	a owl:Class ;
	rdfs:subClassOf
		gist:HistoricalEvent ,
		gist:PhysicalEvent ,
		[
			a owl:Restriction ;
			owl:onProperty tol:isEventOf ;
			owl:allValuesFrom tol:Person ;
		] ,
		[
			a owl:Restriction ;
			owl:onProperty gist:occursIn ;
			owl:cardinality "1"^^xsd:nonNegativeInteger ;
		] ,
		[
			a owl:Restriction ;
			owl:onProperty tol:year ;
			owl:minCardinality "1"^^xsd:nonNegativeInteger ;
		]
		;
	skos:definition "TBD"^^xsd:string ;
	skos:editorialNote "Can deities have birth and death? We may need to loosen the restriction."^^xsd:string ;
	skos:prefLabel "Birth"^^xsd:string ;
	.

tol:Century
	skos:definition "A time period of 100 years reckoned from the birth of Jesus Christ."^^xsd:string ;
	skos:editorialNote "Superclass TBD"^^xsd:string ;
	skos:example "9th century AD"^^xsd:string ;
	skos:prefLabel "Century"^^xsd:string ;
	skos:scopeNote
		"There is disagreement about the first and end years of a century. E.g., strictly, the 18th century is the period 1801-1900, while in common usage it is 1800-1899. The granularity of this distinction is not relevant to our purposes."^^xsd:string ,
		"To be distinguished from an arbitrary period of 100 years, such as 1825-1924."^^xsd:string
		;
	.

tol:Death
	a owl:Class ;
	rdfs:subClassOf
		gist:HistoricalEvent ,
		gist:PhysicalEvent ,
		[
			a owl:Restriction ;
			owl:onProperty tol:isEventOf ;
			owl:allValuesFrom tol:Person ;
		] ,
		[
			a owl:Restriction ;
			owl:onProperty gist:occursIn ;
			owl:cardinality "1"^^xsd:nonNegativeInteger ;
		] ,
		[
			a owl:Restriction ;
			owl:onProperty tol:year ;
			owl:minCardinality "1"^^xsd:nonNegativeInteger ;
		]
		;
	skos:definition "TBD"^^xsd:string ;
	skos:editorialNote "Can deities have birth and death? We may need to loosen the restriction."^^xsd:string ;
	skos:prefLabel "Death"^^xsd:string ;
	.

tol:Deity
	a owl:Class ;
	rdfs:subClassOf gist:LivingThing ;
	owl:disjointWith tol:Person ;
	skos:definition "A god or goddess; a being with divine status."^^xsd:string ;
	skos:prefLabel "Deity"^^xsd:string ;
	.

tol:FraternalNiece
	a owl:ObjectProperty ;
	rdfs:subPropertyOf bdo:hasNiece ;
	owl:propertyChainAxiom (
		bdo:hasBrother
		bdo:hasSon
	) ;
	skos:definition "Relates a person to the daughter of his/her brother."^^xsd:string ;
	skos:prefLabel "has fraternal niece"^^xsd:string ;
	skos:scopeNote
		"We do not currently distinguish biological, adoptive, half, and step relationships."^^xsd:string ,
		"While a niece can be related through either a sibling or sibling-in-law, a fraternal niece is always related through a brother."^^xsd:string
		;
	.

tol:GenealogicalGrouping
	a owl:Class ;
	rdfs:subClassOf
		gist:Collection ,
		[
			a owl:Restriction ;
			owl:onProperty gist:hasMember ;
			owl:allValuesFrom [
				owl:unionOf (
					tol:Person
					tol:GenealogicalGrouping
				) ;
			] ;
		]
		;
	skos:definition "A social unit consisting of people with a common ancestor."^^xsd:string ;
	skos:example "Nuclear family, extended family, clan, tribe."^^xsd:string ;
	skos:prefLabel "Genealogical Grouping"^^xsd:string ;
	skos:scopeNote
		"No subclasses, such as family and clan, are defined because the distinctions are not clear-cut. Instead, we use partitive relationships to describe the relationships between different groupings."^^xsd:string ,
		"This class encompasses successively larger and more inclusive genealogical groupings, such as family and clan. A person is said to be a member of a genealogical grouping, and a smaller genealogical grouping is a member of a larger one."^^xsd:string
		;
	.

tol:HistoricalPeriod
	rdfs:subClassOf
		gist:Category ,
		[
			a owl:Restriction ;
			owl:onProperty gist:actualEndYear ;
			owl:cardinality "1"^^xsd:nonNegativeInteger ;
		] ,
		[
			a owl:Restriction ;
			owl:onProperty gist:actualStartYear ;
			owl:cardinality "1"^^xsd:nonNegativeInteger ;
		]
		;
	rdfs:seeAlso bdo:Era ;
	skos:definition "A time interval having some historical signifance or distinguishing features."^^xsd:string ;
	skos:editorialNote "Not sure if needed."^^xsd:string ;
	skos:example "The Middle Ages"^^xsd:string ;
	skos:prefLabel "Historical Period"^^xsd:string ;
	skos:scopeNote "We assume a historical period is recognized as such only after it is over, thus it always has an endpoint."^^xsd:string ;
	.

tol:Lineage
	a owl:Class ;
	rdfs:subClassOf
		gist:OrderedCollection ,
		[
			a owl:Restriction ;
			owl:onProperty gist:hasOrderedMember ;
			owl:allValuesFrom [
				a owl:Restriction ;
				owl:onProperty gist:providesOrderFor ;
				owl:allValuesFrom tol:Person ;
			] ;
		] ,
		[
			a owl:Restriction ;
			owl:onProperty gist:actualStartYear ;
			owl:cardinality "1"^^xsd:nonNegativeInteger ;
		] ,
		[
			a owl:Restriction ;
			owl:onProperty gist:isBasedOn ;
			owl:cardinality "1"^^xsd:nonNegativeInteger ;
		] ,
		[
			a owl:Restriction ;
			owl:onProperty gist:hasMember ;
			owl:minCardinality "2"^^xsd:nonNegativeInteger ;
		]
		;
	skos:definition "An ordered collection of persons in which a relationship or role is passed sequentially from one to the other."^^xsd:string ;
	skos:editorialNote
		"Figure out whether one lineage can/should be be part of another lineage in a split lineage."^^xsd:string ,
		"TODO need better definition."^^xsd:string
		;
	skos:example "The succession of abbots to a monastery; the transmission of a text from teachers to students; an incarnation sequence."^^xsd:string ;
	skos:prefLabel "Lineage"^^xsd:string ;
	skos:scopeNote "The lineage itself has a start date and possibly an end date; it may have a name; and its ordered members have start and possibly end dates. In some types of lineages the members have numeric designations (e.g., 14th Dalai Lama), in others they are ordered by precedence relationships (e.g., teachers in a teaching lineage). Some but not all types of lineages are strictly ordered, and there may be split lineages with multiple branches descending from a single element in a tree-like structure."^^xsd:string ;
	.

tol:Location
	a owl:Class ;
	skos:definition "A real, fictional, or imaginary place."^^xsd:string ;
	skos:prefLabel "Location"^^xsd:string ;
	skos:scopeNote "Differs from and not a subclass of gist:Place, which includings only places that do or did exist."^^xsd:string ;
	.

tol:Marriage
	a owl:Class ;
	owl:equivalentClass [
		owl:intersectionOf (
			gist:Agreement
			gist:TemporalRelation
			[
				a owl:Restriction ;
				owl:onProperty gist:hasParty ;
				owl:allValuesFrom tol:Person ;
			]
			[
				a owl:Restriction ;
				owl:onProperty gist:hasParty ;
				owl:onClass tol:Person ;
				owl:qualifiedCardinality "2"^^xsd:nonNegativeInteger ;
			]
		) ;
	] ;
	skos:definition "A culturally and often legally recognized union between two people, called spouses, that establishes rights and obligations between them."^^xsd:string ;
	skos:editorialNote
		"Cardinality restriction on gist:hasParty of 2 generates Protege error, so using qualified cardinality restriction instead."^^xsd:string ,
		"Predicates should be directed from the relationship to the other objects, to support named graph drops to delete the relationship."^^xsd:string
		;
	skos:prefLabel "Marriage"^^xsd:string ;
	.

tol:Person
	a owl:Class ;
	rdfs:subClassOf
		bdo:Person ,
		foaf:Person
		;
	skos:definition "A human being, alive, dead, imaginary, or fictional."^^xsd:string ;
	skos:prefLabel "Person"^^xsd:string ;
	skos:scopeNote "Differs from and not a subclass of gist:Person, which includings only persons who do or did exist."^^xsd:string ;
	.

tol:PilgrimageSite
	a owl:Class ;
	rdfs:subClassOf gist:Landmark ;
	skos:definition "A shrine or other sacred place that people travel to as an act of religious devotion."^^xsd:string ;
	skos:editorialNote "Check definition - what types of things can this include?"^^xsd:string ;
	skos:example "Mount Tsibri was the site of Zangpo Drakpa's 14th century treasure revelations; Kokonor Lake"^^xsd:string ;
	skos:prefLabel "Pilgrimage Place"^^xsd:string ;
	.

tol:StrictlyOrderedCollection
	a owl:Class ;
	rdfs:subClassOf gist:OrderedCollection ;
	skos:definition "An ordered collection in which no two members occupy the same position."^^xsd:string ;
	skos:editorialNote "Can we express this axiomatically?"^^xsd:string ;
	skos:preflabel "Strictly Ordered Collection"^^xsd:string ;
	.

tol:Student
	a owl:Class ;
	owl:equivalentClass [
		a owl:Class ;
		owl:intersectionOf (
			tol:Person
			[
				a owl:Restriction ;
				owl:onProperty [
					owl:inverseOf gist:hasRecipient ;
				] ;
				owl:someValuesFrom tol:TeacherStudentRelationship ;
			]
		) ;
	] ;
	skos:definition "A person who receives training in a text or practice from another person (the teacher)."^^xsd:string ;
	skos:editorialNote "Not sure if needed."^^xsd:string ;
	skos:prefLabel "Student"^^xsd:string ;
	.

tol:Teacher
	a owl:Class ;
	owl:equivalentClass [
		a owl:Class ;
		owl:intersectionOf (
			tol:Person
			[
				a owl:Restriction ;
				owl:onProperty [
					owl:inverseOf gist:hasGiver ;
				] ;
				owl:someValuesFrom tol:TeacherStudentRelationship ;
			]
		) ;
	] ;
	skos:definition "A person who transmits a text or practice to another person (the student)."^^xsd:string ;
	skos:editorialNote "Not sure if needed."^^xsd:string ;
	skos:prefLabel "Teacher"^^xsd:string ;
	.

tol:TeacherStudentRelationship
	a owl:Class ;
	owl:equivalentClass [
		a owl:Class ;
		owl:intersectionOf (
			gist:TemporalRelation
			gist:Agreement
			[
				a owl:Restriction ;
				owl:onProperty gist:hasParticipant ;
				owl:cardinality "2"^^xsd:nonNegativeInteger ;
			]
			[
				a owl:Restriction ;
				owl:onProperty gist:hasGiver ;
				owl:allValuesFrom tol:Teacher ;
			]
			[
				a owl:Restriction ;
				owl:onProperty gist:hasGiver ;
				owl:cardinality "1"^^xsd:nonNegativeInteger ;
			]
			[
				a owl:Restriction ;
				owl:onProperty gist:hasRecipient ;
				owl:allValuesFrom tol:Student ;
			]
			[
				a owl:Restriction ;
				owl:onProperty gist:hasRecipient ;
				owl:cardinality "1"^^xsd:nonNegativeInteger ;
			]
			[
				a owl:Restriction ;
				owl:onProperty gist:conformsTo ;
				owl:someValuesFrom gist:Intention ;
			]
		) ;
	] ;
	skos:definition "A time-delimited relationship between a teacher and a student."^^xsd:string ;
	skos:editorialNote
		"How to express what the Intention is? I.e., how should an intention be instantiated?"^^xsd:string ,
		"Predicates should be directed from the relationship to the other objects, to support named graph drops to delete the relationship."^^xsd:string ,
		"TODO Add relationship to text (bf:Text?) or Practice (subclass of gist:Behavior? - need to see examples."^^xsd:string
		;
	skos:prefLabel "Teacher-Student Relationship"^^xsd:string ;
	skos:scopeNote "A teacher-student relationshp may be, but is not necessarily, part of a teaching lineage. In some cases the teacher-student relationship is known while the lineage is not."^^xsd:string ;
	.

tol:TeachingLineage
	a owl:Class ;
	owl:disjointWith tol:IncarnationLineage ;
	owl:equivalentClass [
		a owl:Class ;
		owl:intersectionOf (
			tol:Lineage
			[
				a owl:Restriction ;
				owl:onProperty gist:hasOrderedMember ;
				owl:allValuesFrom [
					a owl:Restriction ;
					owl:onProperty gist:providesOrderFor ;
					owl:allValuesFrom tol:Teacher ;
				] ;
			]
			[
				a owl:Restriction ;
				owl:onProperty gist:hasDirectPart ;
				owl:onClass tol:TeacherStudentRelationship ;
				owl:minQualifiedCardinality "2"^^xsd:nonNegativeInteger ;
			]
			[
				a owl:Restriction ;
				owl:onProperty gist:hasOrderedMember ;
				owl:allValuesFrom [
					a owl:Restriction ;
					owl:onProperty gist:sequence ;
					owl:maxCardinality "0"^^xsd:nonNegativeInteger ;
				] ;
			]
		) ;
	] ;
	skos:definition "An ordered collection of teachers transmitting a specific text or practice to their students."^^xsd:string ;
	skos:prefLabel "Teaching Lineage"^^xsd:string ;
	skos:scopeNote "Teachers in a lineage are not designated numerically (as are, e.g., persons in an incarnation lineage), but are ordered through gist:precedesDirectly. Elements in the lineage may certainly co-occur or overlap."^^xsd:string ;
	.

tol:actualYear
	a owl:DatatypeProperty ;
	rdfs:subPropertyOf tol:year ;
	skos:definition "The year in which something existed or took place."^^xsd:string ;
	skos:example "Gyergom Tsultime Sengge was born in 1144 and died in 1204."^^xsd:string ;
	skos:prefLabel "actual year"^^xsd:string ;
	.

tol:approximateYear
	a owl:DatatypeProperty ;
	rdfs:subPropertyOf tol:year ;
	skos:definition "The approximate year in which something existed or took place."^^xsd:string ;
	skos:example "Lhagyari Namgyel Gyatso was born in approximately 1927."^^xsd:string ;
	skos:prefLabel "approximate year"^^xsd:string ;
	.

tol:dissolutionYear
	a owl:DatatypeProperty ;
	rdfs:subPropertyOf tol:actualYear ;
	skos:definition "The year an agreement such as marriage was ended. In the case of marriage, this refers to divorce rather than the end of a marriage by death of one of the spouses."^^xsd:string ;
	skos:editorialNote
		"Use if we need to distinguish divorce from death as the end of a marriage."^^xsd:string ,
		"We may want to do this like birth and death - have a Dissolution object with a year. If there are many things with actual/probable/possible/approximate years (dissolution, founding, etc.) we should establish this as a general pattern."^^xsd:string
		;
	skos:prefLabel "dissolution year"^^xsd:string ;
	.

tol:foundedInYear
	a owl:DatatypeProperty ;
	rdfs:subPropertyOf gist:actualStartYear ;
	skos:definition "TODO"^^xsd:string ;
	skos:editorialNote "We may want to follow the pattern of Birth and Death here, instead of just using a property. Depends on what other information is available. We could have Founding with an agent and a date."^^xsd:string ;
	skos:example "The Tshal-pa tradition was founded in 1123."^^xsd:string ;
	skos:prefLabel "founded in year"^^xsd:string ;
	skos:scopeNote "What is the end date on a tradition? Do we need a predicate other than gist:actualEndYear?"^^xsd:string ;
	.

tol:harUrl
	a owl:AnnotationProperty ;
	rdfs:subPropertyOf rdfs:seeAlso ;
	rdfs:range xsd:anyURI ;
	skos:definition "The URL to the main page about this resource on the Himalayan Art Resources (HAR) site."^^xsd:string ;
	skos:prefLabel "HAR URL"^^xsd:string ;
	.

tol:hasAssignedGender
	rdfs:domain tol:Person ;
	rdfs:range bdo:Gender ;
	skos:definition "The gender of a person assigned at birth."^^xsd:string ;
	skos:example "Jetsun Khacho Wangmo waas assigned male gender at birth, but later identified as female."^^xsd:string ;
	skos:prefLabel "has assigned gender"^^xsd:string ;
	skos:scopeNote "Use if a distinction is made between assigned gender and identified gender; otherwise use bdo:personGender."^^xsd:string ;
	.

tol:hasEvent
	a owl:ObjectProperty ;
	rdfs:range gist:Event ;
	skos:definition "Relates something to an event pertaining to it."^^xsd:string ;
	skos:example "A person's birth or death; the founding of an institution; the dissolution of a marriage."^^xsd:string ;
	skos:prefLabel "has event"^^xsd:string ;
	.

tol:hasFinalRestingPlace
	a owl:ObjectProperty ;
	rdfs:subPropertyOf gist:hasPhysicalLocation ;
	rdfs:domain tol:Person ;
	skos:definition "Relates a person to (one of) his/her final resting place(s)."^^xsd:string ;
	skos:prefLabel "has final resting place"^^xsd:string ;
	skos:scopeNote "Significant people such as the Dalai Lamas have reliquary stupas in geographic locations like temples or chapels. Sometimes there can be relics in multiple places."^^xsd:string ;
	.

tol:hasFraternalCousin
	a owl:ObjectProperty ;
	rdfs:subPropertyOf bdo:hasCousin ;
	skos:definition "Relates a person to his/her cousin on the father's side."^^xsd:string ;
	skos:prefLabel "has fraternal cousin"^^xsd:string ;
	skos:scopeNote "We do not currently distinguish biological, adoptive, half, and step relationships."^^xsd:string ;
	.

tol:hasFraternalNephew
	a owl:ObjectProperty ;
	rdfs:subPropertyOf bdo:hasNephew ;
	owl:propertyChainAxiom (
		bdo:hasBrother
		bdo:hasSon
	) ;
	skos:definition "Relates a person to the son of his/her brother."^^xsd:string ;
	skos:prefLabel "has fraternal nephew"^^xsd:string ;
	skos:scopeNote
		"We do not currently distinguish biological, adoptive, half, and step relationships."^^xsd:string ,
		"While a nephew can be related through either a sibling or sibling-in-law, a fraternal nephew is always related through a brother."^^xsd:string
		;
	.

tol:hasMaternalCousin
	a owl:ObjectProperty ;
	rdfs:subPropertyOf bdo:hasCousin ;
	skos:definition "Relates a person to his/her cousin on the mother's side."^^xsd:string ;
	skos:prefLabel "has maternal cousin"^^xsd:string ;
	skos:scopeNote "We do not currently distinguish biological, adoptive, half, and step relationships."^^xsd:string ;
	.

tol:hasMaternalGrandfather
	a owl:ObjectProperty ;
	rdfs:subPropertyOf
		bdo:hasGrandfather ,
		tol:hasMaternalGrandparent
		;
	owl:propertyChainAxiom (
		tol:hasMother
		tol:hasFather
	) ;
	skos:definition "Relates a person to his/her mother's father."^^xsd:string ;
	skos:prefLabel "has maternal grandfather"^^xsd:string ;
	skos:scopeNote "We do not currently distinguish biological, adoptive, half, and step relationships."^^xsd:string ;
	.

tol:hasMaternalGrandmother
	a owl:ObjectProperty ;
	rdfs:subPropertyOf
		bdo:hasGrandmother ,
		tol:hasMaternalGrandparent
		;
	owl:propertyChainAxiom (
		bdo:hasMother
		bdo:hasMother
	) ;
	skos:definition "Relates a person to his/her mother's mother."^^xsd:string ;
	skos:prefLabel "has maternal grandmother"^^xsd:string ;
	skos:scopeNote "We do not currently distinguish biological, adoptive, half, and step relationships."^^xsd:string ;
	.

tol:hasMaternalGrandparent
	a owl:ObjectProperty ;
	rdfs:subPropertyOf bdo:hasGrandmother ;
	owl:propertyChainAxiom (
		bdo:hasMother
		bdo:hasParent
	) ;
	skos:definition "Relates a person to his/her mother's parent."^^xsd:string ;
	skos:prefLabel "has maternal grandmother"^^xsd:string ;
	skos:scopeNote "We do not currently distinguish biological, adoptive, half, and step relationships."^^xsd:string ;
	.

tol:hasPaternalGrandfather
	a owl:ObjectProperty ;
	rdfs:subPropertyOf
		bdo:hasGrandfather ,
		tol:hasPaternalGrandparent
		;
	owl:propertyChainAxiom (
		bdo:hasFather
		bdo:hasFather
	) ;
	skos:definition "Relates a person to his/her father's father."^^xsd:string ;
	skos:prefLabel "has paternal grandfather"^^xsd:string ;
	skos:scopeNote "We do not currently distinguish biological, adoptive, half, and step relationships."^^xsd:string ;
	.

tol:hasPaternalGrandmother
	a owl:ObjectProperty ;
	rdfs:subPropertyOf
		bdo:hasGrandmother ,
		tol:hasPaternalGrandparent
		;
	owl:propertyChainAxiom (
		bdo:hasFather
		bdo:hasMother
	) ;
	skos:definition "Relates a person to his/her father's mother."^^xsd:string ;
	skos:prefLabel "has paternal grandmother"^^xsd:string ;
	skos:scopeNote "We do not currently distinguish biological, adoptive, half, and step relationships."^^xsd:string ;
	.

tol:hasPaternalGrandparent
	a owl:ObjectProperty ;
	rdfs:subPropertyOf bdo:hasGrandparent ;
	owl:propertyChainAxiom (
		bdo:hasFather
		bdo:hasParent
	) ;
	skos:definition "Relates a person to his/her fathers's parent."^^xsd:string ;
	skos:prefLabel "has maternal grandmother"^^xsd:string ;
	skos:scopeNote "We do not currently distinguish biological, adoptive, half, and step relationships."^^xsd:string ;
	.

tol:hasSororallNephew
	a owl:ObjectProperty ;
	rdfs:subPropertyOf bdo:hasNephew ;
	owl:propertyChainAxiom (
		bdo:hasSister
		bdo:hasSon
	) ;
	skos:definition "Relates a person to his/her sister's son."^^xsd:string ;
	skos:prefLabel "has sororal nephew"^^xsd:string ;
	skos:scopeNote
		"We do not currently distinguishbiological, adoptive, half, and step relationships."^^xsd:string ,
		"While a nephew can be related through either a sibling or sibling-in-law, a sororal nephew is always related through a sister."^^xsd:string
		;
	.

tol:hasSororallNiece
	a owl:ObjectProperty ;
	rdfs:subPropertyOf bdo:hasNiece ;
	owl:propertyChainAxiom (
		bdo:hasSister
		bdo:hasDaughter
	) ;
	skos:definition "Relates a person to his/her sister's daughter."^^xsd:string ;
	skos:prefLabel "has sororal niece"^^xsd:string ;
	skos:scopeNote
		"We do not currently distinguish biological, adoptive, half, and step relationships."^^xsd:string ,
		"While a niece can be related through either a sibling or sibling-in-law, a sororal nephew is always related through a sister."^^xsd:string
		;
	.

tol:identifiesAsGender
	rdfs:subPropertyOf bdo:personGender ;
	rdfs:domain tol:Person ;
	rdfs:range bdo:Gender ;
	skos:definition "The gender a person identifies as."^^xsd:string ;
	skos:example "Jetsun Khacho Wangmo waas assigned male gender at birth, but later identified as female."^^xsd:string ;
	skos:prefLabel "identifies as gender"^^xsd:string ;
	skos:scopeNote "Use if a distinction is made between assigned gender and identified gender; otherwise use bdo:personGender."^^xsd:string ;
	.

tol:isEventOf
	a owl:ObjectProperty ;
	owl:inverseOf tol:hasEvent ;
	skos:definition "Relates an event to the thing it pertains to."^^xsd:string ;
	skos:example "A person's birth or death; the founding of an institution; the dissolution of a marriage."^^xsd:string ;
	skos:prefLabel "is event of"^^xsd:string ;
	.

tol:isInCentury
	a owl:DatatypeProperty ;
	rdfs:range tol:Century ;
	skos:definition "Relates something to the time period in which it exists (existed) or takes (took) place."^^xsd:string ;
	skos:example "Lasum Gyelwa Jangchub was born in the early 8th century; Rinchen Chok died in the 1st century; Khenchen Tashi Tsultrim was borth in the late 13th century."^^xsd:string ;
	skos:prefLabel "is in time period"^^xsd:string ;
	.

tol:possibleYear
	a owl:DatatypeProperty ;
	rdfs:subPropertyOf tol:year ;
	skos:definition "The year in which something existed or took place."^^xsd:string ;
	skos:example "The birth year of Kunkyong Lingpa is commonly accepted to be 1396 (probable year), though some have suggested that he was born in 1408 (possible year)."^^xsd:string ;
	skos:prefLabel "possible year"^^xsd:string ;
	skos:scopeNote "If the year is controversial, this is the less commonly accepted one, and the more commonly accepted one is expressed by tol:probableYear."^^xsd:string ;
	.

tol:probableYear
	a owl:DatatypeProperty ;
	rdfs:subPropertyOf tol:year ;
	skos:definition "The year in which something is likely to have existed or taken place."^^xsd:string ;
	skos:example "The birth year of Kunkyong Lingpa is commonly accepted to be 1396 (probable year), though some have suggested that he was born in 1408 (possible year)."^^xsd:string ;
	skos:prefLabel "probable year"^^xsd:string ;
	skos:scopeNote "If the year is controversial, this is the most commonly accepted one, and the less commonly accepted ones are expressed by tol:possibleYear."^^xsd:string ;
	.

tol:title
	a owl:DatatypeProperty ;
	rdfs:range rdf:langString ;
	skos:definition "An appellation of dignity, honor, distinction, or preeminence attached to a person or family by virtue of rank, office, precedent, privilege, attainment, or lands."^^xsd:string ;
	skos:prefLabel "title"^^xsd:string ;
	.

tol:year
	a owl:DatatypeProperty ;
	rdfs:subPropertyOf gist:atDateTime ;
	skos:definition "The year in which something existed or took place, including actual, approximate, probable, and possible values."^^xsd:string ;
	skos:editorialNote "The modalities actual, approximate, probable, and possible, expressed here with subproperties, could be more naturally modeled with RDF*."^^xsd:string ;
	skos:example "The year a birth took place; the year a death may have taken place; an approximate year of birth; the most likely date of death."^^xsd:string ;
	skos:prefLabel "year"^^xsd:string ;
	.

