# imports: https://w3id.org/semanticarts/ontology/gistCore13.0.0

@prefix bdo: <http://purl.bdrc.io/ontology/core/> .
@prefix gist: <https://w3id.org/semanticarts/ns/ontology/gist/> .
@prefix owl: <http://www.w3.org/2002/07/owl#> .
@prefix rdf: <http://www.w3.org/1999/02/22-rdf-syntax-ns#> .
@prefix rdfs: <http://www.w3.org/2000/01/rdf-schema#> .
@prefix skos: <http://www.w3.org/2004/02/skos/core#> .
@prefix told: <https://w3id.org/treasuryoflives/ns/data/tol/> .
@prefix tolo: <https://w3id.org/treasuryoflives/ns/ontology/tol/> .
@prefix tolx: <https://w3id.org/treasuryoflives/ns/taxonomy/tol/> .
@prefix wiki: <https://www.wikidata.org/wiki/> .
@prefix xsd: <http://www.w3.org/2001/XMLSchema#> .

<https://w3id.org/treasuryoflives/ontology/tolCoreX.x.x>
	a owl:Ontology ;
	owl:imports <https://w3id.org/semanticarts/ontology/gistCore13.0.0> ;
	owl:versionIRI <https://w3id.org/treasuryoflives/ontology/tolCoreX.x.x> ;
	skos:definition "The Treasury of Lives Core Ontology enables the description of historical and contemporary figures in the culture and religion of Tibet, Inner Asia, and the Himalaya. It is used by the Treasury of Lives born-digitial biographical collection (https://treasuryoflives.org) to publish and share its data as Linked Open Data, facilitate the consumption of external RDF, and to to enhance the narrative text with structured data."@en ;
	skos:prefLabel "Treasury of Lives Core Ontology"@en ;
	gist:license "https://creativecommons.org/licenses/by/4.0/"^^xsd:anyURI ;
	.

tolo:Author
	a owl:Class ;
	owl:equivalentClass [
		a owl:Class ;
		owl:intersectionOf (
			gist:Person
			[
				a owl:Restriction ;
				owl:onProperty [
					owl:inverseOf gist:hasParticipant ;
				] ;
				owl:someValuesFrom tolo:Authorship ;
			]
		) ;
	] ;
	skos:definition "A person who has authored or contributed to authoring at least one work."@en ;
	skos:prefLabel "Author"@en ;
	.

tolo:AuthorDisclosure
	a owl:Class ;
	owl:equivalentClass [
		a owl:Class ;
		owl:intersectionOf (
			gist:Text
			[
				a owl:Restriction ;
				owl:onProperty [
					owl:inverseOf gist:refersTo ;
				] ;
				owl:someValuesFrom tolo:Biography ;
			]
		) ;
	] ;
	skos:definition "A disclaimer or disclosure made by the author of a biography."@en ;
	skos:example "A statement indicating that the author of the biography is a relative or student of its subject."@en ;
	skos:prefLabel "Author Disclosure"@en ;
	.

tolo:Authorship
	a owl:Class ;
	owl:equivalentClass [
		a owl:Class ;
		owl:intersectionOf (
			gist:TemporalRelation
			[
				a owl:Restriction ;
				owl:onProperty gist:hasParticipant ;
				owl:someValuesFrom tolo:Author ;
			]
			[
				a owl:Restriction ;
				owl:onProperty gist:hasParticipant ;
				owl:someValuesFrom tolo:Biography ;
			]
		) ;
	] ;
	skos:definition "Relates a bio to a person who has authored it."@en ;
	skos:editorialNote "Using a simple model of authorship until there is a use case for a more complex model with a generic Contribution class and roles as in BIBFRAME."@en ;
	skos:prefLabel "Authorship"@en ;
	.

tolo:Biography
	a owl:Class ;
	rdfs:subClassOf
		gist:FormattedContent ,
		[
			a owl:Restriction ;
			owl:onProperty gist:isAbout ;
			owl:someValuesFrom tolo:Person ;
		]
		;
	skos:definition "A written account of another person's life."@en ;
	skos:prefLabel "Biography"@en ;
	skos:scopeNote
		"Author bios are not instances of tolo:Biography because authors are instances of gist:Person but not tolo:Person."@en ,
		"This definition glosses over the distinction between ContentExpression and FormattedContent. The biography itself is a ContentExpression, the HTML version is FormattedContent, but creating and linking distinct instances of each type entails overhead without apparent benefit."@en
		;
	.

tolo:Birth
	a owl:Class ;
	rdfs:subClassOf
		gist:PhysicalEvent ,
		[
			a owl:Restriction ;
			owl:onProperty gist:hasParticipant ;
			owl:allValuesFrom tolo:Person ;
		] ,
		[
			a owl:Restriction ;
			owl:onProperty gist:hasParticipant ;
			owl:cardinality "1"^^xsd:nonNegativeInteger ;
		] ,
		[
			a owl:Restriction ;
			owl:onProperty gist:atDateTime ;
			owl:someValuesFrom rdfs:Literal ;
		]
		;
	owl:disjointWith tolo:Death ;
	skos:definition "The event of being born."@en ;
	skos:prefLabel "Birth"@en ;
	.

tolo:Collection
	a owl:Class ;
	rdfs:subClassOf
		gist:Collection ,
		[
			a owl:Restriction ;
			owl:onProperty [
				owl:inverseOf gist:isMemberOf ;
			] ;
			owl:someValuesFrom gist:IntellectualProperty ;
		]
		;
	skos:definition "An art collection, museum, or archive that houses original works of art and/or archival documents."@en ;
	skos:example "Cleveland Museum of Art, Collection of Shelley and Donald Rubin, Estate of Lobsang P. Lhalungpa."@en ;
	skos:prefLabel "Collection"@en ;
	.

tolo:Death
	a owl:Class ;
	rdfs:subClassOf
		gist:PhysicalEvent ,
		[
			a owl:Restriction ;
			owl:onProperty gist:hasParticipant ;
			owl:allValuesFrom tolo:Person ;
		] ,
		[
			a owl:Restriction ;
			owl:onProperty gist:hasParticipant ;
			owl:cardinality "1"^^xsd:nonNegativeInteger ;
		] ,
		[
			a owl:Restriction ;
			owl:onProperty gist:atDateTime ;
			owl:someValuesFrom rdfs:Literal ;
		]
		;
	skos:definition "The end of a life."@en ;
	skos:prefLabel "Death"@en ;
	.

tolo:EntityActiveStatus
	a owl:Class ;
	rdfs:subClassOf gist:Category ;
	skos:definition "Indicates whether an entity is active or inactive."@en ;
	skos:prefLabel "Entity Active Status"@en ;
	skos:scopeNote "Can be applied to many types of entities."@en ;
	.

tolo:Founding
	a owl:Class ;
	rdfs:subClassOf
		gist:Event ,
		[
			a owl:Restriction ;
			owl:onProperty gist:hasParticipant ;
			owl:onClass gist:Place ;
			owl:qualifiedCardinality "1"^^xsd:integer ;
		] ,
		[
			a owl:Restriction ;
			owl:onProperty gist:hasParticipant ;
			owl:someValuesFrom tolo:Person ;
		]
		;
	skos:definition "The event of establishng or originating an institution such as a monastery. A founding object is used to attach various dates (year, alternate year, century, etc.), as well as one or more founders, to the institution."@en ;
	skos:prefLabel "Founding"@en ;
	skos:scopeNote "Could be extended to traditions if dates are added to the data. These are currently connected to founders via the direct object property tolo:hasFounder because there are no dates. "@en ;
	.

tolo:HistoricalPeriod
	a owl:Class ;
	rdfs:subClassOf gist:TimeInterval ;
	skos:definition "A named time interval with historical significance."@en ;
	skos:example "The 10th century, the eary/mid/late 19th century."@en ;
	skos:prefLabel "Historical Period"@en ;
	skos:scopeNote "Whereas a time interval is any period of time, such as 2-4pm this afternoon or 1848-1947, a historical period is named and cited in relation to historical events or culture. Historical periods include full and partial centuries, which are ordinally numbered."@en ;
	.

tolo:HusbandStatus
	a owl:Class ;
	rdfs:subClassOf
		gist:Category ,
		[
			a owl:Restriction ;
			owl:onProperty [
				owl:inverseOf gist:isCategorizedBy ;
			] ;
			owl:allValuesFrom tolo:Marriage ;
		]
		;
	skos:definition "Indicates whether a marriage relationship has a junior or senior husband."@en ;
	skos:example "Junior, senior"@en ;
	skos:prefLabel "Husband Status"@en ;
	.

tolo:IdType
	a owl:Class ;
	rdfs:subClassOf gist:Category ;
	skos:definition "A kind of identifier, usually associated with an allocating organization."@en ;
	skos:example "Gendun Drub has Himalayan Art (HAR) identifier 582."@en ;
	skos:prefLabel "ID Type"@en ;
	skos:scopeNote "In some cases, the ID type can be used to construct links by specifying a URL fragment to combine with the identifier to form a URL and a display label to use as link text."@en ;
	.

tolo:Image
	a owl:Class ;
	rdfs:subClassOf gist:FormattedContent ;
	skos:definition "A formatted content object with an image media type."@en ;
	skos:prefLabel "Image"@en ;
	.

tolo:Incarnation
	a owl:Class ;
	rdfs:subClassOf [
		a owl:Restriction ;
		owl:onProperty gist:isMemberOf ;
		owl:allValuesFrom tolo:IncarnationLineage ;
	] ;
	owl:equivalentClass [
		a owl:Class ;
		owl:intersectionOf (
			tolo:LineageMember
			[
				a owl:Restriction ;
				owl:onProperty gist:isMemberOf ;
				owl:someValuesFrom tolo:IncarnationLineage ;
			]
		) ;
	] ;
	skos:definition "The relationship connecting a person to an incarnation lineage and expressing the sequence and ordinal of the person in the lineage."@en ;
	skos:example "The Third Dalai Lama."@en ;
	skos:prefLabel
		"Incarnation"@en ,
		"sprul sku"@bo-x-ewts
		;
	skos:scopeNote "The sequence is used to impose a chronological order on the incarnations, and is required, while the ordinal, which is optional, indicates the numbering according to some tradition. They are typically but not always the same. See tolo:ordinal."@en ;
	.

tolo:IncarnationLineage
	a owl:Class ;
	rdfs:subClassOf [
		a owl:Restriction ;
		owl:onProperty [
			owl:inverseOf gist:isMemberOf ;
		] ;
		owl:allValuesFrom tolo:Incarnation ;
	] ;
	owl:equivalentClass [
		a owl:Class ;
		owl:intersectionOf (
			tolo:Lineage
			[
				a owl:Restriction ;
				owl:onProperty [
					owl:inverseOf gist:isMemberOf ;
				] ;
				owl:someValuesFrom tolo:Incarnation ;
			]
		) ;
	] ;
	skos:definition "A consecutive line of people regarded as incarnations of a non-living person or mythical figure."@en ;
	skos:example "The Dalai Lamas, the Karmapas."@en ;
	skos:prefLabel
		"Incarnation Lineage"@en ,
		"skye brgyud"@bo-x-ewts
		;
	skos:scopeNote "An incarnation lineage is enumerated chronologically and can branch into multiple lines. Usually associated with a seat, such as a monastery, and a tradition."@en ;
	.

tolo:KinshipGroup
	a owl:Class ;
	rdfs:subClassOf
		gist:Collection ,
		[
			a owl:Restriction ;
			owl:onProperty [
				owl:inverseOf gist:isMemberOf ;
			] ;
			owl:allValuesFrom [
				a owl:Class ;
				owl:unionOf (
					tolo:Person
					tolo:Marriage
					tolo:RulerLineage
				) ;
			] ;
		] ,
		[
			a owl:Restriction ;
			owl:onProperty [
				owl:inverseOf gist:isMemberOf ;
			] ;
			owl:someValuesFrom owl:Thing ;
		]
		;
	skos:definition "A social unit consisting of people with a common ancestor."@en ;
	skos:example "The Adro clan; the Jangling family."@en ;
	skos:prefLabel "Kinship Group"@en ;
	skos:scopeNote "Includes Tibetan concepts that may individually mean something more specific, such as: rig (rigs) for clan, race, family; gyu (rgyud) for lineage, descent; dungrab (gdung rabs) for descendants, lineage, generation; dung (gdung) for progeny, descendants, lineage, descent line; ru (rus) for bone, bloodline, lineage, family, clan; khang (khang) for household and tsang (tshang) for family and household. Marriages are also members of kinship groups, distinguishing patrilocal from matrilocal marriages."@en ;
	.

tolo:KinshipGroupType
	a owl:Class ;
	owl:equivalentClass [
		owl:intersectionOf (
			gist:Category
			[
				a owl:Restriction ;
				owl:onProperty [
					owl:inverseOf gist:isCategorizedBy ;
				] ;
				owl:allValuesFrom tolo:KinshipGroup ;
			]
		) ;
	] ;
	skos:definition "A type of kinship group."@en ;
	skos:example "Lhasa aristocracy, clan."@en ;
	skos:prefLabel "Kinship Group Type"@en ;
	.

tolo:Lineage
	a owl:Class ;
	rdfs:subClassOf [
		a owl:Restriction ;
		owl:onProperty [
			owl:inverseOf gist:isMemberOf ;
		] ;
		owl:allValuesFrom tolo:LineageMember ;
	] ;
	owl:equivalentClass [
		a owl:Class ;
		owl:intersectionOf (
			gist:OrderedCollection
			[
				a owl:Restriction ;
				owl:onProperty [
					owl:inverseOf gist:isMemberOf ;
				] ;
				owl:someValuesFrom tolo:LineageMember ;
			]
		) ;
	] ;
	skos:definition "A line of persons serving in a certain role or function, such as the heads of a particular monastery or an incarnation lineage."@en ;
	skos:prefLabel "Lineage"@en ;
	.

tolo:LineageMember
	a owl:Class ;
	owl:equivalentClass [
		a owl:Class ;
		owl:intersectionOf (
			gist:OrderedMember
			[
				a owl:Restriction ;
				owl:onProperty gist:providesOrderFor ;
				owl:someValuesFrom tolo:Person ;
			]
			[
				a owl:Restriction ;
				owl:onProperty gist:isMemberOf ;
				owl:someValuesFrom tolo:Lineage ;
			]
		) ;
	] ;
	skos:definition "An ordered member that relates a lineage to a person in the lineage."@en ;
	skos:prefLabel "Lineage Member"@en ;
	.

tolo:Marriage
	a owl:Class ;
	owl:equivalentClass [
		owl:intersectionOf (
			gist:Agreement
			[
				a owl:Restriction ;
				owl:onProperty tolo:hasWife ;
				owl:someValuesFrom tolo:Person ;
			]
			[
				a owl:Restriction ;
				owl:onProperty tolo:hasHusband ;
				owl:someValuesFrom tolo:Person ;
			]
			[
				a owl:Restriction ;
				owl:onProperty gist:isMemberOf ;
				owl:someValuesFrom tolo:KinshipGroup ;
			]
		) ;
	] ;
	skos:definition "A culturally and often legally recognized union between two people, called spouses, that establishes rights and obligations between them."@en ;
	skos:prefLabel "Marriage"@en ;
	skos:scopeNote "A marriage is associated with the birth kinship group of either the husband ('patrilocal') or wife ('matrilocal')."@en ;
	.

tolo:MarriageTerminationCause
	a owl:Class ;
	rdfs:subClassOf
		gist:Category ,
		[
			a owl:Restriction ;
			owl:onProperty [
				owl:inverseOf gist:isCategorizedBy ;
			] ;
			owl:allValuesFrom tolo:Marriage ;
		]
		;
	skos:definition "The reason for the termination of a marriage."@en ;
	skos:example "Death, divorce, dissolution."@en ;
	skos:prefLabel "Marriage Termination Cause"@en ;
	.

tolo:Monastery
	a owl:Class ;
	owl:equivalentClass [
		a owl:Class ;
		owl:intersectionOf (
			gist:Place
			[
				a owl:Restriction ;
				owl:onProperty gist:isCategorizedBy ;
				owl:oneOf (
					tolx:_PlaceType_monastery
					tolx:_PlaceType_nunnery
				) ;
			]
			[
				a owl:Restriction ;
				owl:onProperty [
					owl:inverseOf gist:hasParticipant ;
				] ;
				owl:someValuesFrom tolo:Founding ;
			]
			[
				a owl:Restriction ;
				owl:onProperty [
					owl:inverseOf gist:hasParticipant ;
				] ;
				owl:someValuesFrom tolo:Founding ;
			]
			[
				a owl:Restriction ;
				owl:onProperty gist:isConnectedTo ;
				owl:someValuesFrom tolo:MonasteryLineage ;
			]
		) ;
	] ;
	skos:definition "A community of ordained individuals affiliated with a particular religious tradition with a common annual ritual calendar and rules. The community is organized hierarchically, with established roles such as abbot, treasurer, and the like. Human-created structures such as temples, assembly halls, residential houses and meditation halls are typical features."@en ;
	skos:prefLabel
		"Monastery"@en ,
		"dgon pa"@bo-x-ewts ,
		"དགོན་པ་"@bo ,
		"寺院"@zh-HANI
		;
	skos:scopeNote "This term designates both tje community and the physical structures that house it. Note that nunneries are included but differentiated by place type."@en ;
	.

tolo:MonasteryLineage
	a owl:Class ;
	owl:equivalentClass [
		a owl:Class ;
		owl:intersectionOf (
			tolo:Lineage
			[
				a owl:Restriction ;
				owl:onProperty gist:isCategorizedBy ;
				owl:oneOf (
					tolx:_Role_monastery_head
					tolx:_Role_lay_administrator
				) ;
			]
			[
				a owl:Restriction ;
				owl:onProperty gist:isConnectedTo ;
				owl:someValuesFrom tolo:Monastery ;
			]
		) ;
	] ;
	skos:definition "A lineage of heads or lay administrators of a particular monastery."@en ;
	skos:example "Katok Khenpo, Drepung are monastery head lineages."@en ;
	skos:prefLabel "Monastery Lineage"@en ;
	.

tolo:PeerReviewStatus
	a owl:Class ;
	rdfs:subClassOf gist:Category ;
	skos:definition "Indicates whether a work, such as a Treasury of Lives biography, has been peer-reviewed."@en ;
	skos:prefLabel "Peer Review Status"@en ;
	.

tolo:Person
	a owl:Class ;
	rdfs:subClassOf
		bdo:Person ,
		gist:Person ,
		wiki:Person
		;
	skos:definition "An individual being who was born, lived, and died in the human realm and is or potentially is the subject of a Treasury of Lives biography."@en ;
	skos:prefLabel
		"Person"@en ,
		"mi"@bo-x-ewts
		;
	skos:scopeNote "May include quasi-historical figures. Encompasses persons from other data sources, such as BDRC, who are referenced from biographies but do not have a biography on the ToL site. Other persons in the data such as users, subscriber contacts, and authors are instances of gist:Person rather than tolo:Person (unless they also become the subject of a biography)."@en ;
	.

tolo:PlaceType
	a owl:Class ;
	rdfs:subClassOf
		gist:Category ,
		[
			a owl:Restriction ;
			owl:onProperty [
				owl:inverseOf gist:isCategorizedBy ;
			] ;
			owl:allValuesFrom gist:Place ;
		]
		;
	skos:definition "A category indicating a kind of place based on natural features or human-designated function."@en ;
	skos:example "Lake, mountain, monastery, school, temple, hermitage."@en ;
	skos:prefLabel "Place Type"@en ;
	skos:scopeNote
		"Some places may have more than one type; e.g., a cave may also function as a hermitage."@en ,
		"There is no clear line between what we might think of as institutions or organizations, such as a monastic order, and the physical structures that house them, so they are all typed as gist:Place and categorized with a tolo:PlaceType."@en
		;
	.

tolo:RegionType
	a owl:Class ;
	rdfs:subClassOf gist:Category ;
	skos:definition "A type of geographic region."@en ;
	skos:example "County seat, folk region."@en ;
	skos:prefLabel "Region Type"@en ;
	.

tolo:Role
	a owl:Class ;
	rdfs:subClassOf gist:Category ;
	skos:definition "A role, office, or vocation played by a person, typically, though not always, in an institutional context."@en ;
	skos:example "Artist, government officer, monastic officer, Indian master."@en ;
	skos:prefLabel "Role"@en ;
	.

tolo:RulerLineage
	a owl:Class ;
	owl:equivalentClass [
		a owl:Class ;
		owl:intersectionOf (
			tolo:Lineage
			[
				a owl:Restriction ;
				owl:onProperty gist:isCategorizedBy ;
				owl:hasValue tolx:_Role_ruler ;
			]
			[
				a owl:Restriction ;
				owl:onProperty gist:isConnectedTo ;
				owl:someValuesFrom gist:GeoRegion ;
			]
			[
				a owl:Restriction ;
				owl:onProperty gist:isMemberOf ;
				owl:someValuesFrom tolo:KinshipGroup ;
			]
		) ;
	] ;
	skos:definition "A lineage of members of a royal family who inherit the role of ruler of the home region. In addition to a kinship group and region, the lineage may also be associated with a place or institution, such as a palace or monastery."@en ;
	skos:example "Derge, Chone."@en ;
	skos:prefLabel "Ruler Lineage"@en ;
	.

tolo:Sponsor
	a owl:Class ;
	rdfs:subClassOf [
		a owl:Class ;
		owl:unionOf (
			gist:Person
			gist:Organization
		) ;
	] ;
	skos:definition "An organization or person who provides funds for a project or activity."@en ;
	skos:prefLabel "Sponsor"@en ;
	skos:scopeNote "Many but not all sponsors are linked to particular biographies that they sponsor. A class is needed in addition to the predicate isSponsoredBy to identify sponsors not connected to individual biographies."@en ;
	.

tolo:StatusAssignment
	a owl:Class ;
	rdfs:subClassOf gist:TemporalRelation ;
	skos:definition "A temporal object expressing a relationship between some resource and a status it is assigned, used to add datetimes, notes, assigner, and other data."@en ;
	skos:prefLabel "Status Assignment"@en ;
	skos:scopeNote "Status assignments will have an actual start datetime, as well as an actual end datetime if there is a subsequent assignment of a different value in the same taxonomy (e.g., from EntityActiveStatus_active to EntityActiveStatus_inactive). The end date of one will be the start date of the next one. Consistency in both precision (use of datetime rather than date) and start/end vs single dates is recommended for ease of querying, even if only date precision is required in specific cases."@en ;
	.

tolo:TeacherStudentRelationship
	a owl:Class ;
	owl:equivalentClass [
		a owl:Class ;
		owl:intersectionOf (
			gist:TemporalRelation
			[
				a owl:Restriction ;
				owl:onProperty gist:hasGiver ;
				owl:someValuesFrom tolo:Person ;
			]
			[
				a owl:Restriction ;
				owl:onProperty gist:hasRecipient ;
				owl:someValuesFrom tolo:Person ;
			]
			[
				a owl:Restriction ;
				owl:onProperty gist:conformsTo ;
				owl:someValuesFrom tolo:Tradition ;
			]
		) ;
	] ;
	skos:definition "A time-delimited relationship between a teacher and a student."@en ;
	skos:prefLabel "Teacher-Student Relationship"@en ;
	.

tolo:Tradition
	a owl:Class ;
	rdfs:subClassOf gist:Intention ;
	skos:definition "An instance of Tibetan religion that identifies as a cohesive group with distinct modes of ritual and learning, as well as associated institutions such as monasteries."@en ;
	skos:example "The major schools and subschools of Tibetan Buddhism as well as Bon."@en ;
	skos:prefLabel
		"Tradition"@en ,
		"chos lugs"@bo-x-ewts
		;
	.

tolo:Vocation
	a owl:Class ;
	owl:equivalentClass [
		a owl:Class ;
		owl:intersectionOf (
			gist:TemporalRelation
			[
				a owl:Restriction ;
				owl:onProperty gist:hasParticipant ;
				owl:someValuesFrom tolo:Person ;
			]
			[
				a owl:Restriction ;
				owl:onProperty gist:isCategorizedBy ;
				owl:someValuesFrom tolo:Role ;
			]
		) ;
	] ;
	skos:definition "Relates a person to a role played by that person, possibly for a defined period of time."@en ;
	skos:prefLabel "Vocation"@en ;
	.

tolo:Website
	a owl:Class ;
	rdfs:subClassOf
		gist:IntellectualProperty ,
		gist:Network
		;
	skos:definition "A network of one or more web pages and related content that is identified by a common domain name and published on at least one web server."@en ;
	skos:example "Lotsawa House, Rubin Museum of Art"@en ;
	skos:prefLabel "Website"@en ;
	.

tolo:WifeStatus
	a owl:Class ;
	rdfs:subClassOf
		gist:Category ,
		[
			a owl:Restriction ;
			owl:onProperty [
				owl:inverseOf gist:isCategorizedBy ;
			] ;
			owl:allValuesFrom tolo:Marriage ;
		]
		;
	skos:definition "Indicates whether a marriage relationship has a junior or senior wife."@en ;
	skos:example "Junior, senior"@en ;
	skos:prefLabel "Wife Status"@en ;
	.

tolo:WorkType
	a owl:Class ;
	rdfs:subClassOf gist:Category ;
	skos:definition "A category of work or intellectual property based on materials, form, or content."@en ;
	skos:example "Painting, sculpture, rock carving, letter, initiation card."@en ;
	skos:prefLabel "Work Type"@en ;
	.

tolo:actualYear
	a owl:DatatypeProperty ;
	rdfs:subPropertyOf tolo:year ;
	skos:definition "The year in which something existed or took place."@en ;
	skos:example "Gyergom Tsultime Sengge was born in 1144 and died in 1204."@en ;
	skos:prefLabel "actual year"@en ;
	.

tolo:alternateEndYear
	a owl:DatatypeProperty ;
	rdfs:subPropertyOf tolo:year ;
	skos:definition "The year in which something is proposed to have ended."@en ;
	skos:prefLabel "alternate end year"@en ;
	.

tolo:alternateStartYear
	a owl:DatatypeProperty ;
	rdfs:subPropertyOf tolo:year ;
	skos:definition "The year in which something is proposed to have started."@en ;
	skos:prefLabel "alternate start year"@en ;
	.

tolo:alternateYear
	a owl:DatatypeProperty ;
	rdfs:subPropertyOf tolo:year ;
	skos:definition "The year in which something is proposed to have existed or taken place."@en ;
	skos:example "According to one source, Kunkyong Lingpa was born in 1396, while according to another source his birth year was 1408. No indication of greater or less likelihood of the two possibilities is implied."@en ;
	skos:prefLabel "alternate year"@en ;
	skos:scopeNote "Differs from tolo:approximateYear, which specifies a single year but is intended to be inexact. In this case, various scholars have proposed different years. If there is an alternate year, there is no actual year; rather, both proposed dates are asserted as alternates."@en ;
	.

tolo:approximateEndYear
	a owl:DatatypeProperty ;
	rdfs:subPropertyOf tolo:year ;
	skos:definition "The approximate year in which an event or relationship, such as a marriage, ended."@en ;
	skos:prefLabel "approximate end year"@en ;
	.

tolo:approximateStartYear
	a owl:DatatypeProperty ;
	rdfs:subPropertyOf tolo:year ;
	skos:definition "The approximate year in which an event or relationship, such as a marriage, began."@en ;
	skos:prefLabel "approximate start year"@en ;
	.

tolo:approximateYear
	a owl:DatatypeProperty ;
	rdfs:subPropertyOf tolo:year ;
	skos:definition "The approximate year in which something existed or took place."@en ;
	skos:example "The birth event of Lhagyari Namgyel Gyatso took place in approximately 1927."@en ;
	skos:prefLabel "approximate year"@en ;
	skos:scopeNote "Differs from tolo:alternateYear, which is used when there is more than one proposed year. In this case, only one year is asserted, but it is intended to be inexact, thus encompassing some number of years before and/or after."@en ;
	.

tolo:creationDate
	a owl:DatatypeProperty ;
	rdfs:subClassOf gist:atDateTime ;
	skos:definition "The date something was created, with day precision."@en ;
	skos:example "Date a photograph was taken."@en ;
	skos:prefLabel "creation date"@en ;
	skos:scopeNote "Differs from the timestamp when metadata for an image or other resource was entered into the database."@en ;
	gist:domainIncludes
		gist:Content ,
		gist:IntellectualProperty
		;
	.

tolo:credit
	a owl:DatatypeProperty ;
	rdfs:domain tolo:Image ;
	rdfs:range xsd:string ;
	skos:definition "A note acknowledging the source of an image."@en ;
	skos:prefLabel "credit"@en ;
	skos:scopeNote "Note that the credit applies to the image file, not the work of art it depicts."@en ;
	.

tolo:depicts
	a owl:ObjectProperty ;
	skos:definition "Relates an image or work of art such as a painting or sculpture to an object it represents."@en ;
	skos:example "The painting identified as HAR 65789 depicts Sachen Kunga Nyingpo; the ivory sculpture identified as HAR 65232 depicts Lhachok Sengge."@en ;
	skos:prefLabel "depicts"@en ;
	skos:scopeNote
		"Image files as well as the works themselves can serve as the subject of this property. E.g., a specific JPG file depicts the HAR 65789 painting; that painting depicts Sachen Kunga Nyingpo. Indirectly we can say that the file depicts the person, though it is not currently clear that the relationship is always transitive."@en ,
		"The object depicted does not have to be a concrete, physical thing; it could be an abstract concept, or an artwork may depict nothing."@en ,
		"This property typically applies to visual representation, as opposed to gist:isAbout, which applies to textual description or representation."@en
		;
	gist:domainIncludes
		gist:FormattedContent ,
		gist:IntellectualProperty
		;
	.

tolo:existsDuring
	a owl:ObjectProperty ;
	skos:definition "Relates an entity to an event, time period, or other temporal object during which it does or did exist."@en ;
	skos:example "Trimalo lived during the 7th century; Dorje Sherab lived during the 12th and 13th centuries."@en ;
	skos:prefLabel "exists during"@en ;
	skos:scopeNote "The subject of tolo:existsDuring is a non-temporal resource. The property contrasts with tolo:occursDuring, which relates a temporal resource (event, temporal relation, time interval) to a containing temporal resource."@en ;
	gist:domainIncludes
		gist:LivingThing ,
		gist:PhysicalIdentifiableItem ,
		tolo:Person
		;
	gist:rangeIncludes
		gist:Event ,
		gist:TemporalRelation ,
		gist:TimeInterval ,
		tolo:HistoricalPeriod
		;
	.

tolo:firstName
	a owl:DatatypeProperty ;
	rdfs:subClassOf gist:name ;
	rdfs:domain tolo:Person ;
	skos:definition "The first name of a person."@en ;
	skos:prefLabel "first name"@en ;
	skos:scopeNote "Neutral as to whether the first name is the given or family name."@en ;
	.

tolo:fullName
	a owl:DatatypeProperty ;
	rdfs:subClassOf gist:name ;
	skos:definition "The full name of a person."@en ;
	skos:prefLabel "full name"@en ;
	skos:scopeNote "Generally used with persons but conceivably could have other uses."@en ;
	gist:domainIncludes tolo:Person ;
	.

tolo:hasBibliographicSource
	a owl:ObjectProperty ;
	rdfs:domain gist:ContentExpression ;
	rdfs:range gist:ContentExpression ;
	skos:definition "Relates a piece of content to a source of information used to create that content."@en ;
	skos:editorialNote "Not currently in use, since bibliographic sources are not yet being modeled as entities, as are place sources. Currently we use tolo:hasSourceStatement to link the bio to a formatted content object. This property will be used in future to relate biographies to their source entities."@en ;
	skos:prefLabel "has source"@en ;
	skos:scopeNote "Written sources are used to create content about persons (i.e., biographies) and places on the Treasury of Lives website and cited with this content."@en ;
	.

tolo:hasCreator
	a owl:ObjectProperty ;
	skos:definition "Relates a man-made object to a person who created it."@en ;
	skos:prefLabel "has creator"@en ;
	gist:domainIncludes
		gist:Content ,
		gist:IntellectualProperty
		;
	.

tolo:hasFounder
	a owl:ObjectProperty ;
	rdfs:range tolo:Person ;
	skos:definition "Relates something, such as a tradition, to its founder."@en ;
	skos:prefLabel "hasFounder"@en ;
	skos:scopeNote "Currently we do not have dates on tradition foundings, so there is no need for the complexity of a founding object. If we get dates in the future, remove this predicate and use the founding structure as for monasteries."@en ;
	gist:domainIncludes tolo:Tradition ;
	.

tolo:hasHusband
	a owl:ObjectProperty ;
	rdfs:subPropertyOf tolo:hasSpouse ;
	rdfs:domain tolo:Marriage ;
	rdfs:range tolo:Person ;
	skos:definition "Relates a marriage relationship to the husband."@en ;
	skos:prefLabel "has husband"@en ;
	skos:scopeNote "Use bdo:hasHusband to assert a direct relationship from wife to husband."@en ;
	.

tolo:hasPreincarnation
	a owl:ObjectProperty ;
	rdfs:domain tolo:Person ;
	rdfs:range tolo:Person ;
	skos:definition "The relationship of a person to a non-living person or mythical figure who is named as a previous emanation."@en ;
	skos:example "Jamgong Kongtrul had the preincarnation Tarnatha."@en ;
	skos:prefLabel "has preincarnation"@en ;
	skos:scopeNote "Not part of the ordered members of incarnation lines and thus represented as a direct relationship between two people. We do not currently have the data to populate this property."@en ;
	.

tolo:hasSourceStatement
	a owl:ObjectProperty ;
	rdfs:domain gist:FormattedContent ;
	rdfs:range gist:FormattedContent ;
	skos:definition "Relates a piece of content, such as a biography, to a statement of sources used to create it."@en ;
	skos:prefLabel "has source statement"@en ;
	.

tolo:hasSpouse
	a owl:ObjectProperty ;
	rdfs:subPropertyOf gist:hasParty ;
	rdfs:domain tolo:Marriage ;
	rdfs:range tolo:Person ;
	skos:definition "Relates a marriage relationship to one of the spouses."@en ;
	skos:prefLabel "has spouse"@en ;
	skos:scopeNote "Use bdo:hasHusband or bdo:hasWife to assert a direct relationship from wife to husband or husband to wife, respectively."@en ;
	.

tolo:hasSummary
	a owl:ObjectProperty ;
	rdfs:domain gist:FormattedContent ;
	rdfs:range gist:FormattedContent ;
	skos:definition "Relates a piece of content, such as a biography, to a brief statement or restatement of its main points."@en ;
	skos:prefLabel "has summary"@en ;
	.

tolo:hasWife
	a owl:ObjectProperty ;
	rdfs:subPropertyOf tolo:hasSpouse ;
	rdfs:domain tolo:Marriage ;
	rdfs:range tolo:Person ;
	skos:definition "Relates a marriage relationship to the wife."@en ;
	skos:prefLabel "has wife"@en ;
	skos:scopeNote "Use bdo:hasWife to assert a direct relationship from husband to wife."@en ;
	.

tolo:isAssignmentOf
	a owl:ObjectProperty ;
	skos:definition "Relates an assignment to the resource it assigns."@en ;
	skos:example "Assignment of a wife status to a marriage."@en ;
	skos:prefLabel "is assignment of"@en ;
	gist:domainIncludes tolo:StatusAssignment ;
	gist:rangeIncludes gist:Category ;
	.

tolo:isAssignmentTo
	a owl:ObjectProperty ;
	skos:definition "Relates an assignment to the thing the resource is assigned to."@en ;
	skos:example "Assignment of a wife status to a marriage."@en ;
	skos:prefLabel "is assignment to"@en ;
	gist:domainIncludes tolo:StatusAssignment ;
	.

tolo:isBranchOf
	a owl:ObjectProperty ;
	rdfs:subPropertyOf gist:isPartOf ;
	skos:definition "Relates a monastery to a larger monastery in another location of which it is a subsidiary or affiliate. The two monasteries share administrative and/or curricular materials."@en ;
	skos:example "The Adzom Gar monastery is a branch of the Katok monastery."@en ;
	skos:prefLabel "is branch of"@en ;
	skos:scopeNote "Differs from the tolo:isDerivedFrom relationship between monasteries, which is used for monasteries in exile."@en ;
	gist:domainIncludes tolo:Monastery ;
	gist:rangeIncludes tolo:Monastery ;
	.

tolo:isDerivedFrom
	a owl:ObjectProperty ;
	skos:definition "Relates a resource to another it is derived from. This could be in the context of a hierarchy, as for traditions and incarnation lineages, or not, as for monasteries in exile."@en ;
	skos:example "The Barom Kagyu tradition is derived from, or branches off of, the Marpa Kagyu tradition; the Kalu Rinpoche incarnation lineage is derived from the Jamgon Kongtrul lineage; the Ganden and Ganden Tritok Khang monasteries in India are derived from the Ganden monastery in Tibet."@en ;
	skos:prefLabel "is derived from"@en ;
	gist:domainIncludes
		tolo:IncarnationLineage ,
		tolo:Monastery ,
		tolo:Tradition
		;
	gist:rangeIncludes
		tolo:IncarnationLineage ,
		tolo:Monastery ,
		tolo:Tradition
		;
	.

tolo:isSponsoredBy
	a owl:ObjectProperty ;
	rdfs:range tolo:Sponsor ;
	skos:definition "Relates a biography or other object to a person or organization that has funded its development."@en ;
	skos:prefLabel "is sponsored by"@en ;
	gist:domainIncludes tolo:Biography ;
	.

tolo:lastName
	a owl:DatatypeProperty ;
	rdfs:subClassOf gist:name ;
	rdfs:domain tolo:Person ;
	skos:definition "The last name of a person."@en ;
	skos:prefLabel "last name"@en ;
	skos:scopeNote "Neutral as to whether the last name is the given or family name."@en ;
	.

tolo:nameVariant
	a owl:DatatypeProperty ;
	rdfs:subPropertyOf gist:name ;
	skos:altLabel "alternate name"@en ;
	skos:definition "An alternate name for a person."@en ;
	skos:example "Gyergom Nyipa (Wylie gyer sgom gnyis pa) is an alternate name for Gyergom Tsultrim Sengge (Wylie gyer sgom tshul khrims seng+ge)."@en ;
	skos:prefLabel "name variant"@en ;
	skos:scopeNote "The primary/alternate distinction may be source- or system-dependent. Other systems or sources may prefer a name different from Treasury of Lives' primary name."@en ;
	.

tolo:occursBy
	a
		owl:ObjectProperty ,
		owl:TransitiveProperty
		;
	skos:definition "Relates a temporal resource to another that provides an upper boundary to the time of its occurrence."@en ;
	skos:example "The exact founding year or century of Pabongkha Hermitage is unknown, but it occurred by at least the 7th century."@en ;
	skos:prefLabel "occurs by"@en ;
	skos:scopeNote "Less precise than tolo:occursDuring."@en ;
	gist:domainIncludes
		gist:Event ,
		gist:TemporalRelation
		;
	gist:rangeIncludes gist:TimeInterval ;
	.

tolo:occursDuring
	a
		owl:ObjectProperty ,
		owl:TransitiveProperty
		;
	skos:definition "Relates a temporal resource (event, time interval, or temporal relation) to another that temporally contains it."@en ;
	skos:example "The birth of Gyergom Tsultrim Sengge occurred during the 12th century; the exact year of the founding of Nyima Tang Monastery is unknown, but it occurred sometime during the 7th century."@en ;
	skos:prefLabel "occurs during"@en ;
	skos:scopeNote "Used when a more precise value, such as year, is unknown or uncertain."@en ;
	gist:domainIncludes
		gist:Event ,
		gist:TemporalRelation ,
		gist:TimeInterval
		;
	gist:rangeIncludes
		gist:Event ,
		gist:TemporalRelation ,
		gist:TimeInterval
		;
	.

tolo:ordinal
	a owl:DatatypeProperty ;
	rdfs:range xsd:integer ;
	skos:definition "An integer used to designate position in a lineage."@en ;
	skos:example "The First Dalai Lama"@en ;
	skos:prefLabel "ordinal"@en ;
	skos:scopeNote
		"Incarnation ordinals reflect the accepted convention of the position of a given individual in the sequence of lives. These occasionally, though rarely, differ from the incarnation sequence due to contested numbering strategies or from the line's originating individual not being counted as the 'first.' An example of the first variant would be the Panchen Lama incarnation line, which has two ordinal values based on differing systems of which individual counts as the First Panchen Lama. In this instance, the actual incarnation sequence is the same in both systems, but lines up with the ordinals in one system and differs in the other. An example of the other variant would be the First Shechen Kongtrul, who is the second member of an incarnation sequence that begins with Jamgon Kongtrul."@en ,
		"This value is stored as an integer value and converted to an ordinal string for display purposes. This provides more flexibility than storing as an ordinal string."@en
		;
	.

tolo:pageNumbers
	a owl:DatatypeProperty ;
	rdfs:range xsd:string ;
	skos:definition "Page numbers used to identify a part of a content object."@en ;
	skos:prefLabel "page numbers"@en ;
	gist:domainIncludes gist:Content ;
	.

tolo:primaryName
	a owl:DatatypeProperty ;
	rdfs:subPropertyOf gist:name ;
	owl:deprecated "true"^^xsd:boolean ;
	skos:definition "The primary or preferred name of a person or other resource."@en ;
	skos:example "Gyergom Tsultrim Sengge is the primary name of the individual called Gyergom Nyipa by the Library of Congress."@en ;
	skos:prefLabel "primary name"@en ;
	skos:scopeNote
		"The primary/alternate distinction may be source- or system-dependent. Other systems or sources may a different name primary."@en ,
		"The same name may be rendered differently in different transliteration or transcription systems. For example, ToL displays a primary name in both its own and the Extended Wylie systems and possibly others."@en
		;
	.

tolo:publicationDate
	a owl:DatatypeProperty ;
	rdfs:subClassOf gist:atDateTime ;
	skos:definition "The date a biography was published, with day precision."@en ;
	skos:prefLabel "publication date"@en ;
	skos:scopeNote "Differs from the timestamp when the biography metadata was entered into the database (tolo:createDateTime)."@en ;
	.

tolo:residesIn
	a owl:ObjectProperty ;
	rdfs:range gist:Place ;
	skos:definition "Relates something to the place where it lives or exists."@en ;
	skos:prefLabel "resides in"@en ;
	.

tolo:title
	a owl:DatatypeProperty ;
	rdfs:range rdf:langString ;
	skos:definition "An appellation of dignity, honor, distinction, or preeminence attached to a person or family by virtue of rank, office, precedent, privilege, attainment, or lands."@en ;
	skos:prefLabel "title"@en ;
	.

tolo:updateDate
	a owl:DatatypeProperty ;
	rdfs:subClassOf gist:atDateTime ;
	skos:definition "The date a biography was updated, with day precision."@en ;
	skos:prefLabel "update date"@en ;
	skos:scopeNote "Differs from the timestamp when the biography metadata was last modified in the database (tolo:lastModifiedDateTime)."@en ;
	.

tolo:url
	a owl:DatatypeProperty ;
	rdfs:range xsd:anyURI ;
	skos:definition "A URL."@en ;
	skos:prefLabel "url"@en ;
	.

tolo:year
	a owl:DatatypeProperty ;
	rdfs:subPropertyOf gist:atDateTime ;
	skos:definition "The year in which something existed or took place, neutral as to start/end and planned/actual/approximate/alternate."@en ;
	skos:example "Gyergom Tsultime Sengge's birth took place in 1144."@en ;
	skos:prefLabel "year"@en ;
	skos:scopeNote "This is a covering concept for approximate, actual, and alternate years (as for births, deaths, and foundings) and will generally not be used directly."@en ;
	.

