# imports: https://w3id.org/semanticarts/ontology/gistCore13.0.0
# imports: https://w3id.org/treasuryoflives/ontology/tolCoreX.x.x

@prefix gist: <https://w3id.org/semanticarts/ns/ontology/gist/> .
@prefix owl: <http://www.w3.org/2002/07/owl#> .
@prefix rdf: <http://www.w3.org/1999/02/22-rdf-syntax-ns#> .
@prefix rdfs: <http://www.w3.org/2000/01/rdf-schema#> .
@prefix skos: <http://www.w3.org/2004/02/skos/core#> .
@prefix tolo: <https://w3id.org/treasuryoflives/ns/ontology/tol/> .
@prefix xsd: <http://www.w3.org/2001/XMLSchema#> .

<https://w3id.org/treasuryoflives/ontology/tolDisplay>
	a owl:Ontology ;
	owl:imports
		<https://w3id.org/semanticarts/ontology/gistCore13.0.0> ,
		<https://w3id.org/treasuryoflives/ontology/tolCoreX.x.x>
		;
	owl:versionIRI <https://w3id.org/treasuryoflives/ontology/tolDisplayX.x.x> ;
	skos:definition "Defines concepts to support Treasury of Lives website display."@en ;
	skos:prefLabel "Treasury of Lives Display Ontology"@en ;
	gist:license "TBD"@en ;
	.

tolo:MapRegionType
	a owl:Class ;
	rdfs:subClassOf gist:Category ;
	skos:definition "TBD"@en ;
	skos:prefLabel "Map Region Type"@en ;
	.

tolo:MappingPriority
	a owl:Class ;
	owl:equivalentClass [
		a owl:Class ;
		owl:intersectionOf (
			gist:Category
			[
				a owl:Restriction ;
				owl:onProperty tolo:level ;
				owl:someValuesFrom xsd:integer ;
			]
			[
				a owl:Restriction ;
				owl:onProperty tolo:minZoomLevel ;
				owl:someValuesFrom xsd:integer ;
			]
		) ;
	] ;
	skos:definition "A category specifying mapping priority level and minimum zoom level."@en ;
	skos:prefLabel "Mapping Priority"@en ;
	.

tolo:RegionType
	a owl:Class ;
	rdfs:subClassOf gist:Category ;
	skos:definition "TBD"@en ;
	skos:prefLabel "Region Type"@en ;
	.

tolo:caption
	a owl:DatatypeProperty ;
	rdfs:domain gist:FormattedContent ;
	rdfs:range xsd:string ;
	skos:definition "A short piece of text under an image that describes or explains it."@en ;
	skos:prefLabel "caption"@en ;
	.

tolo:coordinates
	a owl:DatatypeProperty ;
	rdfs:range xsd:string ;
	skos:definition "Coordinates for map display. This is an unparsed, comma-delimited series of four coordinates that is used as input to a JavaScript program."@en ;
	skos:prefLabel "coordinates"@en ;
	.

tolo:displayLabel
	a owl:AnnotationProperty ;
	skos:definition "The name or label of a person or other resource used for display purposes."@en ;
	skos:example "The display label 'The Fifth Chakri Nyidrak, Tenzin Trinle Wangchuk' combines ordinal, title, and name of Tenzin Trinle Wangchuk."@en ;
	skos:prefLabel "display label"@en ;
	.

tolo:displayOrder
	a owl:AnnotationProperty ;
	skos:definition "Indicates display order in a list of values."@en ;
	skos:example "Used to order a biography author list when there are multiple authors."@en ;
	skos:prefLabel "display order"@en ;
	.

tolo:displayText
	a owl:AnnotationProperty ;
	skos:definition "Display text for a resource, often formatted content such as HTML."@en ;
	skos:example "Ahmad, Zahiruddin. 1999.&nbsp;<em>Sangs-rGyas rGya-mTSHo. Life of the Fifth Dalai Lama</em>. New Delhi: International Academy of Indian Culture &amp; Aditya Prakashan.</p>."@en ;
	skos:prefLabel "display text"@en ;
	.

tolo:hasMappingPriority
	a owl:AnnotationProperty ;
	rdfs:range tolo:MappingPriority ;
	skos:definition "Relates a place to its priority level in map displays."@en ;
	skos:prefLabel "has mapping priority"@en ;
	gist:domainIncludes
		gist:Place ,
		tolo:Institution
		;
	.

tolo:isRenderedAt
	a owl:AnnotationProperty ;
	skos:definition "Relates a resource to the location, such as a geo-point on a map, where it is rendered or displayed."@en ;
	skos:example "Wutai Shan Mountain is rendered at the geo-point at latitude 39.0792 and longitude 113.5647."@en ;
	skos:prefLabel "is rendered at"@en ;
	skos:scopeNote "Considered a display property because in the real world places are not located at single geo-points."@en ;
	.

tolo:maxZoomLevel
	a owl:AnnotationProperty ;
	rdfs:range xsd:integer ;
	skos:definition "Relates a map region to its maximum zoom level."@en ;
	skos:preflabel "maximum zoom level"@en ;
	.

tolo:minZoomLevel
	a owl:AnnotationProperty ;
	rdfs:range xsd:integer ;
	skos:definition "Relates a mapping priority or map region to its minimum zoom level."@en ;
	skos:preflabel "minimum zoom level"@en ;
	.

tolo:zoomLevelOnClick
	a owl:AnnotationProperty ;
	rdfs:range xsd:integer ;
	skos:definition "Relates a map region to its zoom level when clicked."@en ;
	skos:editorialNote "Is it correct that this is the default level?"@en ;
	skos:preflabel "zoom level on click"@en ;
	.

