# imports: http://purl.bdrc.io/ontology/core
# imports: https://w3id.org/semanticarts/ontology/gistCore13.0.0

@prefix bdo: <http://purl.bdrc.io/ontology/core/> .
@prefix gist: <https://w3id.org/semanticarts/ns/ontology/gist/> .
@prefix owl: <http://www.w3.org/2002/07/owl#> .
@prefix rdf: <http://www.w3.org/1999/02/22-rdf-syntax-ns#> .
@prefix rdfs: <http://www.w3.org/2000/01/rdf-schema#> .
@prefix skos: <http://www.w3.org/2004/02/skos/core#> .
@prefix told: <https://w3id.org/treasuryoflives/ns/data/tol/> .
@prefix tolo: <https://w3id.org/treasuryoflives/ns/ontology/tol/> .
@prefix tolx: <https://w3id.org/treasuryoflives/ns/taxonomy/tol/> .
@prefix wiki: <https://www.wikidata.org/wiki/> .
@prefix xsd: <http://www.w3.org/2001/XMLSchema#> .

<https://w3id.org/treasuryoflives/ontology/tolFamilyRelationshipsX.x.x>
	a owl:Ontology ;
	owl:imports
		<http://purl.bdrc.io/ontology/core> ,
		<https://w3id.org/semanticarts/ontology/gistCore13.0.0>
		;
	owl:versionIRI <https://w3id.org/treasuryoflives/ontology/tolFamilyRelationshipsX.x.x> ;
	skos:definition "An add-on ontology that defines fine-grained family relationships. It is not currently used in Treasury of Lives data and thus not part of the current standard set of ToL ontologies. Properties are based on Buda Core Ontology (BDO), which is imported."@en ;
	skos:prefLabel "Treasury of Lives Family Relationships Ontology"@en ;
	gist:license "https://creativecommons.org/licenses/by/4.0/"^^xsd:anyURI ;
	.

tolo:hasFraternalNephew
	a owl:ObjectProperty ;
	rdfs:subPropertyOf bdo:hasNephew ;
	owl:propertyChainAxiom (
		bdo:hasBrother
		bdo:hasSon
	) ;
	skos:definition "Relates a person to the son of his/her brother."@en ;
	skos:prefLabel "has fraternal nephew"@en ;
	skos:scopeNote
		"We do not currently distinguish biological, adoptive, half, and step relationships."@en ,
		"While a nephew can be related through either a sibling or sibling-in-law, a fraternal nephew is always related through a brother."@en
		;
	.

tolo:hasFraternalNiece
	a owl:ObjectProperty ;
	rdfs:subPropertyOf bdo:hasNiece ;
	owl:propertyChainAxiom (
		bdo:hasBrother
		bdo:hasSon
	) ;
	skos:definition "Relates a person to the daughter of his/her brother."@en ;
	skos:prefLabel "has fraternal niece"@en ;
	skos:scopeNote
		"We do not currently distinguish biological, adoptive, half, and step relationships."@en ,
		"While a niece can be related through either a sibling or sibling-in-law, a fraternal niece is always related through a brother."@en
		;
	.

tolo:hasMaternalCousin
	a owl:ObjectProperty ;
	rdfs:subPropertyOf bdo:hasCousin ;
	skos:definition "Relates a person to his/her cousin on the mother's side."@en ;
	skos:prefLabel "has maternal cousin"@en ;
	skos:scopeNote "We do not currently distinguish biological, adoptive, half, and step relationships."@en ;
	.

tolo:hasMaternalGrandfather
	a owl:ObjectProperty ;
	rdfs:subPropertyOf
		bdo:hasGrandfather ,
		tolo:hasMaternalGrandparent
		;
	owl:propertyChainAxiom (
		bdo:hasMother
		bdo:hasFather
	) ;
	skos:definition "Relates a person to his/her mother's father."@en ;
	skos:prefLabel "has maternal grandfather"@en ;
	skos:scopeNote "We do not currently distinguish biological, adoptive, half, and step relationships."@en ;
	.

tolo:hasMaternalGrandmother
	a owl:ObjectProperty ;
	rdfs:subPropertyOf
		bdo:hasGrandmother ,
		tolo:hasMaternalGrandparent
		;
	owl:propertyChainAxiom (
		bdo:hasMother
		bdo:hasMother
	) ;
	skos:definition "Relates a person to his/her mother's mother."@en ;
	skos:prefLabel "has maternal grandmother"@en ;
	skos:scopeNote "We do not currently distinguish biological, adoptive, half, and step relationships."@en ;
	.

tolo:hasMaternalGrandparent
	a owl:ObjectProperty ;
	rdfs:subPropertyOf bdo:hasGrandParent ;
	owl:propertyChainAxiom (
		bdo:hasMother
		bdo:hasParent
	) ;
	skos:definition "Relates a person to his/her mother's parent."@en ;
	skos:prefLabel "has maternal grandmother"@en ;
	skos:scopeNote "We do not currently distinguish biological, adoptive, half, and step relationships."@en ;
	.

tolo:hasPaternalCousin
	a owl:ObjectProperty ;
	rdfs:subPropertyOf bdo:hasCousin ;
	skos:definition "Relates a person to his/her cousin on the father's side."@en ;
	skos:prefLabel "has paternal cousin"@en ;
	skos:scopeNote "We do not currently distinguish biological, adoptive, half, and step relationships."@en ;
	.

tolo:hasPaternalGrandfather
	a owl:ObjectProperty ;
	rdfs:subPropertyOf
		bdo:hasGrandfather ,
		tolo:hasPaternalGrandparent
		;
	owl:propertyChainAxiom (
		bdo:hasFather
		bdo:hasFather
	) ;
	skos:definition "Relates a person to his/her father's father."@en ;
	skos:prefLabel "has paternal grandfather"@en ;
	skos:scopeNote "We do not currently distinguish biological, adoptive, half, and step relationships."@en ;
	.

tolo:hasPaternalGrandmother
	a owl:ObjectProperty ;
	rdfs:subPropertyOf
		bdo:hasGrandmother ,
		tolo:hasPaternalGrandparent
		;
	owl:propertyChainAxiom (
		bdo:hasFather
		bdo:hasMother
	) ;
	skos:definition "Relates a person to his/her father's mother."@en ;
	skos:prefLabel "has paternal grandmother"@en ;
	skos:scopeNote "We do not currently distinguish biological, adoptive, half, and step relationships."@en ;
	.

tolo:hasPaternalGrandparent
	a owl:ObjectProperty ;
	rdfs:subPropertyOf bdo:hasGrandParent ;
	owl:propertyChainAxiom (
		bdo:hasFather
		bdo:hasParent
	) ;
	skos:definition "Relates a person to his/her fathers's parent."@en ;
	skos:prefLabel "has maternal grandmother"@en ;
	skos:scopeNote "We do not currently distinguish biological, adoptive, half, and step relationships."@en ;
	.

tolo:hasSororallNephew
	a owl:ObjectProperty ;
	rdfs:subPropertyOf bdo:hasNephew ;
	owl:propertyChainAxiom (
		bdo:hasSister
		bdo:hasSon
	) ;
	skos:definition "Relates a person to his/her sister's son."@en ;
	skos:prefLabel "has sororal nephew"@en ;
	skos:scopeNote
		"We do not currently distinguishbiological, adoptive, half, and step relationships."@en ,
		"While a nephew can be related through either a sibling or sibling-in-law, a sororal nephew is always related through a sister."@en
		;
	.

tolo:hasSororallNiece
	a owl:ObjectProperty ;
	rdfs:subPropertyOf bdo:hasNiece ;
	owl:propertyChainAxiom (
		bdo:hasSister
		bdo:hasDaughter
	) ;
	skos:definition "Relates a person to his/her sister's daughter."@en ;
	skos:prefLabel "has sororal niece"@en ;
	skos:scopeNote
		"We do not currently distinguish biological, adoptive, half, and step relationships."@en ,
		"While a niece can be related through either a sibling or sibling-in-law, a sororal nephew is always related through a sister."@en
		;
	.

