# imports: http://id.loc.gov/ontologies/bibframe-2-1-0/
# imports: http://purl.bdrc.io/ontology/core/
# imports: https://ontologies.semanticarts.com/o/gistCore10.0.0

@prefix bdo: <http://purl.bdrc.io/ontology/core/> .
@prefix bf: <http://id.loc.gov/ontologies/bibframe/> .
@prefix dct: <http://purl.org/dc/terms/> .
@prefix foaf: <http://xmlns.com/foaf/0.1/> .
@prefix gist: <https://ontologies.semanticarts.com/gist/> .
@prefix owl: <http://www.w3.org/2002/07/owl#> .
@prefix rdf: <http://www.w3.org/1999/02/22-rdf-syntax-ns#> .
@prefix rdfs: <http://www.w3.org/2000/01/rdf-schema#> .
@prefix skos: <http://www.w3.org/2004/02/skos/core#> .
@prefix tol: <https://ontologies.treasuryoflives.org/> .
@prefix vann: <http://purl.org/vocab/vann/> .
@prefix xml: <http://www.w3.org/XML/1998/namespace> .
@prefix xsd: <http://www.w3.org/2001/XMLSchema#> .

tol:core
	a owl:Ontology ;
	dct:license "TBD"^^xsd:string ;
	vann:preferredNamespacePrefix "tol"^^xsd:string ;
	owl:imports
		<http://id.loc.gov/ontologies/bibframe-2-1-0/> ,
		<http://purl.bdrc.io/ontology/core/> ,
		<https://ontologies.semanticarts.com/o/gistCore10.0.0>
		;
	skos:definition "The Treasury of Lives Core Ontology enables the description of historical and contemporary figures in the culture and religion of Tibet, Inner Asia, and the Himalaya. It is used by the Treasury of Lives born-digitial biographical collection (https://treasuryoflives.org) to publish and share its data as Linked Open Data, facilitate the consumption of external RDF, and to to enhance the narrative text with structured data."^^xsd:string ;
	skos:editoralNote
		"Add rdfs:isDefinedBy using onto-toolkit."^^xsd:string ,
		"Combining all terms into one module for now; maybe break up into separate modules later."^^xsd:string
		;
	skos:prefLabel "Treasury of Lives Core Ontology"^^xsd:string ;
	.

tol:Century
	rdfs:subClassOf tol:HistoricalPeriod ;
	skos:definition "A historical period consisting of 100 years."^^xsd:string ;
	skos:editorialNote "Not sure whether we need Century in addition to HistoricalPeriod."^^xsd:string ;
	skos:example "9th century AD."^^xsd:string ;
	skos:prefLabel "Century"^^xsd:string ;
	.

tol:FraternalNiece
	a owl:ObjectProperty ;
	rdfs:subPropertyOf bdo:hasNiece ;
	owl:propertyChainAxiom (
		bdo:hasBrother
		bdo:hasSon
	) ;
	skos:definition "Relates a person to the daughter of his/her brother."^^xsd:string ;
	skos:prefLabel "has fraternal niece"^^xsd:string ;
	skos:scopeNote
		"We do not currently distinguish biological, adoptive, half, and step relationships."^^xsd:string ,
		"While a niece can be related through either a sibling or sibling-in-law, a fraternal niece is always related through a brother."^^xsd:string
		;
	.

tol:GenealogicalGrouping
	a owl:Class ;
	rdfs:subClassOf
		gist:Collection ,
		[
			a owl:Restriction ;
			owl:onProperty gist:hasMember ;
			owl:allValuesFrom [
				owl:unionOf (
					tol:Person
					tol:GenealogicalGrouping
				) ;
			] ;
		]
		;
	skos:definition "A social unit consisting of people with a common ancestor."^^xsd:string ;
	skos:example "Nuclear family, extended family, clan, tribe."^^xsd:string ;
	skos:prefLabel "Genealogical Grouping"^^xsd:string ;
	skos:scopeNote
		"No subclasses, such as family and clan, are defined because the distinctions are not clear-cut. Instead, we use partitive relationships to describe the relationships between different groupings."^^xsd:string ,
		"This class encompasses successively larger and more inclusive genealogical groupings, such as family and clan. A person is said to be a member of a genealogical grouping, and a smaller genealogical grouping is a member of a larger one."^^xsd:string
		;
	.

tol:HistoricalPeriod
	rdfs:subClassOf
		gist:Category ,
		[
			a owl:Restriction ;
			owl:onProperty tol:start ;
			owl:cardinality "1"^^xsd:nonNegativeInteger ;
		]
		;
	rdfs:seeAlso bdo:Era ;
	skos:definition "A time interval having some historical signifance or distinguishing features."^^xsd:string ;
	skos:example "19th century, the 1920s."^^xsd:string ;
	skos:prefLabel "Historical Period"^^xsd:string ;
	skos:scopeNote
		"A historical period has a start date in the past, but may not yet have an end date."^^xsd:string ,
		"Currently only centuries are defined in the taxonomy."^^xsd:string
		;
	.

tol:Lineage
	a owl:Class ;
	rdfs:subClassOf
		gist:OrderedCollection ,
		[
			a owl:Restriction ;
			owl:onProperty gist:hasOrderedMember ;
			owl:allValuesFrom [
				a owl:Restriction ;
				owl:onProperty gist:providesOrderFor ;
				owl:allValuesFrom tol:Person ;
			] ;
		] ,
		[
			a owl:Restriction ;
			owl:onProperty tol:start ;
			owl:cardinality "1"^^xsd:nonNegativeInteger ;
		] ,
		[
			a owl:Restriction ;
			owl:onProperty gist:hasOrderedMember ;
			owl:minCardinality "2"^^xsd:nonNegativeInteger ;
		]
		;
	skos:definition "An ordered collection of persons in which a relationship or role is passed sequentially from one to the other."^^xsd:string ;
	skos:editorialNote "TODO need better definition."^^xsd:string ;
	skos:example "The succession of abbots to a monastery; the transmission of a text from teachers to students; an incarnational sequence."^^xsd:string ;
	skos:prefLabel "Lineage"^^xsd:string ;
	skos:scopeNote "The lineage itself has a start date and possibly an end date; it may have a name; and its ordered members have start and possibly end dates. In some types of lineages the members have numeric designations (e.g., 14th Dalai Lama), in others they are ordered by precedence relationships (e.g., teachers in a teaching lineage). Some but not all types of lineages are strictly ordered."^^xsd:string ;
	.

tol:Location
	a owl:Class ;
	skos:definition "A real, fictional, or imaginary place."^^xsd:string ;
	skos:prefLabel "Location"^^xsd:string ;
	skos:scopeNote "Differs from and not a subclass of gist:Place, which includings only places that do or did exist."^^xsd:string ;
	.

tol:Marriage
	a owl:Class ;
	owl:equivalentClass [
		owl:intersectionOf (
			gist:Agreement
			gist:TemporalRelation
			[
				a owl:Restriction ;
				owl:onProperty gist:hasParty ;
				owl:allValuesFrom tol:Person ;
			]
			[
				a owl:Restriction ;
				owl:onProperty gist:hasParty ;
				owl:onClass tol:Person ;
				owl:qualifiedCardinality "2"^^xsd:nonNegativeInteger ;
			]
		) ;
	] ;
	skos:definition "A culturally and often legally recognized union between two people, called spouses, that establishes rights and obligations between them."^^xsd:string ;
	skos:editorialNote "Cardinality restriction on gist:hasParty of 2 generates Protege error, so using qualified cardinality restriction instead."^^xsd:string ;
	skos:prefLabel "Marriage"^^xsd:string ;
	.

tol:Person
	a owl:Class ;
	rdfs:subClassOf
		bdo:Person ,
		foaf:Person
		;
	skos:definition "A human being, alive, dead, imaginary, or fictional."^^xsd:string ;
	skos:prefLabel "Person"^^xsd:string ;
	skos:scopeNote "Differs from and not a subclass of gist:Person, which includings only persons who do or did exist."^^xsd:string ;
	.

tol:StrictlyOrderedCollection
	a owl:Class ;
	rdfs:subClassOf gist:OrderedCollection ;
	skos:definition "An ordered collection in which no two members occupy the same position."^^xsd:string ;
	skos:editorialNote "Can we express this axiomatically?"^^xsd:string ;
	skos:preflabel "Strictly Ordered Collection"^^xsd:string ;
	.

tol:Student
	a owl:Class ;
	owl:equivalentClass [
		a owl:Class ;
		owl:intersectionOf (
			tol:Person
			[
				a owl:Restriction ;
				owl:onProperty [
					owl:inverseOf gist:hasRecipient ;
				] ;
				owl:someValuesFrom tol:TeacherStudentRelationship ;
			]
		) ;
	] ;
	skos:definition "A person who receives training in a text or practice from another person (the teacher)."^^xsd:string ;
	skos:editorialNote "Not sure if needed."^^xsd:string ;
	skos:prefLabel "Student"^^xsd:string ;
	.

tol:Teacher
	a owl:Class ;
	owl:equivalentClass [
		a owl:Class ;
		owl:intersectionOf (
			tol:Person
			[
				a owl:Restriction ;
				owl:onProperty [
					owl:inverseOf gist:hasGiver ;
				] ;
				owl:someValuesFrom tol:TeacherStudentRelationship ;
			]
		) ;
	] ;
	skos:definition "A person who transmits a text or practice to another person (the student)."^^xsd:string ;
	skos:editorialNote "Not sure if needed."^^xsd:string ;
	skos:prefLabel "Teacher"^^xsd:string ;
	.

tol:TeacherStudentRelationship
	a owl:Class ;
	owl:equivalentClass [
		a owl:Class ;
		owl:intersectionOf (
			gist:TemporalRelation
			gist:Agreement
			[
				a owl:Restriction ;
				owl:onProperty gist:hasParticipant ;
				owl:cardinality "2"^^xsd:nonNegativeInteger ;
			]
			[
				a owl:Restriction ;
				owl:onProperty gist:hasGiver ;
				owl:allValuesFrom tol:Teacher ;
			]
			[
				a owl:Restriction ;
				owl:onProperty gist:hasGiver ;
				owl:cardinality "1"^^xsd:nonNegativeInteger ;
			]
			[
				a owl:Restriction ;
				owl:onProperty gist:hasRecipient ;
				owl:allValuesFrom tol:Student ;
			]
			[
				a owl:Restriction ;
				owl:onProperty gist:hasRecipient ;
				owl:cardinality "1"^^xsd:nonNegativeInteger ;
			]
			[
				a owl:Restriction ;
				owl:onProperty gist:conformsTo ;
				owl:someValuesFrom gist:Intention ;
			]
		) ;
	] ;
	skos:definition "A time-delimited relationship between a teacher and a student."^^xsd:string ;
	skos:editorialNote
		"How to express what the Intention is? I.e., how should an intention be instantiated?"^^xsd:string ,
		"TODO Add relationship to text (bf:Text?) or Practice (subclass of gist:Behavior? - need to see examples."^^xsd:string
		;
	skos:prefLabel "Teacher-Student Relationship"^^xsd:string ;
	skos:scopeNote "A teacher-student relationshp may be, but is not necessarily, part of a teaching lineage. In some cases the teacher-student relationship is known while the lineage is not."^^xsd:string ;
	.

tol:TeachingLineage
	a owl:Class ;
	owl:disjointWith tol:IncarnationLineage ;
	owl:equivalentClass [
		a owl:Class ;
		owl:intersectionOf (
			tol:Lineage
			[
				a owl:Restriction ;
				owl:onProperty gist:hasOrderedMember ;
				owl:allValuesFrom [
					a owl:Restriction ;
					owl:onProperty gist:providesOrderFor ;
					owl:allValuesFrom tol:Teacher ;
				] ;
			]
			[
				a owl:Restriction ;
				owl:onProperty gist:hasDirectPart ;
				owl:onClass tol:TeacherStudentRelationship ;
				owl:minQualifiedCardinality "2"^^xsd:nonNegativeInteger ;
			]
			[
				a owl:Restriction ;
				owl:onProperty gist:hasOrderedMember ;
				owl:allValuesFrom [
					a owl:Restriction ;
					owl:onProperty gist:sequence ;
					owl:maxCardinality "0"^^xsd:nonNegativeInteger ;
				] ;
			]
		) ;
	] ;
	skos:definition "An ordered collection of teachers transmitting a specific text or practice to their students."^^xsd:string ;
	skos:prefLabel "Teaching Lineage"^^xsd:string ;
	skos:scopeNote "Teachers in a lineage are not designated numerically (as are, e.g., persons in an incarnation lineage), but are ordered through gist:precedesDirectly. Elements in the lineage may certainly co-occur or overlap."^^xsd:string ;
	.

tol:alternateBirthYear
	a owl:DatatypeProperty ;
	rdfs:subPropertyOf tol:birthYear ;
	skos:definition "An alternate year in which it is speculated that a person may have been born."^^xsd:string ;
	skos:prefLabel "alternate birth year"^^xsd:string ;
	skos:scopeNote "May be used with edtf:EDTF datatyped strings to allow for partial, uncertain, and approximate dates."^^xsd:string ;
	.

tol:alternateDeathYear
	a owl:DatatypeProperty ;
	rdfs:subPropertyOf tol:deathYear ;
	skos:definition "An alternate year in which it is speculated that a person may have died."^^xsd:string ;
	skos:prefLabel "alternate death year"^^xsd:string ;
	skos:scopeNote "May be used with edtf:EDTF datatyped strings to allow for partial, uncertain, and approximate dates."^^xsd:string ;
	.

tol:birthCentury
	a owl:DatatypeProperty ;
	rdfs:subPropertyOf tol:start ;
	skos:definition "The century in which a person was born."^^xsd:string ;
	skos:prefLabel "birth century"^^xsd:string ;
	skos:scopeNote
		"May be used with edtf:EDTF datatyped strings to allow for partial, uncertain, and approximate dates."^^xsd:string ,
		"This value may be asserted directly, or derived from a known birth year. It is typically provided and displayed only when the year is not known."^^xsd:string
		;
	.

tol:birthYear
	a owl:DatatypeProperty ;
	rdfs:subPropertyOf tol:start ;
	skos:definition "The year in which a person was born."^^xsd:string ;
	skos:prefLabel "birth year"^^xsd:string ;
	skos:scopeNote "May be used with edtf:EDTF datatyped strings to allow for partial, uncertain, and approximate dates."^^xsd:string ;
	.

tol:deathCentury
	a owl:DatatypeProperty ;
	rdfs:subPropertyOf tol:end ;
	skos:definition "The century in which a person died."^^xsd:string ;
	skos:prefLabel "death century"^^xsd:string ;
	skos:scopeNote
		"May be used with edtf:EDTF datatyped strings to allow for partial, uncertain, and approximate dates."^^xsd:string ,
		"This value may be asserted directly, or derived from a known death year. It is typically provided and displayed only when the year is not known."^^xsd:string
		;
	.

tol:deathYear
	a owl:DatatypeProperty ;
	rdfs:subPropertyOf tol:end ;
	skos:definition "The year in which a person died."^^xsd:string ;
	skos:prefLabel "death year"^^xsd:string ;
	skos:scopeNote
		"May be used with edtf:EDTF datatyped strings to allow for partial, uncertain, and approximate dates."^^xsd:string ,
		"This value may be asserted directly, or derived from a known birth year."^^xsd:string
		;
	.

tol:dissolutionDate
	a owl:DatatypeProperty ;
	rdfs:subPropertyOf tol:end ;
	skos:definition "The date an agreement such as marriage was ended. In the case of marriage, this refers to divorce rather than the end of a marriage by death of one of the spouses."^^xsd:string ;
	skos:editorialNote "Use if we need to distinguish divorce from death as the end of a marriage. Might make broader to include dissolution of other types of relationships."^^xsd:string ;
	skos:prefLabel "dissolution date"^^xsd:string ;
	.

tol:end
	a owl:DatatypeProperty ;
	skos:definition "The date, time, or datetime some event, relationship, or other thing ended."^^xsd:string ;
	skos:editorialNote "TODO Re-evaluate with gist 11. EDTF is not recognized by OWL processors. How much uncertainty to we really need to accommodate?"^^xsd:string ;
	skos:prefLabel "end"^^xsd:string ;
	skos:scopeNote "May be used with edtf:EDTF datatyped strings to allow for partial, uncertain, and approximate dates."^^xsd:string ;
	.

tol:harUrl
	a owl:AnnotationProperty ;
	rdfs:subPropertyOf rdfs:seeAlso ;
	rdfs:range xsd:anyURI ;
	skos:definition "The URL to the main page about this resource on the Himalayan Art Resources (HAR) site."^^xsd:string ;
	skos:prefLabel "HAR URL"^^xsd:string ;
	.

tol:hasFinalRestingPlace
	a owl:ObjectProperty ;
	rdfs:subPropertyOf gist:hasPhysicalLocation ;
	rdfs:domain tol:Person ;
	skos:definition "Relates a person to (one of) his/her final resting place(s)."^^xsd:string ;
	skos:prefLabel "has final resting place"^^xsd:string ;
	skos:scopeNote "Significant people such as the Dalai Lamas have reliquary stupas in geographic locations like temples or chapels. Sometimes there can be relics in multiple places."^^xsd:string ;
	.

tol:hasFraternalCousin
	a owl:ObjectProperty ;
	rdfs:subPropertyOf bdo:hasCousin ;
	skos:definition "Relates a person to his/her cousin on the father's side."^^xsd:string ;
	skos:prefLabel "has fraternal cousin"^^xsd:string ;
	skos:scopeNote "We do not currently distinguish biological, adoptive, half, and step relationships."^^xsd:string ;
	.

tol:hasFraternalNephew
	a owl:ObjectProperty ;
	rdfs:subPropertyOf bdo:hasNephew ;
	owl:propertyChainAxiom (
		bdo:hasBrother
		bdo:hasSon
	) ;
	skos:definition "Relates a person to the son of his/her brother."^^xsd:string ;
	skos:prefLabel "has fraternal nephew"^^xsd:string ;
	skos:scopeNote
		"We do not currently distinguish biological, adoptive, half, and step relationships."^^xsd:string ,
		"While a nephew can be related through either a sibling or sibling-in-law, a fraternal nephew is always related through a brother."^^xsd:string
		;
	.

tol:hasMaternalCousin
	a owl:ObjectProperty ;
	rdfs:subPropertyOf bdo:hasCousin ;
	skos:definition "Relates a person to his/her cousin on the mother's side."^^xsd:string ;
	skos:prefLabel "has maternal cousin"^^xsd:string ;
	skos:scopeNote "We do not currently distinguish biological, adoptive, half, and step relationships."^^xsd:string ;
	.

tol:hasMaternalGrandfather
	a owl:ObjectProperty ;
	rdfs:subPropertyOf
		bdo:hasGrandfather ,
		tol:hasMaternalGrandparent
		;
	owl:propertyChainAxiom (
		tol:hasMother
		tol:hasFather
	) ;
	skos:definition "Relates a person to his/her mother's father."^^xsd:string ;
	skos:prefLabel "has maternal grandfather"^^xsd:string ;
	skos:scopeNote "We do not currently distinguish biological, adoptive, half, and step relationships."^^xsd:string ;
	.

tol:hasMaternalGrandmother
	a owl:ObjectProperty ;
	rdfs:subPropertyOf
		bdo:hasGrandmother ,
		tol:hasMaternalGrandparent
		;
	owl:propertyChainAxiom (
		bdo:hasMother
		bdo:hasMother
	) ;
	skos:definition "Relates a person to his/her mother's mother."^^xsd:string ;
	skos:prefLabel "has maternal grandmother"^^xsd:string ;
	skos:scopeNote "We do not currently distinguish biological, adoptive, half, and step relationships."^^xsd:string ;
	.

tol:hasMaternalGrandparent
	a owl:ObjectProperty ;
	rdfs:subPropertyOf bdo:hasGrandmother ;
	owl:propertyChainAxiom (
		bdo:hasMother
		bdo:hasParent
	) ;
	skos:definition "Relates a person to his/her mother's parent."^^xsd:string ;
	skos:prefLabel "has maternal grandmother"^^xsd:string ;
	skos:scopeNote "We do not currently distinguish biological, adoptive, half, and step relationships."^^xsd:string ;
	.

tol:hasPaternalGrandfather
	a owl:ObjectProperty ;
	rdfs:subPropertyOf
		bdo:hasGrandfather ,
		tol:hasPaternalGrandparent
		;
	owl:propertyChainAxiom (
		bdo:hasFather
		bdo:hasFather
	) ;
	skos:definition "Relates a person to his/her father's father."^^xsd:string ;
	skos:prefLabel "has paternal grandfather"^^xsd:string ;
	skos:scopeNote "We do not currently distinguish biological, adoptive, half, and step relationships."^^xsd:string ;
	.

tol:hasPaternalGrandmother
	a owl:ObjectProperty ;
	rdfs:subPropertyOf
		bdo:hasGrandmother ,
		tol:hasPaternalGrandparent
		;
	owl:propertyChainAxiom (
		bdo:hasFather
		bdo:hasMother
	) ;
	skos:definition "Relates a person to his/her father's mother."^^xsd:string ;
	skos:prefLabel "has paternal grandmother"^^xsd:string ;
	skos:scopeNote "We do not currently distinguish biological, adoptive, half, and step relationships."^^xsd:string ;
	.

tol:hasPaternalGrandparent
	a owl:ObjectProperty ;
	rdfs:subPropertyOf bdo:hasGrandparent ;
	owl:propertyChainAxiom (
		bdo:hasFather
		bdo:hasParent
	) ;
	skos:definition "Relates a person to his/her fathers's parent."^^xsd:string ;
	skos:prefLabel "has maternal grandmother"^^xsd:string ;
	skos:scopeNote "We do not currently distinguish biological, adoptive, half, and step relationships."^^xsd:string ;
	.

tol:hasPlaceOfBirth
	a
		owl:ObjectProperty ,
		owl:FunctionalProperty
		;
	rdfs:subPropertyOf gist:hasPhysicalLocation ;
	rdfs:domain tol:Person ;
	skos:definition "Relates a person to his/her birthplace."^^xsd:string ;
	skos:prefLabel "has place of birth"^^xsd:string ;
	.

tol:hasPlaceOfDeath
	a
		owl:ObjectProperty ,
		owl:FunctionalProperty
		;
	rdfs:subPropertyOf gist:hasPhysicalLocation ;
	rdfs:domain tol:Person ;
	skos:definition "Relates a person to the place of his/her death."^^xsd:string ;
	skos:prefLabel "has place of death"^^xsd:string ;
	.

tol:hasSororallNephew
	a owl:ObjectProperty ;
	rdfs:subPropertyOf bdo:hasNephew ;
	owl:propertyChainAxiom (
		bdo:hasSister
		bdo:hasSon
	) ;
	skos:definition "Relates a person to his/her sister's son."^^xsd:string ;
	skos:prefLabel "has sororal nephew"^^xsd:string ;
	skos:scopeNote
		"We do not currently distinguishbiological, adoptive, half, and step relationships."^^xsd:string ,
		"While a nephew can be related through either a sibling or sibling-in-law, a sororal nephew is always related through a sister."^^xsd:string
		;
	.

tol:hasSororallNiece
	a owl:ObjectProperty ;
	rdfs:subPropertyOf bdo:hasNiece ;
	owl:propertyChainAxiom (
		bdo:hasSister
		bdo:hasDaughter
	) ;
	skos:definition "Relates a person to his/her sister's daughter."^^xsd:string ;
	skos:prefLabel "has sororal niece"^^xsd:string ;
	skos:scopeNote
		"We do not currently distinguish biological, adoptive, half, and step relationships."^^xsd:string ,
		"While a niece can be related through either a sibling or sibling-in-law, a sororal nephew is always related through a sister."^^xsd:string
		;
	.

tol:nameVariant
	a owl:DatatypeProperty ;
	rdfs:subPropertyOf gist:name ;
	skos:definition "A variant form of a person's name."^^xsd:string ;
	skos:editoralNote "TODO Explain more about how these differ from the primary name. Make sure these are different names rather than a difference encoding of the primary name."^^xsd:string ;
	skos:editorialNote "Should domain be tol:Person?"^^xsd:string ;
	skos:prefLabel "name variant"^^xsd:string ;
	.

tol:primaryName
	a owl:DatatypeProperty ;
	rdfs:subPropertyOf gist:name ;
	skos:definition "The primary form of a person's name."^^xsd:string ;
	skos:editorialNote "Should domain be tol:Person?"^^xsd:string ;
	skos:prefLabel "primary name"^^xsd:string ;
	.

tol:primaryTitle
	a owl:DatatypeProperty ;
	rdfs:subPropertyOf tol:title ;
	rdfs:domain tol:Person ;
	skos:definition "The primary form of a person's title."^^xsd:string ;
	skos:prefLabel "primary title"^^xsd:string ;
	.

tol:start
	a owl:DatatypeProperty ;
	skos:definition "The date, time, or datetime some event, relationship, or other thing started."^^xsd:string ;
	skos:editorialNote "TODO Re-evaluate with gist 11. EDTF is not recognized by OWL processors. How much uncertainty to we really need to accommodate?"^^xsd:string ;
	skos:prefLabel "start"^^xsd:string ;
	skos:scopeNote "May be used with edtf:EDTF datatyped strings to allow for partial, uncertain, and approximate dates."^^xsd:string ;
	.

tol:title
	a owl:DatatypeProperty ;
	rdfs:domain tol:Person ;
	rdfs:range xsd:string ;
	skos:definition "An appellation of dignity, honor, distinction, or preeminence attached to a person or family by virtue of rank, office, precedent, privilege, attainment, or lands."^^xsd:string ;
	skos:prefLabel "title"^^xsd:string ;
	.

tol:titleVariant
	a owl:DatatypeProperty ;
	rdfs:subPropertyOf tol:title ;
	rdfs:domain tol:Person ;
	skos:definition "A variant form of a person's title."^^xsd:string ;
	skos:editoralNote "Explain more about how these differ from the primary name."^^xsd:string ;
	skos:prefLabel "title variant"^^xsd:string ;
	.

