# imports: http://purl.bdrc.io/ontology/core/

@prefix bdo: <http://purl.bdrc.io/ontology/core/> .
@prefix dct: <http://purl.org/dc/terms/> .
@prefix dctype: <http://purl.org/dc/dcmitype/> .
@prefix foaf: <http://xmlns.com/foaf/0.1/> .
@prefix owl: <http://www.w3.org/2002/07/owl#> .
@prefix rdf: <http://www.w3.org/1999/02/22-rdf-syntax-ns#> .
@prefix rdfs: <http://www.w3.org/2000/01/rdf-schema#> .
@prefix skos: <http://www.w3.org/2004/02/skos/core#> .
@prefix tolo: <https://ontologies.treasuryoflives/tolo/> .
@prefix vann: <http://purl.org/vocab/vann/> .
@prefix xml: <http://www.w3.org/XML/1998/namespace> .
@prefix xsd: <http://www.w3.org/2001/XMLSchema#> .

tolo:core
	a owl:Ontology ;
	dct:license "TBD"^^xsd:string ;
	vann:preferredNamespacePrefix "tolo"^^xsd:string ;
	owl:imports <http://purl.bdrc.io/ontology/core/> ;
	owl:versionIRI <https://ontologies.treasuryoflives/tolo/core/1.0.0> ;
	skos:definition "The Treasury of Lives Core Ontology enables the description of historical and contemporary figures in the culture and religion of Tibet, Inner Asia, and the Himalaya. It is used by the Treasury of Lives born-digitial biographical collection (https://treasuryoflives.org) to publish and share its data as Linked Open Data, facilitate the consumption of external RDF, and to to enhance the narrative text with structured data."@en ;
	skos:editoralNote
		"Add rdfs:isDefinedBy using onto-toolkit, but keep in source files."@en ,
		"Combining all terms into one module for now; maybe break up into separate modules later."@en
		;
	skos:prefLabel "Treasury of Lives Core Ontology"@en ;
	.

tolo:Category
	a owl:Class ;
	rdfs:subClassOf
		bdo:Type ,
		skos:Concept
		;
	skos:definition "A type of concept used to categorize things."@en ;
	skos:editorialNote
		"Could use gist."@en ,
		"Use a tolo example instead of a bdo one."@en
		;
	skos:example "Male and female are categories (instances) of Gender."@en ;
	skos:prefLabel "Category"@en ;
	skos:scopeNote "A category is typically a term in a controlled vocabulary. The Category class can be subclassed for specific vocabularies; e.g., Gender is a subclass of Category."@en ;
	.

tolo:Century
	rdfs:subClassOf tolo:HistoricalPeriod ;
	skos:definition "A historical century."@en ;
	skos:example "8th century AD, 2nd century BC."@en ;
	skos:prefLabel "Century"@en ;
	.

tolo:Collection
	a owl:Class ;
	rdfs:subClassOf
		dctype:Collection ,
		[
			a owl:Restriction ;
			owl:onProperty tolo:numberOfMembers ;
			owl:cardinality "1"^^xsd:nonNegativeInteger ;
		] ,
		[
			a owl:Restriction ;
			owl:onProperty tolo:hasMember ;
			owl:minCardinality "1"^^xsd:nonNegativeInteger ;
		]
		;
	skos:definition "An identifiable grouping of instances."@en ;
	skos:example "A family or other genealogical grouping."@en ;
	skos:prefLabel "Collection"@en ;
	.

tolo:FraternalNiece
	a owl:ObjectProperty ;
	rdfs:subPropertyOf bdo:hasNiece ;
	owl:propertyChainAxiom (
		bdo:hasBrother
		bdo:hasSon
	) ;
	skos:definition "Relates a person to the daughter of his/her brother."@en ;
	skos:prefLabel "has fraternal niece"@en ;
	skos:scopeNote
		"In 1.0.0 we are not distinguishing biological, adoptive, half, and step relationships."@en ,
		"While a niece can be related through either a sibling or sibling-in-law, a fraternal niece is always related through a brother."@en
		;
	.

tolo:GenealogicalGrouping
	a owl:Class ;
	rdfs:subClassOf
		tolo:Collection ,
		[
			a owl:Restriction ;
			owl:onProperty tolo:isMemberOf ;
			owl:allValuesFrom tolo:GenealogicalGrouping ;
		] ,
		[
			a owl:Restriction ;
			owl:onProperty tolo:hasMember ;
			owl:allValuesFrom [
				owl:unionOf (
					tolo:Person
					tolo:GenealogicalGrouping
				) ;
			] ;
		]
		;
	skos:definition "A social unit consisting of people with a common ancestor."@en ;
	skos:editorialNote
		"Are there other terms included besides family and clan?"@en ,
		"Improve definition to include adoption."^^xsd:string
		;
	skos:example "Nuclear family, extended family, clan."@en ;
	skos:prefLabel "Genealogical grouping"@en ;
	skos:scopeNote
		"No subclasses, such as family and clan, are defined because the distinctions are not clear-cut. Instead, we use partitive relationships to describe the relationships between different groupings."@en ,
		"This class encompasses successively larger and more inclusive genealogical groupings, such as family and clan. A person is said to be a member of a genealogical grouping, and a smaller genealogical grouping is a member of a larger one."@en
		;
	.

tolo:HarUrl
	a owl:AnnotationProperty ;
	rdfs:subPropertyOf rdfs:seeAlso ;
	rdfs:range xsd:anyURI ;
	skos:definition "The URL to the main page about this resource on the Himalayan Art Resources (HAR) site."@en ;
	skos:prefLabel "HAR URL"@en ;
	.

tolo:HistoricalPeriod
	skos:definition "A historical period."@en ;
	skos:example "8th century AD, 2nd century BC."@en ;
	skos:prefLabel "Historical period"@en ;
	.

tolo:Location
	a owl:Class ;
	skos:definition "A real, fictional, or imaginary place."@en ;
	skos:prefLabel "Location"@en ;
	.

tolo:Marriage
	a owl:Class ;
	owl:equivalentClass [
		owl:unionOf (
			tolo:TemporalRelationship
			[
				a owl:Restriction ;
				owl:onProperty tolo:isSpouseIn ;
				owl:cardinality "2"^^xsd:nonNegativeInteger ;
			]
		) ;
	] ;
	skos:definition "TBD"@en ;
	skos:prefLabel "Marriage"@en ;
	.

tolo:OrderedCollection
	a owl:Class ;
	owl:equivalentClass [
		owl:intersectionOf (
			tolo:Collection
			[
				a owl:Restriction ;
				owl:onProperty tolo:hasOrderedMember ;
				owl:minCardinality "1"^^xsd:nonNegativeInteger ;
			]
		) ;
	] ;
	skos:definition "A collection in which resources are ordered into a sequence."@en ;
	skos:prefLabel "Ordered collection"@en ;
	skos:scopeNote "The sequence of items in an ordered collection is not fixed over time but may be reordered."@en ;
	.

tolo:OrderedMember
	owl:equivalentClass [
		owl:intersectionOf (
			[
				a owl:Restriction ;
				owl:onProperty tolo:isOrderedMemberOf ;
				owl:cardinality "1"^^xsd:nonNegativeInteger ;
			]
			[
				a owl:Restriction ;
				owl:onProperty tolo:isProxyFor ;
				owl:cardinality "1"^^xsd:nonNegativeInteger ;
			]
			[
				a owl:Restriction ;
				owl:onProperty tolo:index ;
				owl:cardinality "1"^^xsd:nonNegativeInteger ;
			]
		) ;
	] ;
	skos:definition "The proxy for a resource as it exists in a specific ordered collection. This object both represents the position of an item in an ordered collection, and carries properties that apply to an item only in the context of the collection."@en ;
	skos:example "The proxy of a teacher in a teaching lineage can indicate both the person's position in the lineage and the date the person became a member of the lineage."@en ;
	skos:prefLabel "Ordered Member"@en ;
	skos:scopeNote "An index is required but, based on the Open World Assumption, does not have to be asserted. This avoids the problem of resetting indices in case of changes to the ordered collection. Only the 'has next' pointer has to be moved."@en ;
	.

tolo:Person
	a owl:Class ;
	rdfs:subClassOf
		bdo:Person ,
		foaf:Person
		;
	skos:definition "A human being, alive, dead, imaginary, or fictional."@en ;
	skos:prefLabel "Person"@en ;
	.

tolo:TemporalRelationship
	a owl:Class ;
	rdfs:subClassOf
		[
			a owl:Restriction ;
			owl:onProperty tolo:end ;
			owl:cardinality "1"^^xsd:nonNegativeInteger ;
		] ,
		[
			a owl:Restriction ;
			owl:onProperty tolo:start ;
			owl:cardinality "1"^^xsd:nonNegativeInteger ;
		]
		;
	skos:definition "A time-delimited relationship between two or more objects."@en ;
	skos:editorialNote "Could use gist."@en ;
	skos:example
		"A marriage"@en ,
		"A teacher-student relationship."@en
		;
	skos:prefLabel "Temporal relationship"@en ;
	skos:scopeNote "This class is used to materialize a relationship in order to make other assertions about it, such as start and end datetimes, location, and so on. Start and end dates/times may not be known or specified, but the relationship is in theory time-bound."@en ;
	.

tolo:birthCentury
	a owl:DatatypeProperty ;
	rdfs:subPropertyOf tolo:start ;
	skos:definition "The century in which a person was born."@en ;
	skos:prefLabel "birth century"@en ;
	skos:scopeNote "It is expected that this value will not be directly asserted, but inferred from the value of tolo:birthYear."@en ;
	.

tolo:birthYear
	a owl:DatatypeProperty ;
	rdfs:subPropertyOf tolo:start ;
	skos:definition "The year in which a person was born."@en ;
	skos:prefLabel "birth year"@en ;
	skos:scopeNote "May be used with edtf:EDTF datatyped strings to allow for partial, uncertain, and approximate dates."@en ;
	.

tolo:categorizedBy
	a owl:DatatypeProperty ;
	rdfs:range tolo:Category ;
	skos:definition "Designates a category that is applied to the subject."@en ;
	skos:editorialNote "Could use gist."@en ;
	skos:example "Wencheng Kongjo is categorized by the bdo:Gender category bdr:GenderMale."@en ;
	skos:prefLabel "categorized by"@en ;
	.

tolo:deathYear
	a owl:DatatypeProperty ;
	rdfs:subPropertyOf tolo:end ;
	skos:definition "The year that a person died."@en ;
	skos:prefLabel "death year"@en ;
	skos:scopeNote "May be used with edtf:EDTF datatyped strings to allow for partial, uncertain, and approximate dates."@en ;
	.

tolo:description
	a owl:DatatypeProperty ;
	skos:definition "A statement about someone or something's attributes or characteristics."@en ;
	skos:example "Nyenyo Jagoshong is a Sakya monastery in Tashigang, Tsang. It was founded by Panchen Bumdrak Sumpa in 1490."@en ;
	skos:prefLabel "description"@en ;
	.

tolo:dissolutionDate
	a owl:DatatypeProperty ;
	skos:definition "The date a marriage was ended through divorce rather than the death of one of the spouses."@en ;
	skos:editorialNote "Use if we need to distinguish divorce from death as the end of a marriage. Might make broader to include dissolution of other types of relationships."@en ;
	skos:prefLabel "dissolution date"@en ;
	.

tolo:end
	a owl:DatatypeProperty ;
	skos:definition "The date, time, or datetime some event, relationship, or other thing ended."@en ;
	skos:prefLabel "end"@en ;
	skos:scopeNote "May be used with edtf:EDTF datatyped strings to allow for partial, uncertain, and approximate dates."@en ;
	.

tolo:hasFraternalCousin
	a owl:ObjectProperty ;
	rdfs:subPropertyOf bdo:hasCousin ;
	skos:definition "Relates a person to his/her cousin on the father's side."@en ;
	skos:prefLabel "has fraternal cousin"@en ;
	skos:scopeNote "In 1.0.0 we are not distinguishing biological, adoptive, half, and step relationships."@en ;
	.

tolo:hasFraternalNephew
	a owl:ObjectProperty ;
	rdfs:subPropertyOf bdo:hasNephew ;
	owl:propertyChainAxiom (
		bdo:hasBrother
		bdo:hasSon
	) ;
	skos:definition "Relates a person to the son of his/her brother."@en ;
	skos:prefLabel "has fraternal nephew"@en ;
	skos:scopeNote
		"In 1.0.0 we are not distinguishing biological, adoptive, half, and step relationships."@en ,
		"While a nephew can be related through either a sibling or sibling-in-law, a fraternal nephew is always related through a brother."@en
		;
	.

tolo:hasMaternalCousin
	a owl:ObjectProperty ;
	rdfs:subPropertyOf bdo:hasCousin ;
	skos:definition "Relates a person to his/her cousin on the mother's side."@en ;
	skos:prefLabel "has maternal cousin"@en ;
	skos:scopeNote "In 1.0.0 we are not distinguishing biological, adoptive, half, and step relationships."@en ;
	.

tolo:hasMaternalGrandfather
	a owl:ObjectProperty ;
	rdfs:subPropertyOf
		bdo:hasGrandfather ,
		tolo:hasMaternalGrandparent
		;
	owl:propertyChainAxiom (
		tolo:hasMother
		tolo:hasFather
	) ;
	skos:definition "Relates a person to his/her mother's father."@en ;
	skos:prefLabel "has maternal grandfather"@en ;
	skos:scopeNote "In 1.0.0 we are not distinguishing biological, adoptive, half, and step relationships."@en ;
	.

tolo:hasMaternalGrandmother
	a owl:ObjectProperty ;
	rdfs:subPropertyOf
		bdo:hasGrandmother ,
		tolo:hasMaternalGrandparent
		;
	owl:propertyChainAxiom (
		bdo:hasMother
		bdo:hasMother
	) ;
	skos:definition "Relates a person to his/her mother's mother."@en ;
	skos:prefLabel "has maternal grandmother"@en ;
	skos:scopeNote "In 1.0.0 we are not distinguishing biological, adoptive, half, and step relationships."@en ;
	.

tolo:hasMaternalGrandparent
	a owl:ObjectProperty ;
	rdfs:subPropertyOf bdo:hasGrandmother ;
	owl:propertyChainAxiom (
		bdo:hasMother
		bdo:hasParent
	) ;
	skos:definition "Relates a person to his/her mother's parent."@en ;
	skos:prefLabel "has maternal grandmother"@en ;
	skos:scopeNote "In 1.0.0 we are not distinguishing biological, adoptive, half, and step relationships."@en ;
	.

tolo:hasMember
	a owl:ObjectProperty ;
	owl:inverseOf tolo:isMemberOf ;
	skos:definition "Relates any kind of grouping to a resource that is a member of it."@en ;
	skos:editorialNote "Could use gist."@en ;
	skos:prefLabel "has member"@en ;
	.

tolo:hasNext
	a owl:ObjectProperty ;
	rdfs:domain tolo:OrderedMember ;
	rdfs:range tolo:OrderedMember ;
	skos:definition "Relates an ordered member in an ordered collection to the immediately following ordered member."@en ;
	skos:prefLabel "has next"@en ;
	skos:scopeNote "This predicate is more convenient to use than tolo:index: when modifying the ordering of collection members it requires only moving a single pointer rather than resequencing the entire collection."@en ;
	.

tolo:hasOrderedMember
	a owl:ObjectProperty ;
	rdfs:subPropertyOf tolo:hasMember ;
	rdfs:domain tolo:OrderedCollection ;
	rdfs:range tolo:OrderedMember ;
	skos:definition "Relates an ordered collection to an ordered member belonging to it."@en ;
	skos:prefLabel "has ordered member"@en ;
	skos:scopeNote "Note that the ordered members of the collection are the proxies of the resources that we typically think of as belonging to a collection, not these resources themselves."@en ;
	.

tolo:hasPaternalGrandfather
	a owl:ObjectProperty ;
	rdfs:subPropertyOf
		bdo:hasGrandfather ,
		tolo:hasPaternalGrandparent
		;
	owl:propertyChainAxiom (
		bdo:hasFather
		bdo:hasFather
	) ;
	skos:definition "Relates a person to his/her father's father."@en ;
	skos:prefLabel "has paternal grandfather"@en ;
	skos:scopeNote "In 1.0.0 we are not distinguishing biological, adoptive, half, and step relationships."@en ;
	.

tolo:hasPaternalGrandmother
	a owl:ObjectProperty ;
	rdfs:subPropertyOf
		bdo:hasGrandmother ,
		tolo:hasPaternalGrandparent
		;
	owl:propertyChainAxiom (
		bdo:hasFather
		bdo:hasMother
	) ;
	skos:definition "Relates a person to his/her father's mother."@en ;
	skos:prefLabel "has paternal grandmother"@en ;
	skos:scopeNote "In 1.0.0 we are not distinguishing biological, adoptive, half, and step relationships."@en ;
	.

tolo:hasPaternalGrandparent
	a owl:ObjectProperty ;
	rdfs:subPropertyOf bdo:hasGrandparent ;
	owl:propertyChainAxiom (
		bdo:hasFather
		bdo:hasParent
	) ;
	skos:definition "Relates a person to his/her fathers's parent."@en ;
	skos:prefLabel "has maternal grandmother"@en ;
	skos:scopeNote "In 1.0.0 we are not distinguishing biological, adoptive, half, and step relationships."@en ;
	.

tolo:hasSororallNephew
	a owl:ObjectProperty ;
	rdfs:subPropertyOf bdo:hasNephew ;
	owl:propertyChainAxiom (
		bdo:hasSister
		bdo:hasSon
	) ;
	skos:definition "Relates a person to his/her sister's son."@en ;
	skos:prefLabel "has sororal nephew"@en ;
	skos:scopeNote
		"In 1.0.0 we are not distinguishing biological, adoptive, half, and step relationships."@en ,
		"While a nephew can be related through either a sibling or sibling-in-law, a sororal nephew is always related through a sister."@en
		;
	.

tolo:hasSororallNiece
	a owl:ObjectProperty ;
	rdfs:subPropertyOf bdo:hasNiece ;
	owl:propertyChainAxiom (
		bdo:hasSister
		bdo:hasDaughter
	) ;
	skos:definition "Relates a person to his/her sister's daughter."@en ;
	skos:prefLabel "has sororal niece"@en ;
	skos:scopeNote
		"In 1.0.0 we are not distinguishing biological, adoptive, half, and step relationships."@en ,
		"While a niece can be related through either a sibling or sibling-in-law, a sororal nephew is always related through a sister."@en
		;
	.

tolo:index
	a owl:DatatypeProperty ;
	rdfs:domain tolo:Proxy ;
	skos:definition "The position of an ordered member in an ordered collection."@en ;
	skos:prefLabel "index"@en ;
	.

tolo:isMemberOf
	a owl:ObjectProperty ;
	owl:inverseOf tolo:hasMember ;
	skos:definition "Relates any kind of grouping to a resource that is a member of it."@en ;
	skos:editorialNote "Could use gist."@en ;
	skos:prefLabel "is member of"@en ;
	.

tolo:isOrderedMemberOf
	a owl:ObjectProperty ;
	rdfs:subPropertyOf tolo:isMemberOf ;
	owl:inverseOf tolo:hasOrderedMember ;
	skos:definition "Relates an ordered member to the ordered collection it belongs to."@en ;
	skos:prefLabel "is ordered member of"@en ;
	skos:scopeNote "Note that the ordered members of the collection are the proxies of the resources that we typically think of as belonging to a collection, not these resources themselves."@en ;
	.

tolo:isProxyFor
	a owl:ObjectProperty ;
	rdfs:domain tolo:OrderedMember ;
	skos:definition "Relates an ordered member to the non-literal resource it represents in an ordered collection, in order to express positional and other information that relate to the resource only in the context of the collection."@en ;
	skos:editorialNote "If we need to model ordered collections of literals, we may need two predicates, isProxyForObject and isProxyForLiteral, or to wrap the literal in an object like tolo:Text."@en ;
	skos:prefLabel "is proxy for"@en ;
	.

tolo:isSpouseIn
	a owl:ObjectProperty ;
	rdfs:domain tolo:Person ;
	rdfs:range tolo:Marriage ;
	skos:definition "This person is one of two spouses in a marital relationship."@en ;
	skos:prefLabel "is spouse in"@en ;
	.

tolo:name
	a owl:DatatypeProperty ;
	rdfs:range xsd:string ;
	skos:definition "A word or set of words by which a person, animal, place, or thing is known, addressed, or referred to."@en ;
	skos:prefLabel "name"@en ;
	.

tolo:nameVariant
	a owl:DatatypeProperty ;
	rdfs:subPropertyOf tolo:name ;
	skos:definition "A variant form of a person's name."@en ;
	skos:editoralNote "Explain more about how these differ from the primary name."@en ;
	skos:prefLabel "name variant"@en ;
	.

tolo:numberOfMembers
	a owl:DatatypeProperty ;
	rdfs:range xsd:integer ;
	skos:definition "The number of resources in a collection or other grouping."@en ;
	skos:prefLabel "number of members"@en ;
	.

tolo:primaryName
	a owl:DatatypeProperty ;
	rdfs:subPropertyOf tolo:name ;
	skos:definition "The primary form of a person's name."@en ;
	skos:prefLabel "primary name"@en ;
	.

tolo:primaryTitle
	a owl:DatatypeProperty ;
	rdfs:subPropertyOf tolo:title ;
	rdfs:domain tolo:Person ;
	skos:definition "The primary form of a person's title."@en ;
	skos:prefLabel "primary title"@en ;
	.

tolo:start
	a owl:DatatypeProperty ;
	skos:definition "The date, time, or datetime some event, relationship, or other thing started."@en ;
	skos:prefLabel "start"@en ;
	skos:scopeNote "May be used with edtf:EDTF datatyped strings to allow for partial, uncertain, and approximate dates."@en ;
	.

tolo:title
	a owl:DatatypeProperty ;
	rdfs:domain tolo:Person ;
	rdfs:range xsd:string ;
	skos:definition "An appellation of dignity, honor, distinction, or preeminence attached to a person or family by virtue of rank, office, precedent, privilege, attainment, or lands."@en ;
	skos:prefLabel "title"@en ;
	.

tolo:titleVariant
	a owl:DatatypeProperty ;
	rdfs:subPropertyOf tolo:title ;
	rdfs:domain tolo:Person ;
	skos:definition "A variant form of a person's title."@en ;
	skos:editoralNote "Explain more about how these differ from the primary name."@en ;
	skos:prefLabel "title variant"@en ;
	.

