# imports: http://purl.bdrc.io/ontology/core/

@prefix bdo: <http://purl.bdrc.io/ontology/core/> .
@prefix dct: <http://purl.org/dc/terms/> .
@prefix dctype: <http://purl.org/dc/dcmitype/> .
@prefix foaf: <http://xmlns.com/foaf/0.1/> .
@prefix owl: <http://www.w3.org/2002/07/owl#> .
@prefix rdf: <http://www.w3.org/1999/02/22-rdf-syntax-ns#> .
@prefix rdfs: <http://www.w3.org/2000/01/rdf-schema#> .
@prefix skos: <http://www.w3.org/2004/02/skos/core#> .
@prefix tolo: <https://ontologies.treasuryoflives/tolo/> .
@prefix vann: <http://purl.org/vocab/vann/> .
@prefix xml: <http://www.w3.org/XML/1998/namespace> .
@prefix xsd: <http://www.w3.org/2001/XMLSchema#> .

tolo:core
	a owl:Ontology ;
	dct:license "TBD"^^xsd:string ;
	vann:preferredNamespacePrefix "tolo"^^xsd:string ;
	owl:imports <http://purl.bdrc.io/ontology/core/> ;
	owl:versionIRI <https://ontologies.treasuryoflives/tolo/core/1.0.0> ;
	skos:definition "The Treasury of Lives Core Ontology enables the description of historical and contemporary figures in the culture and religion of Tibet, Inner Asia, and the Himalaya. It is used by the Treasury of Lives born-digitial biographical collection (https://treasuryoflives.org) to publish and share its data as Linked Open Data, as well as to enhance the narrative text with structured data."@en ;
	skos:editoralNote
		"Add rdfs:isDefinedBy using onto-toolkit, but keep in source files."@en ,
		"Combining all terms into one module for now; maybe break up into separate modules later."@en ,
		"Figure out issues of namespacing, ontology IRI, and versioning."@en
		;
	skos:prefLabel "Treasury of Lives Core Ontology"@en ;
	.

tolo:Category
	a owl:Class ;
	rdfs:subClassOf skos:Concept ;
	skos:definition "A type of concept used to categorize things."@en ;
	skos:editorialNote
		"Consider whether we want to use just skos:Concept directly."@en ,
		"Could use gist."@en
		;
	skos:example "Male and female are categories (instances) of Gender."@en ;
	skos:prefLabel "Category"@en ;
	skos:scopeNote "A category is typically a term in a controlled vocabulary. The Category class can be subclassed for specific vocabularies; e.g., Gender is a subclass of Category."@en ;
	.

tolo:Century
	rdfs:subClassOf tolo:HistoricalPeriod ;
	skos:definition "A historical century."@en ;
	skos:example "8th century AD, 2nd century BC."@en ;
	skos:prefLabel "Century"@en ;
	.

tolo:Collection
	a owl:Class ;
	rdfs:subClassOf
		dctype:Collection ,
		[
			a owl:Restriction ;
			owl:onProperty tolo:numberOfMembers ;
			owl:cardinality "1"^^xsd:nonNegativeInteger ;
		] ,
		[
			a owl:Restriction ;
			owl:onProperty tolo:hasMember ;
			owl:minCardinality "1"^^xsd:nonNegativeInteger ;
		]
		;
	skos:definition "An aggregation of resources."@en ;
	skos:editorialNote "Could use gist."@en ;
	skos:prefLabel "Collection"@en ;
	.

tolo:FraternalNiece
	a owl:ObjectProperty ;
	rdfs:subPropertyOf bdo:hasNiece ;
	owl:propertyChainAxiom (
		bdo:hasBrother
		bdo:hasSon
	) ;
	skos:definition "Relates a person to the daughter of his/her brother."@en ;
	skos:prefLabel "has fraternal niece"@en ;
	skos:scopeNote
		"In 1.0.0 we are not distinguishing biological, adoptive, half, and step relationships."@en ,
		"While a niece can be related through either a sibling or sibling-in-law, a fraternal niece is always related through a brother."@en
		;
	.

tolo:Gender
	rdfs:subClassOf tolo:Category ;
	skos:definition "A person or animal's biological sex."@en ;
	skos:example "Male, female."@en ;
	skos:prefLabel "Gender"@en ;
	.

tolo:GenealogicalGrouping
	a owl:Class ;
	rdfs:subClassOf
		tolo:Collection ,
		[
			a owl:Restriction ;
			owl:onProperty tolo:isMemberOf ;
			owl:allValuesFrom tolo:GenealogicalGrouping ;
		] ,
		[
			a owl:Restriction ;
			owl:onProperty tolo:hasMember ;
			owl:allValuesFrom [
				owl:unionOf (
					tolo:Person
					tolo:GenealogicalGrouping
				) ;
			] ;
		]
		;
	skos:definition "A social unit consisting of people with a common ancestor."@en ;
	skos:editorialNote
		"Are there other terms included besides family and clan?"@en ,
		"Improve definition to include adoption."^^xsd:string
		;
	skos:example "Nuclear family, extended family, clan."@en ;
	skos:prefLabel "Genealogical grouping"@en ;
	skos:scopeNote
		"No subclasses, such as family and clan, are defined because the distinctions are not clear-cut. Instead, we use partitive relationships to describe the relationships between different groupings."@en ,
		"This class encompasses successively larger and more inclusive genealogical groupings, such as family and clan. A person is said to be a member of a genealogical grouping, and a smaller genealogical grouping is a member of a larger one."@en
		;
	.

tolo:HistoricalPeriod
	skos:definition "A historical period."@en ;
	skos:example "8th century AD, 2nd century BC."@en ;
	skos:prefLabel "Historical period"@en ;
	.

tolo:Location
	a owl:Class ;
	skos:definition "A real, fictional, or imaginary place."@en ;
	skos:prefLabel "Location"@en ;
	.

tolo:Marriage
	a owl:Class ;
	rdfs:subClassOf tolo:TemporalRelation ;
	skos:definition ""@en ;
	skos:prefLabel "Marriage"@en ;
	.

tolo:OrderedCollection
	a owl:Class ;
	rdfs:subClassOf tolo:Collection ;
	owl:equivalentClass [
		owl:intersectionOf (
			tolo:Collection
			[
				a owl:Restriction ;
				owl:onProperty [
					owl:inverseOf tolo:isProxyIn ;
				] ;
				owl:minCardinality "1"^^xsd:nonNegativeInteger ;
			]
		) ;
	] ;
	skos:definition "A collection in which resources are ordered into a sequence."@en ;
	skos:editorialNote "TODO We could formalize this by stating every proxy has index 1, and/or at least one previous, and/or at least one next. Note that because there can be proxies with the same rank, there could be more than one previous or more than one next."^^xsd:string ;
	skos:prefLabel "Ordered collection"@en ;
	skos:scopeNote "The items in an OrderedCollection are not fixed over time but may be reordered."@en ;
	.

tolo:Person
	a owl:Class ;
	rdfs:subClassOf
		bdo:Person ,
		foaf:Person
		;
	skos:definition "A human being, alive, dead, imaginary, or fictional."@en ;
	skos:editorialNote "Note that this aligns with schema:Person but not gist:Person, since the latter does not include fictional persons. Though we can consider whether we need to include them. It maybe advantageous since we don't always know whether someone was real or not (?). Will this cause problems? Do we then need a class RealThing to assert that some people are real and others not?"@en ;
	skos:prefLabel "Person"@en ;
	.

tolo:Proxy
	owl:equivalentClass [
		owl:intersectionOf (
			[
				a owl:Restriction ;
				owl:onProperty tolo:isProxyFor ;
				owl:cardinality "1"^^xsd:nonNegativeInteger ;
			]
			[
				a owl:Restriction ;
				owl:onProperty tolo:isProxyIn ;
				owl:cardinality "1"^^xsd:nonNegativeInteger ;
			]
			[
				a owl:Restriction ;
				owl:onProperty tolo:index ;
				owl:cardinality "1"^^xsd:nonNegativeInteger ;
			]
		) ;
	] ;
	skos:definition "The representation of a resource as it exists in a specific Collection. This object both represents the position of an item in an ordered collection, and carries properties that apply to an item only in the context of the Collection."@en ;
	skos:example "The proxy of a teacher in a teaching lineage can indicate both the person's position in the lineage and the date the person became a member of the lineage."@en ;
	skos:prefLabel "Proxy"@en ;
	skos:scopeNote "An index is required but, based on the Open World Assumption, does not have to be asserted. This avoids the problem of resetting indices in case of changes to the OrderedCollection. Only the hasNext pointer would have to be moved."@en ;
	.

tolo:StrictlyOrderedCollection
	a owl:Class ;
	rdfs:subClassOf tolo:OrderedCollection ;
	skos:definition "A strict OrderedCollection - i.e., one in which no two items may have the same index."@en ;
	skos:editorialNote
		"TODO This can be formalized by stating that every element has index of 1, and/or exactly one next, an/dor exactly one previous; and none have the same index."@en ,
		"We may not need this. Are some lineages strictly ordered and others not?"@en
		;
	skos:prefLabel "Strictly ordered collection"@en ;
	.

tolo:TemporalRelation
	a owl:Class ;
	rdfs:subClassOf
		[
			a owl:Restriction ;
			owl:onProperty tolo:end ;
			owl:cardinality "1"^^xsd:nonNegativeInteger ;
		] ,
		[
			a owl:Restriction ;
			owl:onProperty tolo:start ;
			owl:cardinality "1"^^xsd:nonNegativeInteger ;
		]
		;
	skos:definition "A time-delimited relationship between two or more things."@en ;
	skos:editorialNote "Could use gist."@en ;
	skos:example
		"A marriage"@en ,
		"A teacher-student relationship."@en ,
		"An employment relationship between employer and employee."@en
		;
	skos:prefLabel "Temporal relation"@en ;
	skos:scopeNote "This class is used to materialize a relationship in order to make other assertions about it, such as start and end datetimes, location, and so on. Start and end dates/times may not be known or specified, but the relationship is in theory time-bound."@en ;
	.

tolo:birthdate
	a owl:DatatypeProperty ;
	rdfs:subPropertyOf tolo:start ;
	skos:definition "The date, time, or datetime that a person was born."@en ;
	skos:prefLabel "birthdate"^^xsd:string ;
	skos:scopeNote "Can be used with edtf:EDTF datatyped strings to allow for partial, uncertain, and approximate dates."@en ;
	.

tolo:categorizedBy
	a owl:DatatypeProperty ;
	rdfs:range tolo:Category ;
	skos:definition "Designates a category that is applied to the subject."@en ;
	skos:editorialNote "Could use gist."@en ;
	skos:example "Wencheng Kongjo is categorized by the Gender category 'female.'"@en ;
	skos:prefLabel "categorized by"@en ;
	.

tolo:deathDate
	a owl:DatatypeProperty ;
	rdfs:subPropertyOf tolo:end ;
	skos:definition "The date, time, or datetime that a person died."@en ;
	skos:prefLabel "death date"^^xsd:string ;
	skos:scopeNote "Can be used with edtf:EDTF datatyped strings to allow for partial, uncertain, and approximate dates."@en ;
	.

tolo:description
	a owl:DatatypeProperty ;
	skos:definition "A statement about someone or something's attributes or characteristics."@en ;
	skos:example "Nyenyo Jagoshong is a Sakya monastery in Tashigang, Tsang. It was founded by Panchen Bumdrak Sumpa in 1490."@en ;
	skos:prefLabel "description"@en ;
	.

tolo:dissolutionDate
	a owl:DatatypeProperty ;
	skos:definition "The date a marriage was ended through divorce rather than the death of one of the spouses."@en ;
	skos:editorialNote "Use if we need to distinguish divorce from death as the end of a marriage. Might make broader to include dissolution of other types of relationships. In that case, maybe move to tolo_core."@en ;
	skos:prefLabel "dissolution date"^^xsd:string ;
	.

tolo:end
	a owl:DatatypeProperty ;
	skos:definition "The date, time, or datetime some event, relationship, or other thing ended."@en ;
	skos:prefLabel "end"^^xsd:string ;
	skos:scopeNote "Can be used with edtf:EDTF datatyped strings to allow for partial, uncertain, and approximate dates."@en ;
	.

tolo:hasFraternalCousin
	a owl:ObjectProperty ;
	rdfs:subPropertyOf bdo:hasCousin ;
	skos:definition "Relates a person to his/her cousin on the father's side."@en ;
	skos:prefLabel "has fraternal cousin"@en ;
	skos:scopeNote "In 1.0.0 we are not distinguishing biological, adoptive, half, and step relationships."@en ;
	.

tolo:hasFraternalNephew
	a owl:ObjectProperty ;
	rdfs:subPropertyOf bdo:hasNephew ;
	owl:propertyChainAxiom (
		bdo:hasBrother
		bdo:hasSon
	) ;
	skos:definition "Relates a person to the son of his/her brother."@en ;
	skos:prefLabel "has fraternal nephew"@en ;
	skos:scopeNote
		"In 1.0.0 we are not distinguishing biological, adoptive, half, and step relationships."@en ,
		"While a nephew can be related through either a sibling or sibling-in-law, a fraternal nephew is always related through a brother."@en
		;
	.

tolo:hasGender
	a owl:ObjectProperty ;
	rdfs:range tolo:Gender ;
	skos:definition ""^^xsd:string ;
	skos:prefLabel "has gender"@en ;
	.

tolo:hasMaternalCousin
	a owl:ObjectProperty ;
	rdfs:subPropertyOf bdo:hasCousin ;
	skos:definition "Relates a person to his/her cousin on the mother's side."@en ;
	skos:prefLabel "has maternal cousin"@en ;
	skos:scopeNote "In 1.0.0 we are not distinguishing biological, adoptive, half, and step relationships."@en ;
	.

tolo:hasMaternalGrandfather
	a owl:ObjectProperty ;
	rdfs:subPropertyOf
		bdo:hasGrandfather ,
		tolo:hasMaternalGrandparent
		;
	owl:propertyChainAxiom (
		tolo:hasMother
		tolo:hasFather
	) ;
	skos:definition "Relates a person to his/her mother's father."@en ;
	skos:prefLabel "has maternal grandfather"@en ;
	skos:scopeNote "In 1.0.0 we are not distinguishing biological, adoptive, half, and step relationships."@en ;
	.

tolo:hasMaternalGrandmother
	a owl:ObjectProperty ;
	rdfs:subPropertyOf
		bdo:hasGrandmother ,
		tolo:hasMaternalGrandparent
		;
	owl:propertyChainAxiom (
		bdo:hasMother
		bdo:hasMother
	) ;
	skos:definition "Relates a person to his/her mother's mother."@en ;
	skos:prefLabel "has maternal grandmother"@en ;
	skos:scopeNote "In 1.0.0 we are not distinguishing biological, adoptive, half, and step relationships."@en ;
	.

tolo:hasMaternalGrandparent
	a owl:ObjectProperty ;
	rdfs:subPropertyOf bdo:hasGrandmother ;
	owl:propertyChainAxiom (
		bdo:hasMother
		bdo:hasParent
	) ;
	skos:definition "Relates a person to his/her mother's parent."@en ;
	skos:prefLabel "has maternal grandmother"@en ;
	skos:scopeNote "In 1.0.0 we are not distinguishing biological, adoptive, half, and step relationships."@en ;
	.

tolo:hasMember
	a owl:ObjectProperty ;
	owl:inverseOf tolo:isMemberOf ;
	skos:definition "Relates any kind of grouping to a resource that is a member of it."@en ;
	skos:editorialNote "Could use gist."@en ;
	skos:prefLabel "has member"@en ;
	skos:scopeNote
		"The members of an OrderedCollection are either its proxies or the resources represented by the proxies. Use ^isProxyIn to refer specifically to proxies."@en ,
		"This is a specific partitive predicate designed to avoid the ambiguities of a general 'hasPart' predicate."@en
		;
	.

tolo:hasNext
	a owl:ObjectProperty ;
	rdfs:domain tolo:Proxy ;
	rdfs:range tolo:Proxy ;
	owl:inverseOf tolo:hasPrevious ;
	skos:definition "Relates a Proxy in an OrderedCollection to the immediately following Proxy."@en ;
	skos:editorialNote "For now not defining the inverse hasPrevious"@en ;
	skos:prefLabel "has next"@en ;
	.

tolo:hasPaternalGrandfather
	a owl:ObjectProperty ;
	rdfs:subPropertyOf
		bdo:hasGrandfather ,
		tolo:hasPaternalGrandparent
		;
	owl:propertyChainAxiom (
		bdo:hasFather
		bdo:hasFather
	) ;
	skos:definition "Relates a person to his/her father's father."@en ;
	skos:prefLabel "has paternal grandfather"@en ;
	skos:scopeNote "In 1.0.0 we are not distinguishing biological, adoptive, half, and step relationships."@en ;
	.

tolo:hasPaternalGrandmother
	a owl:ObjectProperty ;
	rdfs:subPropertyOf
		bdo:hasGrandmother ,
		tolo:hasPaternalGrandparent
		;
	owl:propertyChainAxiom (
		bdo:hasFather
		bdo:hasMother
	) ;
	skos:definition "Relates a person to his/her father's mother."@en ;
	skos:prefLabel "has paternal grandmother"@en ;
	skos:scopeNote "In 1.0.0 we are not distinguishing biological, adoptive, half, and step relationships."@en ;
	.

tolo:hasPaternalGrandparent
	a owl:ObjectProperty ;
	rdfs:subPropertyOf bdo:hasGrandparent ;
	owl:propertyChainAxiom (
		bdo:hasFather
		bdo:hasParent
	) ;
	skos:definition "Relates a person to his/her fathers's parent."@en ;
	skos:prefLabel "has maternal grandmother"@en ;
	skos:scopeNote "In 1.0.0 we are not distinguishing biological, adoptive, half, and step relationships."@en ;
	.

tolo:hasSororallNephew
	a owl:ObjectProperty ;
	rdfs:subPropertyOf bdo:hasNephew ;
	owl:propertyChainAxiom (
		bdo:hasSister
		bdo:hasSon
	) ;
	skos:definition "Relates a person to his/her sister's son."@en ;
	skos:prefLabel "has sororal nephew"@en ;
	skos:scopeNote
		"In 1.0.0 we are not distinguishing biological, adoptive, half, and step relationships."@en ,
		"While a nephew can be related through either a sibling or sibling-in-law, a sororal nephew is always related through a sister."@en
		;
	.

tolo:hasSororallNiece
	a owl:ObjectProperty ;
	rdfs:subPropertyOf bdo:hasNiece ;
	owl:propertyChainAxiom (
		bdo:hasSister
		bdo:hasDaughter
	) ;
	skos:definition "Relates a person to his/her sister's daughter."@en ;
	skos:prefLabel "has sororal niece"@en ;
	skos:scopeNote
		"In 1.0.0 we are not distinguishing biological, adoptive, half, and step relationships."@en ,
		"While a niece can be related through either a sibling or sibling-in-law, a sororal nephew is always related through a sister."@en
		;
	.

tolo:hasSpouseRole
	a owl:ObjectProperty ;
	skos:editorialNote
		"TODO: finish"@en ,
		"links a person to his/her spouse through a Marriage relationship"@en
		;
	skos:prefLabel "has spouse role"^^xsd:string ;
	.

tolo:index
	a owl:DatatypeProperty ;
	rdfs:domain tolo:Proxy ;
	skos:definition "The position of a Proxy in an OrderedCollection."@en ;
	skos:prefLabel "index"^^xsd:string ;
	.

tolo:isMemberOf
	a owl:ObjectProperty ;
	owl:inverseOf tolo:hasMember ;
	skos:definition "Relates any kind of grouping to a resource that is a member of it."@en ;
	skos:editorialNote "Could use gist."@en ;
	skos:prefLabel "is member of"@en ;
	skos:scopeNote
		"The members of an OrderedCollection are either its proxies or the resources represented by the proxies. Use ^isProxyIn to refer specifically to proxies."@en ,
		"This is a specific partitive predicate designed to avoid the ambiguities of a general 'isPartOf' predicate."@en
		;
	.

tolo:isProxyFor
	a owl:ObjectProperty ;
	rdfs:domain tolo:Proxy ;
	skos:definition "Relates a Proxy to the resource it represents in an OrderedCollection."@en ;
	skos:prefLabel "is proxy for"@en ;
	.

tolo:isProxyIn
	a owl:ObjectProperty ;
	rdfs:domain tolo:Proxy ;
	rdfs:range tolo:OrderedCollection ;
	skos:definition "Relates a Proxy to the OrderedCollection it belongs to."@en ;
	skos:prefLabel "is proxy in"@en ;
	.

tolo:name
	a owl:DatatypeProperty ;
	skos:definition "A word or set of words by which a person, animal, place, or thing is known, addressed, or referred to."@en ;
	skos:editorialNote
		"Could use gist."@en ,
		"Do we need to distinguish name variant from just name? In that case, do we also need primary name? Would name variant apply only to persons, or to other things as well?"@en
		;
	skos:prefLabel "name"@en ;
	.

tolo:numberOfMembers
	a owl:DatatypeProperty ;
	skos:definition "The number of resources in a Collection or other grouping."@en ;
	skos:prefLabel "number of members"^^xsd:string ;
	.

tolo:start
	a owl:DatatypeProperty ;
	skos:definition "The date, time, or datetime some event, relationship, or other thing started."@en ;
	skos:prefLabel "start"^^xsd:string ;
	skos:scopeNote "Can be used with edtf:EDTF datatyped strings to allow for partial, uncertain, and approximate dates."@en ;
	.

tolo:title
	a owl:DatatypeProperty ;
	rdfs:domain tolo:Person ;
	skos:definition "An appellation of dignity, honor, distinction, or preeminence attached to a person or family by virtue of rank, office, precedent, privilege, attainment, or lands."@en ;
	skos:prefLabel "title"@en ;
	.

